# Условие
Проверить и получить формулу для кубического сплайна
# Решение
$S_{3, 2}\left( x \right) = a_{i_{0}} + a_{i_{1}}\left( x - x_{i} \right) + a_{i_{2}}\left( x - x_{i} \right)^{2} + a_{i_{3}}\left( x - x_{i} \right)^{3}$
$t = \dfrac{x - x_{i}}{h_{i}}$

Рассмотрим отрезок $\left[ x_{i}, x_{i + 1} \right]$
$h = h_{i}$
$S\left( x_{i} \right) = a_{0} = f_{i}$
$S'\left( x_{i} \right) = a_{1} = f'_{i}$
$S\left( x_{i + 1} \right) = a_{0} + a_{1}\cdot h + a_{2}\cdot h^{2} + a_{3}\cdot h^{3} = f_{i + 1}$
$S'\left( x_{i + 1} \right) = a_{1} + 2a_{2}\cdot h + 3a_{3}\cdot h^{2} = f'_{i + 1}$

$\begin{cases} a_{3}h^{3} + a_{2}h^{2} = f_{i + 1} - f_{i} - f'_{i}\cdot h \\ 3a_{3}h^{2} + 2 a_{2}h = f'_{i + 1} - f'_{i} \end{cases}$
$\begin{cases} 2a_{3}h^{3} + 2a_{2}h^{2} = 2f_{i + 1} - 2f_{i} - 2f_{fi}' \cdot h  \\ 3a_{3}h^{3} + 2a_{2}h^{2} = \left( f'_{i + 1} - f'_{i} \right) \cdot h \end{cases}$
$\implies \left( f'_{i + 1} - f'_{i} \right) \cdot h - 3a_{3}h^{3} = 2f_{i + 1} - 2f_{i} - 2f_{fi}' \cdot h - 2a_{3}h^{3}$
$a_{3} = \dfrac{\left( f'_{i + 1} - f'_{i} \right) \cdot h - 2\left( f_{i + 1} - f_{i} - f_{fi}' \cdot h \right)}{h^{3}} = \dfrac{\left( f'_{i + 1} + f'_{i} \right)\cdot h - 2\left( f_{i + 1} - f_{i} \right)}{h^{3}}$
$a_{2} = -\dfrac{\left( f_{i + 1}' + 2f_{i}' \right)h - 3\left( f_{i + 1} - f_{i} \right)}{h^{2}}$

$S\left( x \right) = a_{3}h^{3}t^{3} + a_{2}h^{2}t^{2} + f'_{i}th + f_{i}$
$S\left( x \right) = h_{i}\left( f'_{i + 1} + f'_{i} \right)t^{3} - 2\left( f_{i + 1} \right)$