**Метод квадратного корня**
	$A = LU$
	$U = DV$

	$D = \begin{pmatrix}d_1 & 0 & \ldots & 0 \\ 0 & d_2 & \ldots & 0 \\ \ldots & \ldots & \ldots & \ldots \\ 0 & 0 & \ldots & d_n\end{pmatrix}$
	$V = \begin{pmatrix}1 & V_{12} & \ldots & V_{1n} \\ 0 & 1 & \ldots & V_{2n} \\ \ldots & \ldots & \ldots & \ldots \\ 0 & 0 & \ldots & 1\end{pmatrix}$
	$d_{i} = u_{ii}$
	$v_{ij} = \dfrac{u_{ij}}{u_{ii}}$

	$A = LDV$

	$A = A^{T}$
	$A^{T} = (LDV)^{T} = V^{T}D^{T}L^{T} = V^{T}DL^{T}=A$
	$LDV = A$

	$L = V^{T}$
	$V = L^{T}$

	$A = V^{T}DV$

$(Ax, x) > 0$
$(Dx, x) > 0$

$x = Vy$
$(Dx, x) = (DVy, Vy) = (V^{T}DVy, y) = (Ay, y) > 0$
	$d_{i} > 0$

$D^{1/2} =$ матрице $D$, с извлечённым корнем из каждого элемента



$A = V^{T}D^{1/2}D^{1/2}V$
$A = W^{T}W$

$Ax = f$
$W^{T}Wx = f$
$W^{T}y = f$
$Wx = y$


---

$a_{ij} = \sum \limits_{ k = 1 } ^{ n } W^{T}_{ik}W_{kj} = \sum \limits_{ k = 1 } ^{ i }W_{ki}W_{kj} = a_{ij}$

$a_{11} = W_{11} W_{11}$
$W_{11} = \sqrt{ a_{11 }}$

$a_{1j} = W_{11}W_{1j}  \quad   \quad w_{1j} = \dfrac{a_{1j}}{w_{11}}$

$a_{ii} = \sum \limits_{ k = 1 } ^{ i }W_{ki}W_{ki} = \sum \limits_{ k = 1 } ^{ i - 1 }W_{ki}^{2} + W_{ii}^{2}$
$W_{ii} = \sqrt{ a_{ii} - \sum \limits_{ k=1 }^{ i - 1 }W_{ki}^{2} }$
$a_{ij} = \sum \limits_{ k=1 }^{ i - 1 } W_{ki}W_{kj} + W_{ii}W_{ij}$
$W_{ij} = \dfrac{a_{ii} - \sum \limits_{ k=1 }^{ i - 1 }W_{ki}W_{kj}}{W_{ii}}  \quad   \quad j = i + 1, \ldots, n$


# QR разложение

$(p, x) = p_{1}x_{1} + p_{2}x_{2} + \ldots + p_{n}x_{n} = 0$
$p = \begin{pmatrix}p_1\\ p_2\\ \ldots \\ p_n\end{pmatrix}$


$y = x - 2\frac{(p, x)}{(p, p)}p = x - \frac{2}{(p, p)}(p, x) \cdot p = x - \frac{2}{(p, p)}pp^{T}x = \underbrace{ \left( I - \frac{2}{(p, p)}pp^{T} \right) }_{ P }x$

$P = I - \frac{2}{(p, p)} pp^{T}$

---
1. $p^{2} = I$
	$P^{2}x = P(Px) = P\left( x - 2 \frac{p, x}{(p, p)}p \right)= Px - 2\frac{p, x}{(p, p)}Pp = Px - 2 \frac{p, x}{(p, p)}\left( p - 2\frac{p, p}{(p, p)}p \right) = x - 2\frac{(p, x)}{(p, p)}p + 2\frac{(p, x)}{(p, p)}p = x$
2. $P^{T} = P$
	$P^{T} = \left( I - \frac{2}{(p, p)}pp^{T} \right)^{T} = I - \frac{2}{(p, p)}(p^{T})^{T} p^{T} = P$
3. $P^{T} \cdot P = P^{2} = I$
4. Если взять вместо $p$, $\beta p$, $P$ не изменится 
	$P = I - \frac{2}{(\beta p, \beta p)}(\beta p)(\beta p)^{T} = I - \frac{2}{(\beta, p)}pp^{T}$
5. $P = x - y$
	$x - y = \underbrace{ 2\frac{(p, x)}{(p, p)} }_{ \beta }p$
6. $p_{1} = p_{2} = \ldots = p_{k} = 0$
	$y_{1} = x_{1},  \quad y_{2} = x_{2},  \quad  \ldots,  \quad  y_{k} = x_{k}$
	$y_{i} = x_{i} - \frac{2p_{i}}{\sum \limits_{ l=1 }^{ n }p_{i}^{2}}\sum \limits_{ k=1 }^{ n }p_{k}x_{k}$