$$
A_{k - 1} = \begin{pmatrix}
a_{11}^{(1)} & a_{12}^{(1)} & \ldots & a_{1k-1}^{(1)} & a_{1k}^{(1)} & a_{1k + 1}^{(1)} & \ldots & a_{1n}^{(1)} \\
0  & a_{22}^{(2)} &  \ldots & a_{2k - 1}^{(2)} & a_{2k}^{(2)} & a_{2k + 1}^{(2)} & \ldots & a_{2n}^{2} \\
\ldots & \ldots & \ldots & \ldots & \ldots & \ldots & \ldots & \ldots \\
0 & 0 & \ldots & a_{k - 1, k - 1}^{(k - 1)} & a_{k - 1, k}^{(k - 1)} & a_{k - 1, k + 1}^{(k - 1)} & \ldots & a_{k - 1, n}^{(k - 1)}
\end{pmatrix}
$$
$$
a_{k}^{(k)} = P_{k}a_{k}^{(k - 1)} = \begin{pmatrix}
a_{1k}^{(1)}  \\
a_{2k}^{(2)}  \\
\ldots \\
a_{k - 1, k}^{(k - 1)} \\
a_{k, k}^{(k)} \\
0 \\
\ldots
\end{pmatrix}
$$
$$
p^{(k)} = a_{k}^{(k - 1)} - a_{k}^{(k)}
$$
$$
\begin{align}
p_{e}^{(k)} = 0, & e = 1, 2, \ldots, k - 1 \\
p_{k}^{(k)} = a_{kk}^{(k - 1)} - a_{}
\end{align}
$$