# 1
$$
u_{xx} - 2\sin \left( x \right) u_{xy} - \cos ^{2}\left( x \right) u_{yy} - \cos \left( x \right) u_{y} = 0
$$
$$
a = 1;\ b = -\sin \left( x \right);\ c= - \cos ^{2}\left( x \right) 
$$
$$
D = \sin^{2}\left( x \right) + \cos ^{2}\left( x \right) = 1 >0 - \text{гиперболический тип}
$$
## Характеристическое уравнение
$$
dy^{2} + 2\sin \left( x \right) dxdy - \cos ^{2}\left( x \right) dx^{2} = 0
$$
$$
dy = \left(-\sin \left( x \right) \pm 1 \right) dx
$$
$$
\begin{cases}
y = \cos \left( x \right) + x & \xi = y - x - \cos \left( x \right)  \\
y = \cos \left( x \right) - x   & \zeta = y + x - \cos \left( x \right) 
\end{cases} 
$$
$$
\begin{cases}
u_{y} = u_{\xi} + u_{\zeta} \\
u_{xx} = u_{\xi\xi} \left( -1 + \sin \left( x \right)  \right) ^{2} + 2u_{\xi\xi} \left( -1 + \sin \left( x \right)  \right) \left( 1 + \sin \left( x \right)  \right)  + u_{\zeta\zeta}\left( 1 + \sin \left( x \right)  \right) ^{2} + u_{\xi} \cdot \cos \left( x \right) + u_{\zeta}\cos \left( x \right)  \\
u_{xy} = u_{\xi\xi}\left( -1 + \sin \left( x \right)  \right)  + u_{\xi\zeta}\left( -1 + \sin \left( x \right)  + 1 + \sin \left( x \right)  \right)  + u_{\zeta\zeta}\left( 1 - \sin \left( x \right)  \right)  \\
u_{yy} = u_{\xi\zeta} + 2u_{\xi\zeta} + u_{\zeta\zeta}
\end{cases}
$$
$$
u_{\xi\xi}\left( \sin ^{2}\left( x \right)  - 2\sin \left( x \right) + 1 \right) - 2 u_{\xi\zeta}\cos ^{2}\left( x \right) + u_{\zeta\zeta}\left( \sin ^{2}\left( x \right)  + 2\sin \left( x \right) + 1 \right) + \cos \left( x \right) \left( u_{\xi} + u_{\zeta} \right) - 2u_{\xi\xi}\left( -\sin \left( x \right)  + \sin ^{2}\left( x \right)  \right) - 4u_{\xi@\zeta}\sin ^{2}\left( x \right)  - 2u_{\zeta\zeta}\left( \sin \left( x \right)  - \sin ^{2}\left( x \right)  \right)  -
$$
$$
- u_{\xi\xi}\cos ^{2}\left( x \right) - 2 \cos ^{2}\left( x \right) u_{\xi\zeta} - \cos ^{2}\left( x \right) \cdot u_{\zeta\zeta} - \cos \left( u_{\xi} + u_{\zeta} \right) = 0
$$
$$
u_{\xi\xi}\left( \sin ^{2}\left( x \right) - 2 \sin \left( x \right)  + 1 + 2 \sin \left( x \right)  - 2 \sin ^{2}\left( x \right)  - \cos ^{2}\left( x \right)  \right) - 
$$
$$
- u_{\xi\zeta}\left( 2 \cos ^{2}\left( x \right)  + 4 \sin ^{2}\left( x \right)  + 2 \cos ^{2}\left( x \right)  \right) + u_{\zeta\zeta} \left( \sin ^{2}\left( x \right)  + 2 \sin \left( x \right)  + 1 - 2\sin \left( x \right) - 2 \sin ^{2}\left( x \right) - \cos ^{2}\left( x \right)  \right) = 0
$$
$$
- 4u_{\xi\zeta} = 0 \implies u_{\xi\zeta} = 0
$$
$$
u\left( \xi, \zeta \right)  = f_{1}\left( x \right)  + f_{2}\left( \zeta \right) 
$$
$$
u\left( x, y \right) = f_{1}y - x - \cos \left( x \right) + f_{2}\left( y + x - \cos \left( x \right)  \right) 
$$
# 2
$$
x^{2}u_{xx} - y^{2}u_{yy} - 2yu_{y} = 0
$$
## Характеристическое уравнение
$$
x^{2}dy^{2} - y^{2}dx^{2} = 0
$$
$$
\begin{cases}
xdy - ydx = 0 & \dfrac{dx}{x} = \dfrac{dy}{y} & \ln \left( x \right) = \ln \left( y \right)  + C_{1} & \xi = \dfrac x y\\
xdy + ydx = 0 & \dfrac{dx}{x} = - \dfrac{dy}{y} & \ln \left( x \right) = -\ln \left( y \right)  + C_{2} & \zeta = xy
\end{cases}
$$
$$
u_{y} = - u _{\xi}\cdot\dfrac x {y^{2}} + u_{\zeta} \cdot x
$$
$$
u_{xx} = u_{\xi\xi} \cdot \dfrac{1}{y^{2}} + 2 u_{\xi\zeta} + u_{\zeta\zeta}\cdot y^{2}
$$
$$
u_{yy} = u_{\xi\xi}\cdot\dfrac{x^{2}}{y^{4}}- 2u_{\xi\zeta} \dfrac{x^{2}}{y^{2}} + u_{\zeta\zeta} \cdot x^{2} + u_{\xi}\dfrac{2x}{y^{3}}
$$
$$
u_{\xi\xi}\cdot\dfrac{x^{2}}{y^{2}} + u_{\xi\zeta}\cdot_{2}x^{2} + u_{\zeta\zeta} \cdot x^{2}y^{2} - u_{\xi\xi} \dfrac{x^{2}}{y^{2}} + u_{\xi\zeta} \cdot 2 x^{2} - u_{\zeta\zeta}x^{2}y^{2} - u_{\xi}\cdot_{2}\dfrac{x}{y} + u_{\xi}\cdot_{2}\dfrac{x}{y} - 2xy u_{\zeta} = 0
$$
$$
4x^{2}u_{\xi\zeta} - 2xy \cdot u_{\zeta}
$$