# Линейное однородное вчп 1-го порядка
$$
(1) \quad  a_{1}\left( x, y, z \right) \dfrac{\partial u}{\partial x} + a_{2}\left( x, y, z \right) \dfrac{\partial u}{\partial y} + a_{3}\left( x, y, z \right) \dfrac{\partial u}{\partial z} = 0
$$
# Квазилинейное неоднородное вчп 1-го порядка
$$
\left( 2 \right)  \quad a_{1}\left( x, y, z \right) \dfrac{\partial z}{\partial x} + a_{2}\left( x, y, z \right)\dfrac{\partial z}{\partial y}  = a_{3}\left( x, y, z \right)  
$$
# Характеристические уравнения
$$
\dfrac{dx}{a_{1}\left( x, y, z \right) } = \dfrac{dy}{a_{2}\left( x, y, z \right) } = \dfrac{dz}{a_{3}\left( x,y, z \right) }
$$
$$
\begin{cases}
\phi_{1}\left( x, y, z \right) = C_{1} \\
\phi_{2}\left( x, y, z \right) = C_{2}
\end{cases} \implies \begin{matrix}
1) & u\left( x, y, z \right) = \Phi \left( \phi_{1}\left( x, y, z \right) , \phi_{2}\left( x, y, z \right)  \right) \\
2)  & \Phi \left( \phi_{1}\left( x, y, z \right) , \phi_{2}\left( x, y, z \right) = 0 \right)  
\end{matrix}
$$
# №1
$$
\left( z - y \right) ^{2}\dfrac{\partial u}{\partial x} + z \dfrac{\partial u}{\partial y} + y \dfrac{\partial u}{\partial z} = 0
$$
$$
u\left( 0, y, z \right) = 2y\left( y - z \right) 
$$
## Характеристическое уравнение
$$
\dfrac{dx}{\left( z - y \right) ^{2}} = \dfrac{dy}{z} = \dfrac{dz}{y}
$$
## Решение
$$
\dfrac{dy}{z}=\dfrac{dz}{y}
$$
$$
y^{2} - z^{2} = C_{1} = \phi_{1}
$$
$$
\dfrac{dy}{z} = \dfrac{dz}{y} = \dfrac{dz - dy}{y - z} = \dfrac{d\left( z - y \right) }{-\left( z - y \right) }
$$
$$
\dfrac{dx}{\left( z - y \right) ^{2}} = \dfrac{d\left( z - y \right) }{- \left( z - y \right) }
$$
$$
dx = -\left( z - y \right) d\left( z - y \right)
$$
$$
x = - \dfrac 1 2 \left( z - y \right) ^{2} + C_{2}
$$
$$
x + \dfrac 1 2 \left( z - y \right) ^{2} = C_{2} = \phi_{2}\left( x, y, z \right) 
$$
$$
u\left( x, y, z \right) = \Phi \left( y^{2} - z^{2}, x + \dfrac 1 2 \left( z - y \right) ^{2} \right) 
$$

$$
\begin{cases}
u\left( 0, y, z \right)  = 2y\left( y - z \right)  \\
\phi_{1}\left( 0, y, z \right) = y^{2} - z^{2} \\
\phi_{2}\left( 0, y, z \right) = \dfrac 1 2 \left( z - y \right) ^{2}
\end{cases}
$$
$$
2\phi_{2} + \phi_{1} = 2y\left( y - z \right)  = u
$$
$$
u\left( x, y, z \right)  = 2x + \left( z - y \right) ^{2} + y^{2} - z^{2}
$$
# №2
$$
\dfrac{\partial z}{\partial x} + \left( 2y - z \right) \dfrac{\partial z}{\partial y} = y + 2z
$$
## Характеристическое
$$
\dfrac{dx}{1} = \dfrac{dy}{2y - z} = \dfrac
$$