---
Owner: Artemii
tags:
  - Практика
---
$\mathsf{  
a_0 y^{(n)} + \ldots a_{n - 1}y' + a_n y = f(x)  
}$

$\mathsf{  
e^{\lambda i x}  
}$

  

# №1

![[IMG_20240514_122204.jpg]]

# №2

$\mathsf{  
y'' - y = 2e^x - x^2  
}$

$\mathsf{  
\lambda^2 - 1= 0  
}$

$\mathsf{  
\lambda = \pm 1  
}$

$\mathsf{  
y_{оо} = C_1e^x + C_2 e^{-x}  
}$

  

$\mathsf{  
y_{чн1} = 2e^x = Ae^x \cdot x  
}$

$\mathsf{  
y_{чн2} = -x^2 = Bx^2 + Cx + D  
}$

  

$\mathsf{  
y_{чн2} = 1x^2 + 2  
}$

  

$\mathsf{  
Ae^x + Axe^x - Ae^x \cdot x = 2e^x - x^2  
}$

$\mathsf{  
A = 2 - \dfrac{x^2}{e^x}  
}$

  

$\mathsf{  
y_{чн1} = 2e^x \cdot x - x^3  
}$

  

$\mathsf{  
y = C_1e^x + C_2 e^{-x} + 2e^x \cdot x - x^3 + x^2 + 2  
}$

  

# №3

$\mathsf{  
y'' + y' - 2y = 3x e^x  
}$

$\mathsf{  
\lambda_1 = 1  
}$

$\mathsf{  
\lambda = -2  
}$

  

$\mathsf{  
y_{оо} = C_1 e^x + C_2e^{-2x}  
}$

  

Так как e^x это решение, повышаем на максимальную кратность корня

$\mathsf{  
y_{чн} = (Ax^2 + Bx + C) e^x  
}$

  

  

544-548

549-559