Можно смотреть по второй производной
# №2
$f(x) = 3 \sqrt[3]{ x^2 } - x^2$
$f'(x) = 2 \cdot \frac{1}{\sqrt[3]{x} } - 2x$
$$f'(x) = 0 \iff \begin{cases}
2 - 2x \sqrt[3]{ x } = 0  & x = \pm 1 \\
x \neq 0
\end{cases}$$
$f''(x) = - \dfrac 2 3 x^{- \frac 4 3} - 2$
$f''(1) = - \dfrac 2 3 - 2 < 0$
$(1; 2) - max$

# №3
$f(x) = x \cdot e^{\frac{x^2}{2}}$
$f'(x) = e^{\frac{x^2}{2}} + x^2 \cdot e^{\frac{x^2}{2}}$
$f'' = 0$
$(- \infty; + \infty)$ - $f$ возрастает

# №4
$f(x) = \dfrac{x^3}{3} - x^2 - 3x$
$f'(x)  = x^2 - 2x - 3$

$$x^2 - 2x - 3 = 0 \iff \begin{cases}
x_{1} = \dfrac{2 + \sqrt{ 26 }}{2} \\
x_{2} = \dfrac{2 - \sqrt{ 26 }}{2}
\end{cases}$$

$f(0) = 0$ - max
$f(1) = \dfrac 1 3 - 1 - 3 =$

