$$
\dfrac{\partial^{2}u}{\partial t^{2}}=a^{2}\dfrac{\partial^{2}u}{\partial x^{2}}
$$
$$
u\left( x, t \right) = \theta _{1}\left( x - at \right) + \theta _{2}\left( x + at \right)
$$
$$
u_{1}\left( x, t \right) = \theta _{1}\left( x - at \right)
$$
$$
\begin{cases}
\dfrac{\partial u_{1}}{\partial x} = \theta _{1}'\left( x - at \right) \cdot 1 & \dfrac{\partial^{2}u_{1}}{\partial x^{2}} = \theta ''_{1}\left( x - at \right) \cdot 1^{2} \\
\dfrac{\partial u_{1}}{\partial t} = \theta _{1}'\left( x - at \right) \left( -a \right) & \dfrac{\partial^{2} u_{1}}{\partial t^{2}} = \theta''_{1}\left( x - at \right) \left( -a \right) ^{2}
\end{cases}
$$
$$
\dfrac{\partial^{2}u_{1}}{\partial t^{2}} - a^{2}\dfrac{\partial^{2}u_{1}}{\partial x^{2}} = 0
$$
$$
\begin{cases}
u_{1} - \text{прямая волна} \\
u_{2} - \text{обратная волна}
\end{cases}
$$
