$$
\dfrac{\partial^{2}u}{\partial t^{2}} = a^{2} \dfrac{\partial^{2}u}{\partial x^{2}}
$$
$$
u \lvert_{t = 0} = \phi\left( x \right), \quad \dfrac{\partial u}{\partial t} \lvert_{t = 0} = \psi\left( x \right)  
$$
$$
u\left( x, t \right)  = \dfrac{\phi\left( x - at \right)  + \phi\left(x + at \right) }{x + at} + \frac{1}{2a}\int \limits_{ x - at }^{ x + at } \psi \left( \xi \right) d\xi
$$
$$
\dfrac{\partial u}{\partial t}|_{t=0} = \dfrac{( \phi' \cdot (-a) + \phi'(a) )}{2} + \dfrac{1}{2a} \left[ \psi(x+at)\cdot a - \psi(x-at) \cdot(-a) \right] \lvert_{t = 0} = \psi(x)
$$

$$
\int \limits_{ x - at }^{ x + at } \psi \left( \xi \right) d\xi = \int \limits_{ 0 }^{ x + at } \psi \left( x \right) d\xi - \int \limits_{ 0 }^{ x - at } \psi \left( x \right) d\xi 
$$


$$
v(x, t, \tau) = \dfrac 1 {2a} \int\limits_{x-a(t-\tau)}^{x+a(t-\tau)} f(\xi, \tau) d\xi \quad x\in R
$$
$$
u(x, t) = \int\limits_0^t v(x, t, \tau) d\tau
$$
$$
v\left( x, t, t \right)  = 0, \quad  \frac{\partial v}{\partial t}\left( x, t, t \right) = f\left( x, t \right) , \quad \frac{\partial^{2} v }{\partial t^{2}} = a^{2}\frac{\partial^{2}v}{\partial x^{2}} + \cancel{ f\left( x, t \right) }
$$
$$
u\left( x, 0 \right) = \int \limits_{ 0 }^{ 0 } v\left( x, 0, \tau \right) = 0
$$
$$
\dfrac{\partial u}{\partial t}\lvert_{t = 0} = v\left( x, t, t \right)  + \int \limits_{ 0 }^{ t } \dfrac{\partial v\left( x, t, \tau \right) }{\partial t}
$$
$$
\dfrac{\partial u}{\partial t} = \int\limits_0^t \dfrac{\partial v(x, t, \tau}{\partial t} d\tau
$$
$$
\dfrac{\partial^2 u}{\partial t^2} \dfrac{\partial v(x, t, t)}{\partial t} + \int\limits_0^t \dfrac{\partial^2 v(x, t, \tau)}{\partial t^2} d\tau
$$
$$
\dfrac{\partial^2 u}{\partial x^2} = \int\limits_0^t \dfrac{\partial^2 v(x, t, \tau)}{\partial x^2} d\tau
$$
$$
\dfrac{\partial^2 u}{\partial t^2} - a^2\dfrac{\partial^2 u}{\partial x^2} = f(x, t)
$$
