---
Редакторы: Artemii
Тэги:
  - II семестр
  - Практика
Дата: Invalid date
Статус: Готово
---
$\mathsf  
{  
f(x, y) = c  
}$

$\mathsf  
{  
c  
}$ - линия уровня

  

  

$\mathsf{u = \sqrt{1 - x^2 - y^2}}$

$\mathsf  
{  
1 - (x^2 + y^2) \ge 0  
}$

$\mathsf  
{  
1 \ge x^2 + y^2  
}$

  

  

$\mathsf  
{  
c = 0;\quad \sqrt{1 - x^2 - y^2} = 0}$

$\mathsf  
{  
1 - x^2 - y^2 = 0  
}$

$\mathsf  
{  
1 = x^2 + y^2  
}$

  

$\mathsf  
{  
c = \dfrac 1 2; \quad \sqrt{1 - x^2 - y^2} = \dfrac 1 2  
}$

$\mathsf  
{  
\dfrac 3 4 = x^2 + y^2  
}$

![[/Untitled 34.png|Untitled 34.png]]

  

  

![[/Untitled 1 13.png|Untitled 1 13.png]]

  

![[IMG_20230530_123003.jpg]]

  

$\mathsf  
{  
u = \dfrac{1}{\sqrt{xy}}  
}$

$\mathsf{xy \gt 0}$

  

$\mathsf  
{  
c = 1;\quad xy = 1  
}$

  

$\mathsf  
{  
c = 2; \quad xy = \dfrac 1 4  
}$

  

$\mathsf  
{  
c = \dfrac 1 2; \quad xy = 4  
}$

  

![[/Untitled 2 12.png|Untitled 2 12.png]]

НЕ ВКЛЮЧАЯ ГРАНИЦЫ

  

![[/Untitled 3 10.png|Untitled 3 10.png]]

  

  

  

$\mathsf  
{  
\underset{\underset{y \to y_0}{x \to x_0}}\lim f(x, y) = b  
}$

$\mathsf  
{  
\underset{y \to y_0} \lim (\underset{x \to x_0} \lim (f(x, y)))  
}$

$\mathsf  
{  
\underset{x \to x_0} \lim (\underset{y \to y_0} \lim(f(x, y)))  
}$

  

$\mathsf  
{  
f(x, y) = \dfrac{x^y}{1 + x^y}, \quad \begin{matrix}  
\mathsf{x \to \infin} \\  
\mathsf{y \to +0}  
\end{matrix}  
}$

$\mathsf  
{  
\underset{y \to +0} \lim (\underset{x \to \infin} \lim (\dfrac{x^y}{1 + x^y})) = \underset{y \to +0} \lim (\underset{x \to \infin} \lim\left(\dfrac{x^y(1)}{x^y(\dfrac 1 {x^y} + 1)}\right)) = \underset{y \to +0} \lim 1 = 1  
}$

$\mathsf  
{  
\underset{y \to +0} \lim (\underset{x \to \infin} \lim\left(\dfrac{x^y}{1 + x^y}\right)) = \underset{x \to \infin} \lim \dfrac 1 2 = \dfrac 1 2  
}$

  

  

$\mathsf  
{  
f(x, y) = \dfrac{x^2 y^2}{x^2 y^2 + (x - y)^2},\quad  
\begin{matrix}  
\mathsf{x \to 0} \\  
\mathsf{x \to 0}  
\end{matrix}  
}$

$\mathsf  
{  
\underset{y \to 0} \lim (\underset{x \to 0} \lim \left( \dfrac{x^2 y^2}{x^2 y^2 + (x - y)^2} \right)) = \underset{y \to 0} \lim \dfrac 0 {y^2} = \underset{y \to 0} \lim 0 = 0  
}$

$\mathsf  
{  
\underset{x \to 0} \lim (\underset{y \to 0} \lim \left( \dfrac{x^2 t^2}{x^2 y^2 + (x - y)^2} \right)) =\underset{x \to 0} \lim \dfrac 0 {x^2} = 0  
}$

$\mathsf  
{  
\underset{\underset{\underset {y = kx}{y \to 0}}{x \to 0}} \lim \dfrac{x^4 k^2}{x^4 k^2 + (x - kx)^2} = \underset{\underset{\underset {y = kx}{y \to 0}}{x \to 0}} \lim \dfrac{x^2 \cdot x^2 \cdot k^2}{x^2(x^2 k^2 + (1 - k)^2)} = \underset{\underset{\underset {y = kx}{y \to 0}}{x \to 0}} \lim \dfrac{x^2 k^2}{x^2 k^2 + (1 - k)^2} = \begin{cases}  
\mathsf{0,}& \mathsf{k \neq 1} \\  
\mathsf{1,}& \mathsf{k = 1}  
\end{cases}  
}$

![[/Untitled 4 6.png|Untitled 4 6.png]]

  

$\mathsf  
{  
f(x, y) = x^2 \cdot e^{-(x^2 - y)}, \quad  
\begin{matrix}  
\mathsf{x = y \cdot \cos(\alpha)} \\  
\mathsf{y = t \cdot \sin(\alpha}  
\end{matrix},\quad t \to +\infin  
}$