# №796~
## Условие
$$
\begin{cases}
x' = x - y + z \\
y' = x + y - z \\
z' = 2x - y + 0z
\end{cases}
$$
## Решение
$$
\begin{pmatrix}
1 & -1 & 1 \\
1 & 1 & -1 \\
2 & -1 & 0
\end{pmatrix}
$$
$$
\begin{vmatrix}
1 - \lambda & -1 & 1 \\
1 & 1 - \lambda & -1 \\
2 & -1 & -\lambda
\end{vmatrix} = (1 - x)x^{2} - (1 - x)x + 2x - 2 = 0
$$
$$
(1 - x)\left[ x^{2} - x \right] + 2x  -2 = 0 \\

$$
# №797~
# №798~
# №799~
# №800~
# №801~
# №802~
# №803~
# №804~
# №805~
# №806~
# №807~
# №808~
# №809~
# №810~
# №811~
# №812~