# №796
## Условие
$$
\begin{cases}
x' = x - y + z \\
y' = x + y - z \\
z' = 2x - y + 0z
\end{cases}
$$
## Решение
$$
\begin{pmatrix}
1 & -1 & 1 \\
1 & 1 & -1 \\
2 & -1 & 0
\end{pmatrix}
$$
$$
\begin{vmatrix}
1 - \lambda & -1 & 1 \\
1 & 1 - \lambda & -1 \\
2 & -1 & -\lambda
\end{vmatrix} = (1 - \lambda)\lambda^{2} - (1 - \lambda)\lambda + 2\lambda - 2 = 0
$$
$$
\begin{align}
(1 - \lambda)\left[ \lambda^{2} - \lambda \right] -(2 - 2\lambda) = 0 \\
(1 - \lambda)\left[ \lambda^{2} - \lambda - 2 \right] = 0 \\ 
\end{align}
$$
$$
\begin{align}
\lambda_{1} = 1 \\
\lambda_{2} = 2 \\
\lambda_{3} = -1
\end{align}
$$

### $\lambda_{1}$
$$
\begin{pmatrix}
0 & -1 & 1 \\
1 & 0 & -1 \\
2 & -1 & -1
\end{pmatrix} \cdot \begin{pmatrix}
\alpha \\
\beta \\
\gamma
\end{pmatrix} = 0
$$
$$
\begin{cases}
-\beta + \gamma = 0 & \alpha = \alpha = 1 \\
\alpha - \gamma = 0 & \beta = \alpha \\
2\alpha - \beta - \gamma = 0 & \gamma = \alpha
\end{cases}  \quad V_{1} = \begin{pmatrix}
1 \\
1 \\
1
\end{pmatrix} 
$$
### $\lambda_{2}$
$$
\begin{cases}
-\alpha -\beta + \gamma = 0 & \alpha = \alpha = 1 \\
\alpha -\beta -\gamma = 0 & \beta = 0 \\
2\alpha -\beta -2\gamma = 0 & \gamma = \alpha
\end{cases}  \quad V_{2} = \begin{pmatrix}
1 \\
0 \\
1
\end{pmatrix} 
$$
### $\lambda_{3}$
$$
\begin{cases}
2\alpha -\beta + \gamma = 0 & \alpha = 0 \\
\alpha + 2 \beta -2\gamma = 0 & \beta = \beta = 1 \\
2\alpha -\beta + \gamma = 0 & \gamma = \beta
\end{cases}  \quad V_{3} = \begin{pmatrix}
0 \\
1 \\
1
\end{pmatrix} 
$$

## Ответ
$$
\begin{pmatrix}
x \\
y \\
z
\end{pmatrix} = \begin{pmatrix}
1 \\
1 \\
1
\end{pmatrix} C_{1}e^{t} + \begin{pmatrix}
1 \\
0 \\
1
\end{pmatrix} C_{2}e^{2t} + \begin{pmatrix}
0 \\
1 \\
1
\end{pmatrix}C_{3}e^{-t}
$$

# №797
## Условие
$$
\begin{cases}
x' = x - 2y - z \\
y' = -x + y + z \\
z' = x + 0y - z
\end{cases}
$$
$$
\begin{align}
\lambda_{1} = 0 \\
\lambda_{2} = 2 \\
\lambda_{3} = -1
\end{align}
$$
## Решение
### $\lambda_{1}$
$$
\begin{cases}
\alpha - 2\beta - \gamma = 0 & \alpha = \alpha = 1 \\
-\alpha + \beta + \gamma = 0 & \beta = 0 \\
\alpha - \gamma = 0 & \gamma = \alpha
\end{cases}  \quad V_{1} = \begin{pmatrix}
1 \\
0 \\
1
\end{pmatrix} 
$$
### $\lambda_{2}$
$$
\begin{cases}
-\alpha - 2\beta - \gamma = 0 & \alpha = 3\gamma \\
-\alpha -\beta + \gamma = 0 & \beta = -2\gamma \\
\alpha - 3\gamma = 0 & \gamma = \gamma = 1
\end{cases}  \quad V_{2} = \begin{pmatrix}
3 \\
-2 \\
1
\end{pmatrix} 
$$
### $\lambda_{3}$
$$
\begin{cases}
2\alpha - 2\beta - \gamma = 0 & \alpha = 0 \\
-\alpha + 2\beta + \gamma = 0 & \beta = -\frac{1}{2}\gamma \\
\alpha = 0 & \gamma = \gamma = 2
\end{cases}  \quad V_{3} = \begin{pmatrix}
0 \\
-1 \\
2
\end{pmatrix} 
$$
## Ответ
$$
\begin{pmatrix}
x \\
y \\
z
\end{pmatrix} = \begin{pmatrix}
1 \\
0 \\
1
\end{pmatrix}C_{1}e^{0t} + \begin{pmatrix}
3 \\
-2 \\
1
\end{pmatrix}C_{2}e^{2t} + \begin{pmatrix}
0 \\
-1 \\
2
\end{pmatrix}C_{3}e^{-t}
$$
# №798
## Условие
$$
\begin{cases}
x' = 2x - y + z \\
y' = x + 2y - z \\
z' = x - y + 2z
\end{cases}
$$
$$
\begin{align}
\lambda_{1} = 1 \\
\lambda_{2} = 2 \\
\lambda_{3} = 3
\end{align}
$$
## Решение
### $\lambda_{1}$
$$
\begin{cases}
\alpha - \beta + \gamma = 0 & \alpha = 0 \\
\alpha + \beta - \gamma = 0 & \beta = \beta = 1 \\
\alpha - \beta + \gamma = 0 & \gamma = 1
\end{cases}  \quad V_{1} = \begin{pmatrix}
0 \\
1 \\
1
\end{pmatrix} 
$$
### $\lambda_{2}$
$$
\begin{cases}
-\beta + \gamma = 0 & \alpha = \alpha = 1 \\
\alpha -\gamma = 0 & \beta = \alpha \\
\alpha - \beta = 0 & \gamma = \alpha
\end{cases}  \quad  V_{2} = \begin{pmatrix}
1 \\
1 \\
1
\end{pmatrix} 
$$
### $\lambda_{3}$
$$
\begin{cases}
-\alpha - \beta + \gamma = 0 & \alpha = \alpha = 1 \\
\alpha - \beta - \gamma = 0 & \beta = 0 \\
 \alpha - \beta - \gamma = 0 & \gamma = \alpha
\end{cases}  \quad V_{3} = \begin{pmatrix}
1 \\
0 \\
1
\end{pmatrix}  
$$
## Ответ
$$
\begin{pmatrix}
x \\
y \\
z
\end{pmatrix} = \begin{pmatrix}
0 \\
1 \\
1
\end{pmatrix}C_{1} e^{t} + \begin{pmatrix}
1 \\
1 \\
1
\end{pmatrix}C_{2}e^{2t} + \begin{pmatrix}
1 \\
0 \\
1
\end{pmatrix} C_{3}e^{3t}
$$
# №799
## Условие
$$
\begin{cases}
x' = 3x - y + z \\
y' = x + y + z \\
z' = 4x - y + 4z
\end{cases}
$$
$$
\begin{align}
\lambda_{1} = 1 \\
\lambda_{2} = 2 \\
\lambda_{3} = 5
\end{align}
$$
## Решение
### $\lambda_{1}$
$$
\begin{cases}
2\alpha - \beta + \gamma = 0 & \alpha = -\gamma \\
\alpha + \gamma = 0  & \beta = -\gamma\\
4\alpha - \beta + 3\gamma = 0 & \gamma = \gamma = -1
\end{cases} \quad V_{1} = \begin{pmatrix}
1 \\
1 \\
-1
\end{pmatrix}  
$$
### $\lambda_{2}$
$$
\begin{cases}
\alpha - \beta + \gamma = 0 & \alpha = -\frac{1}{3}\gamma \\
\alpha -\beta + \gamma = 0 & \beta = \frac{2}{3}\gamma \\
4\alpha - \beta + 2 \gamma = 0 & \gamma = \gamma = 3
\end{cases}  \quad V_{2} = \begin{pmatrix}
-1 \\
2 \\
3
\end{pmatrix} 
$$
### $\lambda_{3}$
$$
\begin{cases}
-2\alpha - \beta + \gamma & \alpha = \frac{1}{3}\gamma \\
\alpha - 4 \beta + \gamma & \beta = \frac{1}{3}\gamma \\
4 \alpha - \beta - \gamma = 0 & \gamma = \gamma = 3
\end{cases}  \quad V_{3} = \begin{pmatrix}
1 \\
1 \\
3
\end{pmatrix} 
$$
## Ответ
$$
\begin{pmatrix}
x \\
y \\
z
\end{pmatrix} = \begin{pmatrix}
1 \\
1 \\
-1
\end{pmatrix}C_{1}e^{t} + \begin{pmatrix}
-1 \\
2 \\
3
\end{pmatrix}C_{2}e^{2t} + \begin{pmatrix}
1 \\
1 \\
3
\end{pmatrix}C_{3}e^{5t}
$$

# №800
## Условие
$$
\begin{cases}
x' = -3x + 4y - 2z \\
y' = x + 0y + z \\
z' = 6x - 6y + 5z
\end{cases}
$$
$$
\begin{align}
\lambda_{1} = 1 \\
\lambda_{2} = 2 \\
\lambda_{3} = -1
\end{align}
$$
## Решение
### $\lambda_{1} = 1$
$$
\begin{cases}
-4\alpha + 4\beta - 2\gamma = 0 & \alpha = \alpha = 1 \\
\alpha - \beta + \gamma = 0 & \beta = \alpha \\
6\alpha - 6\beta + 4\gamma = 0 & \gamma = 0
\end{cases} \quad V_{1} = \begin{pmatrix}
1 \\
1 \\
0
\end{pmatrix} 
$$
### $\lambda_{2} = 2$
$$
\begin{cases}
-5\alpha + 4\beta - 2\gamma = 0 & \alpha = 0 \\
\alpha - 2\beta + \gamma = 0 & \beta = \beta = 1 \\
6\alpha - 6\beta + 3 \gamma = 0 & \gamma = 2\beta
\end{cases} \quad V_{2} = \begin{pmatrix}
0 \\
1 \\
2
\end{pmatrix} 
$$
### $\lambda_{3} = -1$
$$
\begin{cases}
-2\alpha + 4\beta - 2\gamma = 0 & \alpha = -\gamma \\
\alpha + \beta + \gamma = 0 & \beta = 0 \\
6\alpha - 6\beta + 6\gamma = 0 & \gamma = \gamma = 1
\end{cases} \quad V_{3} = \begin{pmatrix}
-1 \\
0 \\
1
\end{pmatrix} 
$$
## Ответ
$$
\begin{pmatrix}
x \\
y \\
z
\end{pmatrix} = \begin{pmatrix}
1 \\
1 \\
0
\end{pmatrix}C_{1}e^{t} + \begin{pmatrix}
0 \\
1 \\
2
\end{pmatrix} C_{2}e^{2t} + \begin{pmatrix}
-1 \\
0 \\
1
\end{pmatrix}C_{3}e^{-t}
$$
# №801
## Условие
$$
\begin{cases}
x' = x - y - z \\
y' = x + y + 0z \\
z' = 3x + 0y + z
\end{cases}
$$
$\lambda_{1} = 1,\ \lambda_{2, 3} = 1 \pm 2i$
## Решение
### $\lambda_{1} = 1$
$$
\begin{cases}
-\beta  -\gamma = 0 & \alpha = 0 \\
\alpha = 0 & \beta = -\gamma \\
3\alpha = 0 & \gamma = \gamma = 1
\end{cases}  \quad  V_{1} = \begin{pmatrix}
0 \\
-1 \\
1
\end{pmatrix} 
$$
### $\lambda_{2} = 1 - 2i$
$$
\begin{cases}
2i\alpha - \beta - \gamma = 0 & \alpha = -\frac{2}{3}i\gamma \\
\alpha + 2i\beta = 0 & \beta = \frac{1}{3}\gamma \\
3\alpha - \gamma + 2i\gamma = 0 & \gamma = \gamma = 3
\end{cases}  \quad  V_{2} = \begin{pmatrix}
-2i \\
1 \\
3
\end{pmatrix} 
$$

$$
V_{2} \cdot e^{(1 - 2i)t} = e^{t}\begin{pmatrix}
-2i \cdot \left( \cos(2t) - i \sin(2t) \right) \\
\cos(2t) - i \sin(2t) \\
3\cos(2t) - 3i \sin(2t)
\end{pmatrix} = e^{t} \begin{pmatrix}
-2i\cos(2t) + 2 \sin(2t) \\
-\cos(2t) + i\sin(2t) \\
3 \cos(2t) - 3i\sin(2t)
\end{pmatrix}
$$
## Ответ
$$
\begin{pmatrix}
x \\
y \\
z
\end{pmatrix} = e^{t}\left( \begin{pmatrix}
0 \\
-1 \\
1
\end{pmatrix}C_{1} + \begin{pmatrix}
2 \sin(2t) \\
-\cos(2t) \\
3 \cos(2t)
\end{pmatrix} C_{2} + \begin{pmatrix}
-2\cos(2t) \\
\sin(2t) \\
-3\sin(2t)
\end{pmatrix}C_{3} \right) 
$$

# №802
## Условие
$$
\begin{cases}
x' = 2x + y + 0z \\
y' = x + 3y - z \\
z' = -x + 2y + 3z
\end{cases}
$$
$$
\begin{align}
\lambda_{1} = 2 \\
\lambda_{2, 3} = 3 \pm i
\end{align}
$$
## Решение
### $\lambda_{1} = 2$
$$
\begin{cases}
\beta = 0 & \alpha = \gamma \\
\alpha + \beta - \gamma = 0 & \beta = 0 \\
-\alpha + 2\beta + \gamma = 0 & \gamma = \gamma = 1
\end{cases}  \quad V_{1} = \begin{pmatrix}
1 \\
0 \\
1
\end{pmatrix} 
$$
### $\lambda_{2} = 3 - i$
$$
\begin{cases}
(-1 + i)\alpha + \beta = 0 & \alpha = \frac{\gamma}{5}\left( 2 - i \right)  \\
\alpha + i\beta - \gamma = 0 & \beta = \frac{\gamma}{5} \left( 1 - 3i \right)  \\
-\alpha + 2\beta + i\gamma = 0 & \gamma = \gamma = 5
\end{cases}  \quad  V_{2} = \begin{pmatrix}
2 - i \\
1 - 3i \\
5
\end{pmatrix} 
$$
$$
e^{(3 - i) \cdot t} \cdot \begin{pmatrix}
2 - i \\
1 - 3i \\
5
\end{pmatrix} = e^{3t}\begin{pmatrix}
\left( 2 - i \right) \left( \cos(t) - i \sin(t) \right) \\
\left( 1 - 3i \right) \left( \cos(t) - i \sin(t) \right) \\
5 \left( \cos(t) - i \sin(t) \right)
\end{pmatrix} = \begin{pmatrix}
2 \cos(t) - i \cos(t) - 2i\sin(t) - \sin(t) \\
\cos(t) - 3i\cos(t) - i\sin(t) - 3\sin(t) \\
5\cos(t) - 5i\sin(t)
\end{pmatrix}
$$
## Ответ
$$
\begin{pmatrix}
x \\
y \\
z
\end{pmatrix} = \begin{pmatrix}
1 \\
0 \\
1
\end{pmatrix} C_{1}e^{2t} + e^{3t}\left[ \begin{pmatrix}
2 \cos(t) - \sin(t) \\
\cos(t) - 3\sin(t) \\
5\cos(t)
\end{pmatrix} C_{2} + \begin{pmatrix}
- \cos(t) - 2\sin(t)\\
- 3\cos(t) - \sin(t) \\
- 5\sin(t)
\end{pmatrix}C_{3} \right]
$$
# №803
## Условие
$$
\begin{cases}
x' = 2x - y + 2z \\
y' = x + 0y + 2z \\
z' = -2x + y - z
\end{cases}
$$
$$
\begin{align}
\lambda_{1} = 1 \\
\lambda_{2, 3} = \pm i
\end{align}
$$
## Решение
### $\lambda_{1} = 1$
$$
\begin{cases}
\alpha - \beta + 2\gamma = 0 & \alpha = 0 \\
\alpha - \beta + 2\gamma = 0 & \beta = 2\gamma \\
-2\alpha + \beta - 2\gamma = 0 & \gamma = \gamma = 1
\end{cases}  \quad  V_{1} = \begin{pmatrix}
0 \\
2 \\
1
\end{pmatrix} 
$$

### $\lambda_{2} = -i$
$$
\begin{cases}
(2 + i)\alpha - \beta + 2\gamma = 0 & \alpha = \gamma \left( -1 + i \right)  \\
\alpha + i\beta + 2\gamma = 0 & \beta = \gamma \left( -1 + i \right)  \\
-2\alpha + \beta + (-1 + i)\gamma = 0 & \gamma = \gamma = 1
\end{cases} \quad V_{2} = \begin{pmatrix}
-1 + i \\
-1 + i \\
1
\end{pmatrix} 
$$
$$
e^{-it}\cdot \begin{pmatrix}
-1 + i \\
-1 + i \\
1
\end{pmatrix} = \begin{pmatrix}
\left( -1 + i \right) \left( \cos(t) - i\sin(t) \right) \\
\left( -1 + i \right) \left( \cos(t) - i\sin(t) \right)  \\
\cos(t) - i\sin(t) 
\end{pmatrix} = \begin{pmatrix}
-\cos(t) + i\cos(t) + i\sin(t) + \sin(t) \\
-\cos(t) + i\cos(t) + i\sin(t) + \sin(t) \\
\cos(t) - i\sin(t)
\end{pmatrix}
$$
## Ответ
$$
\begin{pmatrix}
x \\
y \\
z
\end{pmatrix} = \begin{pmatrix}
0 \\
2 \\
1
\end{pmatrix}C_{1}e^{t} + \begin{pmatrix}
-\cos(t) + \sin(t) \\
-\cos(t) + \sin(t) \\
\cos(t)
\end{pmatrix} C_{2} + \begin{pmatrix}
\cos(t) + \sin(t) \\
\cos(t) + \sin(t) \\
\sin(t)
\end{pmatrix}C_{3}
$$

# №804
## Условие
$$
\begin{cases}
x' = 4x - y - z \\
y' = x + 2y - z \\
z' = x - y + 2z
\end{cases}
$$
$$
\begin{align}
\lambda_{1} = 2 \\
\lambda_{2, 3} = 3
\end{align}
$$
## Решение
### $\lambda_{1} = 2$
$$
\begin{cases}
2\alpha - \beta - \gamma = 0 & \alpha = \alpha = 1 \\
\alpha - \gamma = 0 & \beta = \alpha \\
\alpha - \beta = 0 & \gamma = \alpha
\end{cases} \quad V_{1} = \begin{pmatrix}
1 \\
1 \\
1
\end{pmatrix} 
$$
### $\lambda_{2, 3} = 3$
$$
\begin{cases}
\alpha - \beta - \gamma = 0 & \alpha = \beta + \gamma \\
\alpha - \beta - \gamma = 0 & \beta = \beta \\
\alpha - \beta - \gamma = 0 & \gamma = \gamma
\end{cases} \quad V_{2} = \begin{pmatrix}
2 \\
1 \\
1
\end{pmatrix} \quad V_{3} = \begin{pmatrix}
5 \\
3 \\
2
\end{pmatrix}
$$
## Ответ
$$
\begin{pmatrix}
x \\
y \\
z
\end{pmatrix} = \begin{pmatrix}
1 \\
1 \\
1
\end{pmatrix}C_{1}e^{2t} + \left( \begin{pmatrix}
2 \\
1 \\
1
\end{pmatrix}C_{2} + \begin{pmatrix}
5 \\
3 \\
2
\end{pmatrix}C_{3} \right)e^{3t}
$$
# №805
## Условие
$$
\begin{cases}
x' = 2x - y - z \\
y' = 3x - 2y - 3z \\
z' = -x + y + 2z
\end{cases}
$$
$$
\begin{align}
\lambda_{1} = 0 \\
\lambda_{2, 3} = 1
\end{align}
$$
## Решение
### $\lambda_{1} = 0$
$$
\begin{cases}
2\alpha - \beta - \gamma = 0 & \alpha = -\gamma \\
3\alpha - 2\beta - 3\gamma = 0 & \beta = -3\gamma \\
-\alpha + \beta + 2\gamma = 0 & \gamma = \gamma = -1
\end{cases} \quad V_{1} = \begin{pmatrix}
1 \\
3 \\
-1
\end{pmatrix} 
$$
### $\lambda_{2, 3} = 1$
$$
\begin{cases}
\alpha - \beta - \gamma = 0 & \alpha = \gamma + \beta \\
3\alpha - 3\beta - 3\gamma = 0 & \beta = \beta \\
-\alpha + \beta + \gamma = 0 & \gamma = \gamma
\end{cases} \quad V_{2} = \begin{pmatrix}
2 \\
1 \\
1
\end{pmatrix}  \quad V_{3} = \begin{pmatrix}
5 \\
3 \\
2
\end{pmatrix} 
$$
## Ответ
$$
\begin{pmatrix}
x \\
y \\
z
\end{pmatrix} = \begin{pmatrix}
1 \\
3 \\
-1
\end{pmatrix}C_{1} + \left[ \begin{pmatrix}
2 \\
1 \\
1
\end{pmatrix}C_{2} + \begin{pmatrix}
5 \\
3 \\
2
\end{pmatrix} C_{3} \right]e^{t}
$$
# №806
## Условие
$$
\begin{cases}
x' = -2x + y - 2z \\
y' = x - 2y + 2z \\
z' = 3x - 3y + 5z
\end{cases}
$$
$$
\begin{align}
\lambda_{1} = 3 \\
\lambda_{2, 3} = -1
\end{align}
$$
## Решение
### $\lambda_{1} = 3$
$$
\begin{cases}
-5\alpha + \beta - 2\gamma = 0 & \alpha = -\beta \\
\alpha - 5\beta + 2\gamma = 0 & \beta = \frac{1}{3}\gamma \\
3\alpha - 3\beta + 2\gamma = 0 & \gamma = \gamma = 3
\end{cases} \quad V_{1} = \begin{pmatrix}
-1 \\
1 \\
3
\end{pmatrix} 
$$
### $\lambda_{2, 3} = -1$
$$
\begin{cases}
-\alpha + \beta - 2\gamma = 0 & \alpha = \alpha \\
\alpha - \beta + 2\gamma = 0 & \beta = \beta \\
3\alpha - 3\beta + 6\gamma = 0 & \gamma = \frac{-\alpha + \beta}{2}
\end{cases} \quad V_{2} = \begin{pmatrix}
-1 \\
1 \\
1
\end{pmatrix} \quad V_{3} = \begin{pmatrix}
-1 \\
3 \\
2
\end{pmatrix} 
$$
## Ответ
$$
\begin{pmatrix}
x \\
y \\
z
\end{pmatrix} = \begin{pmatrix}
-1 \\
1 \\
3
\end{pmatrix}C_{1}e^{3t} \left( \begin{pmatrix}
-1 \\
1 \\
1
\end{pmatrix}C_{2} + \begin{pmatrix}
-1 \\
3 \\
2
\end{pmatrix}C_{3} \right) e^{-t}
$$
# №807
## Условие
$$
\begin{cases}
x' = 3x - 2y - z \\
y' = 3x - 4y - 3z \\
z' = 2x - 4y + 0z
\end{cases}
$$
$$
\begin{align}
\lambda_{1, 2} = 2 \\
\lambda_{3} = -5
\end{align}
$$
## Решение
### $\lambda_{1, 2} = 2$
$$
\begin{cases}
\alpha - 2\beta - \gamma = 0 & \alpha = \alpha \\
3\alpha - 6\beta - 3\gamma = 0 & \beta = \beta \\
2\alpha - 4\beta - 2\gamma = 0 & \gamma = \alpha - 2\beta
\end{cases} \quad V_{1} = \begin{pmatrix}
2 \\
1 \\
0
\end{pmatrix} \quad V_{2} = \begin{pmatrix}
3 \\
2 \\
-1
\end{pmatrix} 
$$
### $\lambda_{3} = -5$
$$
\begin{cases}
8\alpha - 2\beta - \gamma = 0 & \alpha = \frac{1}{2}\gamma \\
3\alpha + \beta - 3\gamma = 0 & \beta = \frac{3}{2}\gamma \\
2\alpha - 4\beta + 5\gamma = 0 & \gamma = \gamma = 2
\end{cases} \quad V_{3} = \begin{pmatrix}
1 \\
3 \\
2
\end{pmatrix} 
$$
## Ответ
$$
\begin{pmatrix}
x \\
y \\
z
\end{pmatrix} = 
\left( \begin{pmatrix}
2 \\
1 \\
0
\end{pmatrix}C_{1} + \begin{pmatrix}
3 \\
2 \\
-1
\end{pmatrix} C_{2} \right) e^{2t} + \begin{pmatrix}
1 \\
3 \\
2
\end{pmatrix}C_{3}e^{-5t}
$$
# №808
## Условие
$$
\begin{cases}
x' = x - y + z \\
y' = x + y - z \\
z' = 0x - y + 2z
\end{cases}
$$
$$
\begin{align}
\lambda_{1, 2} = 1 \\
\lambda_{3} = 2 
\end{align}
$$
## Решение
### $\lambda_{3} = 2$
$$
\begin{cases}
-\alpha - \beta + \gamma = 0 & \alpha = \gamma \\
\alpha - \beta - \gamma = 0 & \beta = 0 \\
-\beta = 0 & \gamma = \gamma = 1
\end{cases} \quad V_{3} = \begin{pmatrix}
1 \\
0 \\
1
\end{pmatrix} 
$$
### $\lambda_{1, 2} = 1$
$$
\begin{cases}
-\beta + \gamma = 0 & \alpha = \gamma \\
\alpha - \gamma = 0 & \beta = \gamma \\
-\beta + \gamma = 0 & \gamma = \gamma = 1
\end{cases} \quad V_{1} = \begin{pmatrix}
1 \\
1 \\
1
\end{pmatrix} 
$$

$2 > 3 - 2 = 1$
Ищем решение

$$
\begin{pmatrix}
at + b \\
ct + d \\
ft + g
\end{pmatrix}e^{t}
$$
$$
\begin{cases}
a + at + b = at + b - ct - d + ft + g & a = -ct - d + ft + g & a = f \\
c + ct + d = at + b + ct + d - ft - g & c = at + b - ft - g & c = b - g \\
f + ft + g = -ct - d + 2ft + 2g & f = -ct - d + ft + g
\end{cases}
$$
$$
\begin{cases}
0 = -c + f & a = -d + g \\
0 = at - ft & c = b - g \\
0 = -ct + ft & f = -d + g
\end{cases}
$$
$$
\begin{cases}
a = f \\
c = f \\
d = -b \\
f = - d + g \\
b = b \\
g = g
\end{cases}
$$
$$
\begin{cases}
a = C_{1} + C_{2} \\
c = C_{1} + C_{2} \\
d = -C_{1} \\
f = C_{1} + C_{2} \\
b = C_{1} \\
g = C_{2}
\end{cases}
$$
$$
\begin{pmatrix}
C_{1}t + C_{2}t + C_{1} \\
C_{1}t + C_{2}t -C_{1} \\
C_{1}t + C_{2}t + C_{2}
\end{pmatrix} e^{t}
$$

## Ответ
$$
\begin{pmatrix}
x \\
y \\
z
\end{pmatrix} = \begin{pmatrix}
C_{1}t + C_{2}t + C_{1} \\
C_{1}t + C_{2}t - C_{1} \\
C_{1}t + C_{2}t + C_{2}
\end{pmatrix}e^{t} + \begin{pmatrix}
1 \\
0 \\
1
\end{pmatrix}C_{3}e^{2t}
$$
# №809
## Условие
$$
\begin{cases}
x' = -x + y - 2z \\
y' = 4x + y + 0z \\
z' = 2x + y - z
\end{cases}
$$
$$
\begin{align}
\lambda_{1} = 1 \\
\lambda_{2, 3} = -1
\end{align}
$$
## Решение
### $\lambda_{1} = 1$
$$
\begin{cases}
-2\alpha + \beta - 2\gamma = 0 & \alpha = 0 \\
4\alpha = 0 & \beta = 2\gamma \\
2\alpha + \beta - 2\gamma = 0 & \gamma = \gamma = 1
\end{cases} \quad V_{1} = \begin{pmatrix}
0 \\
2 \\
1
\end{pmatrix} 
$$

### $\lambda_{2, 3} = -1$
$$
\begin{cases}
\beta - 2\gamma = 0 & \alpha = \gamma \\
4\alpha + 2\beta = 0 & \beta = -2\gamma \\
2\alpha + \beta = 0 & \gamma = \gamma
\end{cases}
$$
$3 - 2 = 1$

$$
\begin{pmatrix}
\alpha_{1}t + \beta_{1} \\
\alpha_{2}t + \beta_{2} \\
\alpha_{3}t + \beta_{3}
\end{pmatrix}e^{t}
$$
$$
\begin{cases}
\alpha_{1} - \alpha_{1} t - \beta_{1} = -\alpha_{1} t - \beta_{1} + \alpha_{2}t + \beta_{2} - 2\alpha_{3}t - 2\beta_{3} & \alpha_{1} = \alpha_{2}t + \beta_{2} - 2\alpha_{3}t - 2\beta_{3} \\
\alpha_{2} - \alpha_{2}t - \beta_{2} = 4\alpha_{1}t + 4\beta_{1} + \alpha_{2}t + \beta_{2} & \alpha_{2} = 4\alpha_{1}t + 4\beta_{1} + 2\alpha_{2}t + 2\beta_{2} \\
\alpha_{3} - \alpha_{3}t - \beta_{3} = 2\alpha_{1}t + 2\beta_{1} + \alpha_{2}t + \beta_{2} - \alpha_{3}t - \beta_{3} & \alpha_{3} = 2\alpha_{1}t + 2\beta_{1} + \alpha_{2}t + \beta_{2}
\end{cases}
$$
$$
\begin{cases}
0 = \alpha_{2} - 2\alpha_{3} & \alpha_{1} = \beta_{2} - 2\beta_{3} \\
0 = 4\alpha_{1} + 2\alpha_{2} & \alpha_{2} = 4\beta_{1} + 2\beta_{2} \\
0 = 2\alpha_{1} + \alpha_{2} & \alpha_{3} = 2\beta_{1} + \beta_{2}
\end{cases}
$$
$$
\begin{cases}
\alpha_{1} = C_{2} \\
\alpha_{2} = 2C_{2} \\
\alpha_{3} = C_{2} \\
\beta_{1} = -2C_{1} \\
\beta_{2} = C_{2} + 2 C_{1} \\
\beta_{3} = C_{1}
\end{cases}
$$
## Ответ
$$
\begin{pmatrix}
x \\
y \\
z
\end{pmatrix} = \begin{pmatrix}
0 \\
2 \\
1
\end{pmatrix} C_{3}e^{t} + \begin{pmatrix}
C_{2}t -2C_{1} \\
2C_{2}t + C_{2} + 2C_{1} \\
C_{2}t + C_{1}
\end{pmatrix}e^{-t}
$$
# №810~
## Условия
$$
\begin{cases}
x' = 2x + y + 0z \\
y' = 0x + 2y + 4z \\
z' = x + 0y - z
\end{cases}
$$
$$
\begin{align}
\lambda_{1, 2} = 0 \\
\lambda_{3} = 3
\end{align}
$$
## Решение

# №811~
# №812~

# Итого
```math
812 - 796 + 1
812 - 810 + 1
```

