847-850
# 847
$$
\begin{cases}
x' = -x + 2y \\
y' = -3x + 4y + e^{3t}
\end{cases}
$$
$$
\begin{pmatrix}
-1 - \lambda & 2 \\
-3 & 4 - \lambda
\end{pmatrix} = 0
$$
$$
\lambda_{1} = 1, \lambda_{2} = 2
$$
## $\lambda_{1} = 1$
$$
\begin{cases}
-2\alpha + 2\beta = 0 & \alpha = \beta \\
-3\alpha + 3\beta = 0 & \beta = \beta = 1
\end{cases} \quad V_{1} = \begin{pmatrix}
1 \\
1
\end{pmatrix}
$$
## $\lambda_{2} = 2$
$$
\begin{cases}
-3\alpha + 2\beta = 0 & \alpha = \dfrac{2}{3}\beta \\
-3 \alpha + 2\beta = 0 & \beta = \beta = 3
\end{cases} \quad V_{2} = \begin{pmatrix} 
2 \\
3
\end{pmatrix} 
$$

$$
\begin{cases}
x = C_{1}e^{t} + 2C_{2}e^{2t} \\
y = C_{1}e^{t} + 3C_{2}e^{2t}
\end{cases}
$$
$$
\begin{cases}
x' = C'_{1}(t)e^{t} + C_{1}(t)e^{t} + 2C'_{2}(t)e^{2t} + 4C_{2}(t)e^{2t} \\
y' = C'_{1}(t)e^{t} + C_{1}(t)e^{t} + 6C'_{2}(t)e^{2t} + 6C_{2}(t)e^{2t}
\end{cases}
$$
$$
\begin{cases}
C_{1}'(t)e^{t} + 2C_{2}'(t) e^{2t} = 0 \\
C_{1}'(t) e^{t} + 3C_{2}'(t)e^{2t} = \dfrac{e^{3t}}{e^{2t} + 1}
\end{cases}
$$
$$
\begin{cases}
C_{1}'(t) = -2C_{2}'(t)e^{t} \\
-2C_{2}'(t)e^{2t} + 3C_{2}'(t)e^{2t} = \dfrac{e^{3t}}{e^{2t} + 1}
\end{cases}
$$
$$
\begin{cases}
C_{2}'(t) = \dfrac{e^{t}}{e^{2t} + 1} \\
C_{2}(t) = \arctan(e^{t}) + D_{2}
\end{cases}
$$
$$
\begin{cases}
C_{1}'(t) = -\dfrac{e^{2t}}{e^{2t} + 1} \\
C_{1}(t) = -\ln \left| e^{2t} + 1 \right| + D_{1}
\end{cases}
$$
$$
\begin{pmatrix}
x \\
y
\end{pmatrix} = \begin{pmatrix}
-\ln \left| e^{2t} + 1 \right| + D_{1} \\
-\ln \left| e^{2t} + 1 \right| + D_{1}
\end{pmatrix}e^{t} + \begin{pmatrix}
2\left[ \arctan(e^{t}) + D_{2} \right] \\
3 \left[ \arctan(e^{t}) + D_{2} \right] 
\end{pmatrix}e^{2t}
$$
## 848
$$\begin{cases}
{x'=-4x-2y+\dfrac{2}{e^t - 1}}\\
{y'=6x+3y-\dfrac{3}{e^t - 1}}
\end{cases}$$
$$\begin{vmatrix}
{-4-\lambda} && {-2} \\
{6} && {3-\lambda}
\end{vmatrix} = 0$$
$\lambda_{1} = 0, \lambda_{2} = -1$
## $\lambda_{1} = 0$
$$
\begin{cases}
-4\alpha - 2\beta = 0 & \alpha = -\frac{1}{2}\beta \\
6\alpha + 3\beta = 0 & \beta = \beta = 1
\end{cases} \quad V_{1} = \begin{pmatrix}
-1 \\
2
\end{pmatrix} 
$$
## $\lambda_{2} = -1$
$$
\begin{cases}
-3\alpha - 2\beta = 0 & \alpha = -\frac{2}{3}\beta \\
6\alpha + 4\beta = 0 & \beta = \beta = 3
\end{cases} \quad V_{2}=\begin{pmatrix}
-2 \\
3
\end{pmatrix} 
$$

$$\begin{cases}
{x=-C_1+2C_2 e^{-t}}\\
{y=2C_1+3C_2 e^{-t}}
\end{cases}$$
$$\begin{cases}
{-C_1' +2 C_2' e^{-t}= \dfrac{2}{e^t - 1}}\\
{-2C_1' +3 C_2' e^{-t}=-\dfrac{3}{e^t - 1}}
\end{cases}$$
$$\begin{cases}
{C_1'= \dfrac{12}{e^t - 1}}\\
{C_2' =7\dfrac{e^{t}}{e^t - 1}}
\end{cases}$$
$$\begin{cases}
{C_1= 12\ln(e^t - 1)-12t + D_1}\\
{C_2=7\ln(e^t - 1) + D_2}
\end{cases}$$
$$
\begin{pmatrix}
x \\
y
\end{pmatrix} = \begin{pmatrix}
D_{1} \\
-2D_{1}
\end{pmatrix}e^{0t} + \begin{pmatrix}
2\left( D_{2} + \ln \left| e^{t} - 1 \right| \right) \\
-3\left( D_{2} + \ln \left| e^{t} - 1 \right| \right)  
\end{pmatrix}e^{-t}
$$

# 849

$$\begin{cases}
{x'=x-y+\dfrac{1}{\cos t}}\\
{y'=2x-y}
\end{cases}$$
$$\begin{vmatrix}
{1-\lambda} && {-1} \\
{2} && {-1-\lambda}
\end{vmatrix} = 0$$
$$\lambda_{1,2}=\pm i$$
## $\lambda = i$
$$
\begin{cases}
{(1-i)\alpha-\beta=0} & \alpha = \alpha = 1 \\
{2\alpha-(1+i)\beta=0} & \beta = \alpha - i
\end{cases} \quad  
\begin{pmatrix}
{1} \\
{1-i}
\end{pmatrix}
$$

$$
\begin{pmatrix}
{1} \\
{1-i}
\end{pmatrix} e^{it} = 
\begin{pmatrix}
{\cos t + i\sin t} \\
{\cos t - \sin t + (\sin t-\cos t)i}
\end{pmatrix} 
$$
$$\begin{cases}
{x=C_1\cos t+C_2 \sin t}\\
{y=C_1(\cos t -\sin t)+C_2 (\sin t - \cos t)}
\end{cases}$$
$$\begin{cases}
{C_1'\cos t+C_2' \sin t=\dfrac 1 {\cos t}}\\
{C_1'(\cos t -\sin t)+C_2' (\sin t - \cos t)=0}
\end{cases}$$
$$\begin{cases}
{C_1'\cos t+C_2' \sin t=\dfrac 1 {\cos t}}\\
{C_1'\sin t+C_2' \cos t=0}
\end{cases}$$
$$\begin{cases}
{C_1'=\dfrac 1 {\cos 2t}}\\
{C_2' =-\dfrac {\tan x} {\cos 2t}}
\end{cases}$$