# 766
$$y''+y'=f(x)$$
$$y(0)=0$$
$$y'(1)=0$$
$$y=C_0e^{-x}+C_1$$
$$\begin{cases}
C_0+C_1=0  \\
-\dfrac{C_0}{e}=0
\end{cases}$$
$$y_1=e^{-x}+1$$
$$y_2=1$$
$$G(x, s)=\begin{cases}
{a(s)(e^{-x}+1) \quad 0 \le x\le s} \\
{b(s) \quad s \le x \le 1}
\end{cases}$$
$$\begin{cases}
{a(s)(e^{-x}+1)=b(s)} \\
{a(s)e^{-x}=1}
\end{cases}$$
$$\begin{cases}
{b(s)=1+e^x} \\
{a(s)=e^x}
\end{cases}$$
$$G(x, s)=\begin{cases}
{e^s(e^{-x}+1) \quad 0 \le x\le s} \\
{(e{-s}+1) \quad s \le x \le 1}
\end{cases}$$
# 767
$$y''-y=f(x)$$
$$y'(0)=0$$
$$y'(2)+y(2)=0$$
$$y=C_0e^{-x}+C_1e^{x}$$
$$\begin{cases}
C_0=C_1  \\
-C_0e^{-2}+C_1e^{2}+C_0e^{-2}+C_1e^{2}=0
\end{cases}$$
$$\begin{cases}
C_0=C_1  \\
2C_1e^{2}=0
\end{cases}$$
$$y_1=e^{-x}+e^x$$
$$y_2=e^{-x}$$
$$G(x, s)=\begin{cases}
{a(s)(e^{-x}+e^{x}) \quad 0 \le x\le s} \\
{b(s)e^{-x} \quad s \le x \le 2}
\end{cases}$$
$$\begin{cases}
{a(s)(e^{-x}+e^{x})=b(s)e^{-x}} \\
{-b(s)e^{-x}=a(s)(-e^{-x}+e^{x})+1}
\end{cases}$$
$$\begin{cases}
{a(s)=-e^{-x}} \\
{b(s)=(e^{-x}+e^{x})}
\end{cases}$$
$$G(x, s)=\begin{cases}
{e^{-s}(e^{-x}+e^x) \quad 0 \le x\le s} \\
{(e^{-s}+e^s)e^{-x} \quad s \le x \le 2}
\end{cases}$$
# 769

$$x^2y''+2xy'=f(x)$$
$$y(1)=0$$
$$y'(3)=0$$
$$y=\dfrac{C_0}{x}+C_1$$
$$\begin{cases}
C_0=-C_1  \\
-\dfrac{C_0}{x^2}=0
\end{cases}$$
$$\begin{cases}
C_0=-C_1  \\
C_0=0
\end{cases}$$
$$y_1=\dfrac 1 x-1$$
$$y_2=1$$
$$G(x, s)=\begin{cases}
{a(s)(\dfrac 1 x - 1) \quad 1 \le x\le s} \\
{b(s) \quad s \le x \le 3}
\end{cases}$$
$$\begin{cases}
{a(s)(\dfrac{1}{s} - 1)=b(s)} \\
{0=-a(s)\dfrac{1}{s^2}+\dfrac{1}{s^2}}
\end{cases}$$
$$\begin{cases}
{b(s)=\dfrac{1}{s} - 1} \\
{a(s)=1}
\end{cases}$$
$$G(x, s)=\begin{cases}
{\dfrac 1 x - 1 \quad 1 \le x\le s} \\
{\dfrac 1 s - 1 \quad s \le x \le 3}
\end{cases}$$
# 770

$$xy''-y'=f(x)$$
$$y'(1)=0$$
$$y(2)=0$$
$$y=C_0x^2+C_1$$
$$\begin{cases}
2C_0 = 0 \\
4C_0+C_1=0
\end{cases}$$
$$y_1=1$$
$$y_2=4x^2-1$$
$$G(x, s)=\begin{cases}
{a(s) \quad 1 \le x\le s} \\
{b(s)(4x^2-1) \quad s \le x \le 2}
\end{cases}$$
$$\begin{cases}
{a(s)=b(s)(4s^2-1)} \\
{8b(s)s=\dfrac 1 s}
\end{cases}$$
$$\begin{cases}
{b(s)=\dfrac 1 {8s^2}} \\
{a(s)=\dfrac 1 2(1-\dfrac 1 {4s^2})}
\end{cases}$$
$$G(x, s)=\begin{cases}
{\dfrac 1 2 (1-\dfrac{1}{4s^2}) \quad 1 \le x\le s} \\
{\dfrac{1}{8s^2} (4x^2-1) \quad s \le x \le 2}
\end{cases}$$
# 771
$$x^2y''-2y=f(x)$$
$$y(1)=0$$
$$y(2)+2y'(2)=0$$
$$y=C_0x^2+\dfrac{C_1} x$$
$$\begin{cases}
C_0+C_1=0 \\
4C_0+\dfrac 1 2 C_1+8C_0-\dfrac 1 2 C_1=0
\end{cases}$$
$$\begin{cases}
C_0=-C_1 \\
C_0=0
\end{cases}$$
$$y_1=x^2-\dfrac 1 x$$
$$y_2=\dfrac 1 x$$
$$G(x, s)=\begin{cases}
{a(s) (x^2-\dfrac 1 x) \quad 1 \le x\le s} \\
{b(s)\dfrac 1 x \quad s \le x \le 2}
\end{cases}$$
$$\begin{cases}
{a(s)(s^2-\dfrac 1 s)=b(s)\dfrac 1 s} \\
{-b(s)\dfrac 1 {s^2}=a(s)(2s+\dfrac1 {s^2})+\dfrac 1 {s^2}}
\end{cases}$$
$$\begin{cases}
{b(s)=-\dfrac 1 {3s^3}(s^3-1)} \\
{a(s)=-\dfrac 1 {3s^3}}
\end{cases}$$
$$G(x, s)=\begin{cases}
{-\dfrac 1 {3s^3}(x^2-\dfrac 1 x) \quad 1 \le x\le s} \\
{-\dfrac 1 {3s^3}(s^3-1)\dfrac 1 x \quad s \le x \le 2}
\end{cases}$$
# 772
$$y''=f(x)$$
$$y(0)=0$$
$$y(+\infty)- ограничено$$
$$y=C_0x+C_1$$
$$\begin{cases}
C_1=0 \\
C_0=0
\end{cases}$$
$$y_1=x$$
$$y_2=1$$
$$G(x, s)=\begin{cases}
{a(s) x \quad 0 \le x\le s} \\
{b(s) \quad s \le x \le +\infty}
\end{cases}$$
$$\begin{cases}
{a(s)s=b(s)} \\
{a(s)=-1}
\end{cases}$$
$$\begin{cases}
{b(s)=-s} \\
{a(s)=-1}
\end{cases}$$
$$G(x, s)=\begin{cases}
{-x \quad 0 \le x\le s} \\
{-s \quad s \le x \le +\infty}
\end{cases}$$