834-840
# №834
## Условие
$$
\begin{cases}
x' = x + 2y \\
y' = x - 5\sin(t)
\end{cases}
$$
## Решение
### Общее Однородное
$$
\begin{vmatrix}
-\lambda + 1 & 2 \\
1 & -\lambda
\end{vmatrix} = \lambda^{2} - \lambda - 2 = 0
$$
$$
\begin{matrix}
\lambda_{1} = -1 \\
\lambda_{2} = 2
\end{matrix}
$$
#### $\lambda_{1} = -1$
$$
\begin{cases}
2\alpha + 2\beta = 0 & \alpha = -\beta \\
\alpha + \beta = 0 & \beta = \beta = 1
\end{cases} \quad V_{1} = \begin{pmatrix}
-1 \\
1
\end{pmatrix} 
$$
#### $\lambda_{2} = 2$
$$
\begin{cases}
-\alpha + 2\beta = 0 & \alpha = 2\beta \\
\alpha - 2\beta = 0 & \beta = \beta = 1
\end{cases} \quad V_{2} = \begin{pmatrix}
2 \\
1
\end{pmatrix} 
$$

### Частное Неоднородное
$$
P =  \begin{pmatrix}
A_{1}\sin(t) + B_{1}\cos(t) \\
A_{2}\sin(t) + B_{2}\cos(t)
\end{pmatrix}
$$

$$
P' = \begin{pmatrix}
A_{1} \cos(t) - B_{1}\sin(t) \\
A_{2} \cos(t) - B_{2} \sin(t)
\end{pmatrix}
$$
$$
\begin{cases}
A_{1} \cos(t) - B_{1}\sin(t) = A_{1}\sin(t) + B_{1}\cos(t) + 2A_{2}\sin(t) + 2B_{2}\cos(t) \\
A_{2} \cos(t) - B_{2} \sin(t) = A_{1}\sin(t) + B_{1}\cos(t) - 5\sin(t)
\end{cases}
$$
$$
\begin{cases}
\cos(t): & A_{1} = B_{1} + 2B_{2} \\
\sin(t):  &  -B_{1} = A_{1} + 2A_{2} \\
 \\
\cos(t): & A_{2} = B_{1} \\
\sin(t): & -B_{2} = A_{1} - 5
\end{cases}
$$
$$
\begin{cases}
A_{1} = -3B_{1} \\
B_{1} = B_{1} \\
A_{2} = B_{1} \\
B_{2} = 3B_{1} + 5
\end{cases}
$$
$$
P = \begin{pmatrix}
-3 \sin(t) + \cos(t) \\
\sin(t) + 8\cos(t)
\end{pmatrix}
$$
## Ответ
$$
\begin{pmatrix}
x \\
y
\end{pmatrix} = C_{1} \begin{pmatrix}
-1 \\
1
\end{pmatrix}e^{-t} + C_{2}\begin{pmatrix}
2 \\
1
\end{pmatrix}e^{2t} + \begin{pmatrix}
-3\sin(t) + \cos(t) \\
\sin(t) + 8\cos(t)
\end{pmatrix}
$$

# №835
## Условие
$$
\begin{cases}
x' = 2x - 4y \\
y' = x - 3y + 3e^{t}
\end{cases}
$$
## Решение
$$
(2 - \lambda) \cdot (-3 - \lambda) - \left( -4 \cdot 1 \right) = 0
$$
$$
\begin{matrix}
\lambda_{1} = 1 \\
\lambda_{2} = -2
\end{matrix}
$$
### Общее однородное
#### $\lambda_{1} = 1$
$$
\begin{cases}
\alpha - 4\beta = 0 & \alpha = 4\beta \\
\alpha - 4\beta = 0 & \beta = \beta = 1
\end{cases}  \quad V_{1} = \begin{pmatrix}
4 \\
1
\end{pmatrix} 
$$
#### $\lambda_{2} = -2$
$$
\begin{cases}
4\alpha - 4\beta = 0 & \alpha = \beta \\
\alpha - \beta = 0 & \beta = \beta = 1
\end{cases} \quad V_{2} = \begin{pmatrix}
1 \\
1
\end{pmatrix} 
$$

### Частное неоднородное
$$
P = \begin{pmatrix}
A_{1}t + B_{1} \\
A_{2}t + B_{2}
\end{pmatrix}e^{t}
$$
$$
P' = \begin{pmatrix}
\left( A_{1}t + B_{1} \right)e^{t} + A_{1}e^{t} \\
\left( A_{2}t + B_{2} \right) e^{t} + A_{2}e^{t} 
\end{pmatrix}
$$
$$
\begin{cases}
A_{1}t + B_{1} + A_{1} = 2A_{1}t + 2B_{1} - 4 A_{2}t - 4B_{2} \\
A_{2}t + B_{2} + A_{2} = A_{1}t + B_{1} - 3A_{2}t - 3B_{2} + 3
\end{cases}
$$
$$
\begin{cases}
t^{1}: & A_{1} = 2A_{1} - 4A_{2} & A_{2} = A_{1} - 3A_{2} \\
t^{0}: & B_{1} + A_{1} = 2B_{1} - 4B_{2} & B_{2} + A_{2} = B_{1} - 3B_{2} + 3
\end{cases}
$$
$$
\begin{cases}
A_{1} = B_{1} - 4B_{2} \\
A_{1} = 4A_{2} \\
A_{1} = A_{2} + 3A_{2} \\
A_{2} = B_{1} - 4B_{2} + 3 \\
 \\
3A_{2} = 3A_{2} \\
A_{1} = 4A_{2} \\
B_{1} = 4A_{2} - \frac{1}{2}\left( 3A_{2} + 3 \right) \\
B_{2} = \frac{3}{8}\left( A_{2} + 1 \right)  
\end{cases} \quad \begin{pmatrix}
A_{1} = 4 \\
A_{2} = 1 \\
B_{1} = 1 \\
B_{2} = \frac{3}{4}
\end{pmatrix} 
$$
$$
P = \begin{pmatrix}
4t + 1 \\
t + \frac{3}{4}
\end{pmatrix}
$$
## Ответ
$$
\begin{pmatrix}
x \\
y
\end{pmatrix} = C_{1}\begin{pmatrix}
4 \\
1
\end{pmatrix}e^{t} + C_{2}\begin{pmatrix}
1 \\
1
\end{pmatrix}e^{-2t} + \begin{pmatrix}
4t + 1 \\
t + \frac{3}{4}
\end{pmatrix}
$$

# №836
## Условие
$$
\begin{cases}
x' = 2x - y \\
y' = y - 2x + 18t
\end{cases}
$$
## Решение
$$
(2 - \lambda)(1 - \lambda) - \left( -2 \cdot -1 \right)  = 2\left( 1 - 2\lambda + \lambda^{2} \right) - 2 = 0
$$
$$
\begin{matrix}
\lambda_{1} = 0 \\
\lambda_{2} = 3
\end{matrix}
$$
### Общее однородное
#### $\lambda_{1} = 0$
$$
\begin{cases}
2\alpha - \beta = 0 & \alpha = \alpha = 1 \\
-2\alpha + \beta = 0 & \beta = 2\alpha
\end{cases} \quad V_{1} = \begin{pmatrix}
1 \\
2
\end{pmatrix} 
$$
#### $\lambda_{2} = 3$
$$
\begin{cases}
-\alpha - \beta = 0 & \alpha = \beta \\
-2\alpha - 2\beta = 0 & \beta = \beta = 1
\end{cases} \quad V_{2} = \begin{pmatrix}
1 \\
1
\end{pmatrix} 
$$
### Частное неоднородное
$$
P = \begin{pmatrix}
A_{1}t^{2} + B_{1}t + K_{1} \\
A_{2}t^{2} + B_{2}t + K_{2}
\end{pmatrix}
$$
$$
P' = \begin{pmatrix}
A_{1}t + B_{1} \\
A_{2}t + B_{2}
\end{pmatrix}
$$
$$
\begin{cases}
A_{1}t + B_{1} = 2A_{1}t^{2} + 2B_{1}t + 2K_{1} - A_{2}t^{2} - B_{2}t - K_{2} \\
A_{2}t + B_{2} = A_{2}t^{2} + B_{2}t + K_{2} - 2A_{1}t^{2} - 2B_{1}t - K_{1} + 18t
\end{cases}
$$
$$
\begin{cases}
t^{2}: & 0 = 2A_{1} - A_{2} & 0 = A_{2} - 2A_{1} \\
t^{1}: & A_{1} = 2B_{1} - B_{2} & A_{2} = B_{2} - 2B_{1} + 18 \\
t^{0}: & B_{1} = 2K_{1} - K_{2} & B_{2} = K_{2} - K_{1}
\end{cases}
$$
$$
\begin{cases}
A_{2} = 2A_{1} \\
A_{1} = 2B_{1} - B_{2} \\
A_{1} = 4K_{1} - 2K_{2} - K_{2} + K_{1} & A_{1} = 5K_{1} - 3K_{2} \\
A_{2} = K_{2} - K_{1} -4K_{1} + 2K_{2} + 18 & A_{2} = -5K_{1} + 3K_{2} + 18 \\
-5K_{1} + 3K_{2} + 18 = 10K_{1} - 6K_{2} \\
9K_{2} = 15K_{1} - 18 & K_{2} = \dfrac{5K_{1}}{3} - 2 \\
B_{1} = 2K_{1} - K_{2} \\
B_{2} = K_{2} - K_{1}
\end{cases} \quad \begin{pmatrix}
K_{1} = 3 \\
K_{2} = 3 \\
B_{2} = 0 \\
B_{1} = 3 \\
A_{1} = 6 \\
A_{2} = 12
\end{pmatrix} 
$$
$$
P = \begin{pmatrix}
6t^{2} + 3t + 3 \\
12t^{2} + 0t + 3
\end{pmatrix}
$$
## Ответ
$$
\begin{pmatrix}
x \\
y
\end{pmatrix} = C_{1} \begin{pmatrix}
1 \\
2
\end{pmatrix} + C_{2} \begin{pmatrix}
1 \\
1
\end{pmatrix} + \begin{pmatrix}
6t^{2} + 3t + 3 \\
12t^{2} + 0t + 3
\end{pmatrix}
$$
# №837
## Условие
$$
\begin{cases}
x' = x + 2y + 16te^{t} \\
y' = 2x - 2y
\end{cases}
$$
## Решение
### Общее однородное
$$
\left( 1 - \lambda \right)\left( -2 - \lambda \right) - \left( 2 \cdot 2 \right) = -2 + 2\lambda - \lambda + \lambda^{2} - 4 = \lambda^{2} + \lambda - 6 = 0
$$
$$
\begin{matrix}
\lambda_{1} = 2 \\
\lambda_{2} = -3
\end{matrix}
$$
#### $\lambda_{1} = 2$
$$
\begin{cases}
-\alpha + 2\beta = 0 & \alpha = 2\beta \\
2\alpha - 4 \beta = 0 & \beta = \beta = 1
\end{cases} \quad V_{1}=\begin{pmatrix}
2 \\
1
\end{pmatrix} 
$$
#### $\lambda_{2} = -3$
$$
\begin{cases}
4 \alpha + 2\beta = 0 & \alpha = -\frac{1}{2}\beta \\
2 \alpha + \beta = 0 & \beta = \beta = 2
\end{cases} \quad V_{2} = \begin{pmatrix}
-1 \\
2
\end{pmatrix} 
$$

### Частное неоднородное
$$
P = \begin{pmatrix}
A_{1}t + B_{1} \\
A_{2}t + B_{2}
\end{pmatrix}e^{t}
$$
$$
P' = \begin{pmatrix}
A_{1}t + B_{1} + A_{1} \\
A_{2}t + B_{2} + A_{2}
\end{pmatrix}e^{t}
$$
$$
\begin{cases}
A_{1}t + B_{1} + A_{1} = A_{1}t + B_{1} + 2A_{2}t + 2B_{2} + 16t \\
A_{2}t + B_{2} + A_{2} = 2A_{1}t + 2B_{1} - 2A_{2}t -2B_{2}
\end{cases}
$$
$$
\begin{cases}
t^{1}: & A_{1} = A_{1} + 2A_{2} + 16 & A_{2} = 2A_{1} - 2A_{2} \\
t^{0}: & B_{1} + A_{1} = B_{1} + 2B_{2} & B_{2} + A_{2} = 2B_{1} - 2B_{2}
\end{cases}
$$
$$
\begin{cases}
A_{2} = -8 \\
A_{1} = -12 \\
B_{2} = -6 \\
B_{1} = -26
\end{cases}
$$
$$
P = \begin{pmatrix}
-12t - 26 \\
-8t - 6
\end{pmatrix}
$$
## Ответ
$$
\begin{pmatrix}
2 \\
1
\end{pmatrix} = C_{1} \begin{pmatrix}
2 \\
1
\end{pmatrix} e^{2t} + C_{2} \begin{pmatrix}
-1 \\
2
\end{pmatrix} e^{-3} + \begin{pmatrix}
-12t - 26 \\
-8 - 6
\end{pmatrix}
$$

# №838~
## Условие
$$
\begin{pmatrix}

\end{pmatrix}
$$
## Решение

## Ответ

# №839~
## Условие

## Решение

## Ответ

# №840~
## Условие

## Решение

## Ответ

