# 751

$$
\begin{cases}
y'' - y = 2x \\
y(0) = 0 \\
y(1) = -1
\end{cases}
$$
$$
\lambda = \pm1
$$
$$
y = C_{1}e^{-x} + C_{2}e^{x}
$$
$$
\begin{cases}
C_1=-C_2 \\
C_1e^{-1}+C_2e=-1
\end{cases} \implies \begin{cases}
C_2=\dfrac 1 {e^{-1}-e} \\
C_{1} = -\dfrac 1 {e^{-1}-e}
\end{cases}
$$
$$
y = -\dfrac 1 {e^{-1}-e} e^{-1} + \dfrac 1 {e^{-1}-e} e^x
$$
# 752
$$
\begin{cases}
y'' + y' = 1 \\
y'(0) = 0 \\
y(1) = 1
\end{cases}
$$
$$
\lambda^{2} + \lambda = 0
$$
$$
\begin{matrix}
\lambda = -1 \\
\lambda = 0
\end{matrix}
$$
$$
y = C_{1}e^{-x} + C_2+x
$$
$$
\begin{cases}
1-C_1=0 \\
C_1e^{-1}+C_2=0
\end{cases} \implies \begin{cases}
C_1=1 \\
C_2=-e^{-1}
\end{cases}
$$
$$
y = e^{-x}-e^{-1}+x
$$