869 - 873 без 871, 872

# №868
## Условие
$$
\begin{pmatrix}
0 & 1 \\
-1 & 0
\end{pmatrix}
$$
## Решение
### Нахождение общего решения
$$
-\lambda \cdot (-\lambda) + 1 = 0
$$
$$
\lambda = \pm i
$$
$$
\begin{cases}
\alpha i + \beta = 0 & \beta = \alpha \\
-\alpha - \beta i = 0 & \alpha = \alpha = 1
\end{cases} \quad V_{1} = \begin{pmatrix}
1 \\
i
\end{pmatrix} e^{it} = \begin{pmatrix}
\cos(t) + i\sin(t) \\
i\cos(t) - \sin(t)
\end{pmatrix}
$$
$$
X = C_{1}\begin{pmatrix}
\cos(t) \\
-\sin(t)
\end{pmatrix} + C_{2}\begin{pmatrix}
\sin(t) \\
\cos(t)
\end{pmatrix}
$$
### Подстановка
$$
X_{1} = \begin{pmatrix}
\cos(t) \\
-\sin(t)
\end{pmatrix}
$$
$$
C_{1}\begin{pmatrix}
1 \\
0
\end{pmatrix} + C_{2}\begin{pmatrix}
0 \\
1
\end{pmatrix} = \begin{pmatrix}
1 \\
0
\end{pmatrix}
$$
$$
\begin{pmatrix}
C_{1} \\
C_{2}
\end{pmatrix} = \begin{pmatrix}
1 \\
0
\end{pmatrix}
$$

$$
X_{2} = \begin{pmatrix}
\sin(t) \\
\cos(t)
\end{pmatrix}
$$
$$
C_{1}\begin{pmatrix}
1 \\
0
\end{pmatrix} + C_{2}\begin{pmatrix}
0 \\
1
\end{pmatrix} = \begin{pmatrix}
1 \\
0
\end{pmatrix}
$$
$$
\begin{pmatrix}
C_{1} \\
C_{2}
\end{pmatrix} = \begin{pmatrix}
0 \\
1
\end{pmatrix}
$$
$$
e^{At} = \begin{pmatrix}
\cos(t) & \sin(t) \\
-\sin(t) & \cos(t)
\end{pmatrix}
$$
$$
e^{A} = \begin{pmatrix}
\cos(1) & \sin(1) \\
-\sin(1) & \cos(1)
\end{pmatrix}
$$
## Ответ
$$
e^{A} = \begin{pmatrix}
\cos(1) & \sin(1) \\
-\sin(1) & \cos(1)
\end{pmatrix}
$$
# №869
## Условие
$$
A = \begin{pmatrix}
2 & 1 \\
0 & 2
\end{pmatrix}
$$
## Решение
$$
\lambda_{1, 2} = 2
$$
$$
X = \begin{pmatrix}
A_{1}t + B_{1} \\
A_{2}t + B_{2}
\end{pmatrix}e^{2t}
$$
$$
\ldots
$$
$$
X = \begin{pmatrix}
C_{1}t + C_{2} \\
C_{1}
\end{pmatrix}e^{2t}
$$
$$
\begin{pmatrix}
C_{1} \\
C_{0}
\end{pmatrix} = \begin{pmatrix}
1 \\
0
\end{pmatrix} \implies \begin{pmatrix}
e^{2t} \\
0
\end{pmatrix}
$$
$$
\begin{pmatrix}
C_{1} \\
C_{0}
\end{pmatrix} = \begin{pmatrix}
0 \\
1
\end{pmatrix} \implies \begin{pmatrix}
te^{2t} \\
e^{2t}
\end{pmatrix}
$$
## Ответ
$$
e^{tA} = \begin{pmatrix}
e^{2t} & te^{2t} \\
0 & e^{2t}
\end{pmatrix} \quad e^{A} = \begin{pmatrix}
e^{2} & e^{2} \\
0 & e^{2}
\end{pmatrix} 
$$
# №870
## Условие
$$
A = \begin{pmatrix}
3 & -1 \\
2 & 0
\end{pmatrix}
$$
## Решение
$$
\lambda^{2} - 3\lambda + 2 = 0
$$
$$
\begin{matrix}
\lambda_{1} = 1 \\
\lambda_{2} = 2
\end{matrix}
$$
$$
\begin{cases}
2\alpha - \beta = 0 & \alpha = \frac{\beta}{2} \\
2 \alpha - \beta = 0 & \beta = \beta = 2
\end{cases} \quad V_{1} = \begin{pmatrix}
1 \\
2
\end{pmatrix} 
$$
$$
\begin{cases}
\alpha - \beta = 0 & \alpha = \beta \\
2\alpha - 2\beta = 0 & \beta = \beta = 1
\end{cases} \quad V_{2} = \begin{pmatrix}
1 \\
1
\end{pmatrix} 
$$
$$
X = C_{1}\begin{pmatrix}
1 \\
2
\end{pmatrix}e^{t} + C_{2}\begin{pmatrix}
1 \\
1
\end{pmatrix}e^{2t}
$$

$$
C_{1}\begin{pmatrix}
1 \\
2
\end{pmatrix} + C_{2}\begin{pmatrix}
1 \\
1
\end{pmatrix} = \begin{pmatrix}
1 \\
0
\end{pmatrix}
$$
$$
\begin{pmatrix}
C_{1} \\
C_{2}
\end{pmatrix} = \begin{pmatrix}
-1 \\
2
\end{pmatrix} \implies \begin{pmatrix}
-e^{t} + 2e^{2t} \\
-2e^{t} + 2e^{2t}
\end{pmatrix}
$$

$$
C_{1}\begin{pmatrix}
1 \\
2
\end{pmatrix} + C_{2} \begin{pmatrix}
1 \\
1
\end{pmatrix} = \begin{pmatrix}
0 \\
1
\end{pmatrix}
$$
$$
\begin{pmatrix}
C_{1} \\
C_{2}
\end{pmatrix} = \begin{pmatrix}
1 \\
-1
\end{pmatrix} \implies \begin{pmatrix}
e^{t} -e^{2t} \\
2e^{t} - e^{2t}
\end{pmatrix}
$$

$$
e^{At} = \begin{pmatrix}
-e^{t} + 2e^{2t} & e^{t} - e^{2t} \\
-2e^{t} + 2e^{2t} & 2e^{t} - e^{2t}
\end{pmatrix} \quad  e^{A} = \begin{pmatrix}
-e + 2e^{2} & e - e^{2} \\
-2e + 2e^{2} & 2e - e^{2}
\end{pmatrix}
$$
## Ответ
# №871-
## Условие
$$
A = \begin{pmatrix}
-2 & -4 \\
1 & 2
\end{pmatrix}
$$
## Решение
$$
\lambda^{2} = 0
$$
$$
\lambda_{1, 2} = 0
$$
$$
\begin{cases}
-2\alpha - 4\beta = 0 & \alpha = -2\beta \\
\alpha + 2\beta = 0 & \beta = \beta = 1
\end{cases} \quad  
$$
## Ответ
# №872-
## Условие
## Решение
## Ответ
# №873
## Условие
$$
A = \begin{pmatrix}
2 & 1 & 0 \\
0 & 2 & 1 \\
0 & 0 & 2
\end{pmatrix}
$$
## Решение
$$
(2 - \lambda)^{3} = 0
$$
$$
\lambda_{1, 2, 3} = 2
$$
$$
S = 3 - rank\left( A - 2E \right) = 1
$$
$$
P = \begin{pmatrix}
A_{1}t^{2} + B_{1}t + D_{1} \\
A_{2}t^{2} + B_{2}t + D_{2} \\
A_{3}t^{2} + B_{3}t + D_{3}
\end{pmatrix}e^{2t}
$$
$$
P' = \begin{pmatrix}
2A_{1}t^{2} + 2A_{1}t + 
\end{pmatrix}
$$
## Ответ