---
Редакторы: Artemii
Тэги:
  - II семестр
  - Практика
Дата: 2023-12-05
Статус: Готово
---
$\mathsf  
{  
a \le x \le b  
}$

$\mathsf  
{  
P = 2\pi \overset {b}{\underset{a} \int} f(x) \sqrt{1 + (f'(x))^2}~ dx  
}$

![[IMG_20230512_093303.jpg]]

  

![[IMG_20230512_093307_1.jpg]]

$\mathsf  
{  
y = \dfrac 1 3 x^3;\quad -1 \le x \le 1  
}$

$\mathsf  
{  
P = 4\pi \overset 1 {\underset 0 \int} \dfrac 1 3 x^3 \sqrt{1 + x^4}~ dx = \dfrac 1 3 \pi \overset 1 {\underset 0 \int} \sqrt{1 + x^4}~ d(1 +x^4) = \dfrac 2 9 \pi (1 + x^4) ^{\frac 3 2} \overset 1 {\underset 0 \mid} = \dfrac 2 9 \pi 2^{\frac 2 3} \pi - \dfrac 2 9 \pi = \dfrac 2 9 \pi(2\sqrt 2 - 1)  
}$

  

  

## Площадь поверхности циклоиды

  

$\mathsf  
{  
\begin{cases}  
\mathsf{x = x(t)} & \mathsf{\alpha \le t \le \beta} \\  
\mathsf{y = y(t)}  
\end{cases}  
}$

$\mathsf  
{  
P = 2\pi \overset \beta {\underset \alpha \int} y(t) \sqrt{(x'(t))^2 + (y'(t))^2}~dt  
}$

  

  

  

$\mathsf  
{  
p = 2\pi \overset {2\pi} {\underset 0 \int} 3(1 - \cos(t)) \sqrt{9(1 - \cos(t))^2 + 9\sin(t)}~ dt = 6\pi \overset {2\pi} {\underset 0 \int } (1 -\cos(t)) \sqrt{(1 - \cos(t))^2 + \sin^2(t)}~ dt =  
}$

$\mathsf  
{  
= 18\pi \overset {2\pi} {\underset 0 \int }(1 - \cos(t)) \sqrt{1 - 2\cos(t) + \cos^2(t) + \sin^2(t)}~ dt = 18\pi \overset {2\pi} {\underset 0 \int} (1 - \cos(t)) \sqrt{2 - 2\cos(t)}~ dt =  
}$

$\mathsf  
{  
= 18 \sqrt 2 \pi \overset {2\pi} {\underset 0 \int}(1 - \cos(t)) \sqrt{1 - \cos(t)}~ dt = 18 \sqrt 2 \pi \overset {2\pi} {\underset 0 \int}(1 - \cos(t)) \sqrt {2 \sin^2(\frac t 2)}~ dt = 36\pi \overset {2\pi} {\underset 0 \int }(1 - \cos(t)) \sin(\frac t 2)~ dt =  
}$

$\mathsf  
{  
=  
36\cdot 2 \pi \overset {2\pi} {\underset 0 \int} (2\cos^2(\frac t 2) + 1)~ d(\cos(\frac t 2)) =  
72 \pi  
}$

  

  

  

  

$\mathsf  
{  
(x - x_0)^2 + (y - y_0)^2 = R^2 \quad x_0 = 0 \quad y_0 = d + R  
}$

$\mathsf  
{  
x^2 + (y - (d + R))^2 = R^2  
}$

$\mathsf  
{  
y = \pm \sqrt{R^2 - x^2} + d + R  
}$

  

![[/Untitled 30.png|Untitled 30.png]]

$\mathsf  
{  
P = 2\pi \overset b {\underset a \int} y(x) \cdot \sqrt{1 + (y'(x))^2} dx  
}$

$\mathsf  
{  
P = 4\pi \overset R {\underset 0 \int} (\sqrt{R^2 - x^2} + d + R) \sqrt{1 + \dfrac{x^2}{R^2 - x^2}} dx = 4\pi \overset R {\underset 0 \int} (\sqrt{R^2 - x^2} + d + R) \sqrt{\dfrac{R^2}{R^2 - x^2}}dx =  
}$$\mathsf  
{  
= 4\pi \overset R {\underset 0 \int} Rdx + 4\pi \overset R {\underset 0 \int}(d + R) \dfrac R {\sqrt{R^2 - x^2}} dx = 4\pi R^2 + 4\pi(d + R) R \cdot \arcsin (\dfrac x R) \overset R {\underset 0 \mid} = 4\pi R^2 + 4\pi(d + R)R \cdot \dfrac \pi 2  
}$

$\mathsf  
{  
P = 4\pi^2(d + R) R  
}$

  

  

$\mathsf  
{  
P = 2\pi \overset \beta {\underset \alpha \int} \rho(\phi) \cdot \sin(\phi) \cdot \sqrt{(\rho'(\phi))^2 + (\rho(\phi))^2}d\phi  
}$

$\mathsf  
{  
\rho = a(1 + \cos(\phi)) \quad a = 2  
}$

  

![[/Untitled 1 10.png|Untitled 1 10.png]]

$\mathsf  
{  
P = 2x \overset \pi {\underset 0 \int} 2(1 + \cos(\phi)) \sin(\phi) \sqrt{(-2 \sin(\phi)^2 + (2 + 2\cos(\phi))^2} d\phi =  
}$$\mathsf  
{  
= 4 \pi \overset \pi {\underset 0 \int} (1 + \cos(\phi)) \sin(\phi) \cdot 2 \sqrt{\sin^2( \phi) + 1 + 2 \cos(\phi) + \cos^2(\phi)} d\phi =  
}$

$\mathsf  
{  
= 8\pi \overset \pi {\underset 0 \int} (1 + \cos(\phi)) \sin(\phi) \sqrt{2 + 2\cos(\phi)} d\phi =  
8 \sqrt 2 \pi \overset \pi {\underset 0 \int} (1 + \cos(\phi)) \sin(\phi) \sqrt{1 + \cos(\phi)} d\phi =  
}$$\mathsf  
{  
-8 \sqrt 2 \pi \overset \pi {\underset 0 \int} (1 + \cos(\phi) ^{\frac 3 2} d(1 + \cos(\phi)) = -8 \sqrt 2 \pi \dfrac{2 (1 + \cos(\phi))^{\dfrac 5 2}} 5 \overset \pi {\underset 0 \mid} = 8\sqrt 2 \pi \dfrac{2 \cdot 2 ^{\frac 5 2}}{5} = \dfrac {16 \cdot 8} 5 \pi = \dfrac{128 \pi} 5  
}$