---
Owner: Artemii
tags:
  - ДЗ
---
139-144

147-150

# №139

## Условия

$\mathsf{  
(xy + e^x) dx - xdy = 0  
}$

## Решение

$\mathsf{  
\dfrac{dy}{dx} = \dfrac{xy + e^x} x  
}$

$\mathsf{  
\dfrac{dy}{dx} - y = \dfrac{e^x}{x}  
}$

### Лагранж

**Общее однородное**

$\mathsf{  
\dfrac{dy}{dx} = y  
}$

$\mathsf{  
\dfrac{dy} y = dx  
}$

$\mathsf{  
\ln(y) = x + C  
}$

$\mathsf{  
y = e^{x}C  
}$

**Частное неоднородное**

$\mathsf{  
y = C(x) e^x  
}$

$\mathsf{  
y' = C'(x) e^x + C(x) e^x  
}$

$\mathsf{  
C'(x)e^x + C(x) e^x- C(x) e^x = \dfrac{e^x}{x}  
}$

$\mathsf{  
C'(x) = \dfrac 1 x  
}$

$\mathsf{  
C(x) = \ln(x) + \overline C  
}$

$\mathsf{  
y = e^x \left[\ln(x) + \overline C\right]  
}$

  

## Особые решения

1. $\mathsf{  
    x = 0  
    }$
    
    **ПОДХОДИТ**
    
    **ЯВЛЯЕТСЯ ОСОБЫМ РЕШЕНИЕМ**
    

# №140

## Условия

$\mathsf{  
x^2 y' + xy + 1 = 0  
}$

## Решение

  

$\mathsf{  
\dfrac{dy}{dx} + \dfrac{y}{x} = - \dfrac{1}{x^2}  
}$

**Лагранж**

$\mathsf{  
\dfrac{dy}{dx} = -\dfrac y x  
}$

$\mathsf{  
\ln(y) = -\ln(x) + C  
}$

$\mathsf{  
y = \dfrac C x  
}$

  

$\mathsf{  
y = \dfrac {C(x)} x  
}$

$\mathsf{  
y' = \dfrac{C'(x)}{x} - \dfrac{C(x)}{x^2}  
}$

  

$\mathsf{  
\dfrac{C'(x)}{x} - \dfrac{C(x)}{x^2} + \dfrac{C(x)}{x^2} = -\dfrac 1 {x^2}  
}$

$\mathsf{  
C'(x) x - C(x) + C(x) = -1  
}$

$\mathsf{  
C'(x) x = -1  
}$

$\mathsf{  
C(x) = -\ln(x) + \overline C  
}$

  

$\mathsf{  
y = \dfrac{- \ln(x) + \overline C}{x}  
}$

## Особые решения

1. $\mathsf{  
    x^2 = 0  
    }$
    
    **НЕ ПОДХОДИТ**
    
2. $\mathsf{  
    y = 0  
    }$
    
    **НЕ ПОДХОДИТ**
    

# №141

## Условия

$\mathsf{  
y = x(y' - x \cos(x))  
}$

## Решение

$\mathsf{  
y' = \dfrac{y}x + x \cos(x)  
}$

### Лагранж

**Общее однородное**

$\mathsf{  
\dfrac{dx} x = \dfrac{dy} y  
}$

$\mathsf{  
\ln(xC) = \ln(y)  
}$

$\mathsf{  
xC = y  
}$

  

$\mathsf{  
y = C(x) x  
}$

$\mathsf{  
y' = C'(x)x + C(x)  
}$

  

$\mathsf{  
xC'(x) + C(x) = C(x) + x \cos(x)  
}$

$\mathsf{  
C'(x) = \cos(x)  
}$

$\mathsf{  
C(x) = \sin(x) + \overline C  
}$

  

$\mathsf{  
y = x \sin(x) + x\overline C  
}$

  

## Особые решения

1. $\mathsf{  
    x = 0  
    }$
    
    **НЕ ПОДХОДИТ**
    

# №142

## Условия

$\mathsf{  
2x(x^2 + y)dx = dy  
}$

## Решение

$\mathsf{  
\dfrac{dy}{dx} = 2xy + 2x^3  
}$

### Лагранж

**Общее однородное**

$\mathsf{  
\dfrac{dy}{dx} = 2xy  
}$

$\mathsf{  
\dfrac{dy}{y} = 2xdx  
}$

$\mathsf{  
\ln(y) = x^2 + C  
}$

  

$\mathsf{  
y = C(x)e^{x^2}  
}$

$\mathsf{  
y' = C'(x) e^{x^2} + 2xC(x) e^{x^2}  
}$

  

$\mathsf{  
C'(x) e^{x^2} + 2x C(x) e^{x^2} = 2xC(x)e^{x^2} + 2x^3  
}$

$\mathsf{  
C'(x) = \dfrac{2x^3}{e^{x^2}}  
}$

$\mathsf{  
C(x) = -\dfrac{x^2 + 1}{e^{x^2}} + \overline C  
}$

  

$\mathsf{  
y = -x^2 - 1+ e^{x^2}\overline C  
}$

## Особые решения

1. $\mathsf{  
    e^{x^2} = 0  
    }$
    
    **НЕ ПОДХОДИТ**
    

# №143

## Условия

$\mathsf{  
(xy' - 1) \ln(x) = 2y  
}$

## Решение

$\mathsf{  
y' = \dfrac{2y}{\ln(x)x} + \dfrac{1} x  
}$

### Лагранж

$\mathsf{  
y' = \dfrac{2y}{\ln(x) x}  
}$

$\mathsf{  
\dfrac{dy}{2y} = \dfrac{dx}{\ln(x) \cdot x}  
}$

$\mathsf{  
\dfrac 1 2 \ln(y) = \ln(\ln(x)C)  
}$

$\mathsf{  
y = C\ln^2(x)  
}$

  

$\mathsf{  
y = C(x)\ln^2(x)  
}$

$\mathsf{  
y' = \dfrac{C'(x)x \ln^2(x) + 2C(x) \ln(x)}{x}  
}$

$\mathsf{  
\dfrac{xC'(x) \ln^2(x) + 2C(x) \ln(x)}{x} = \dfrac{2C(x)\ln^2(x)}{\ln(x)x} + \dfrac{1} x  
}$

$\mathsf{  
xC'(x) \ln^2(x) + 2C(x) \ln(x) = 2C(x) \ln(x) + 1  
}$

$\mathsf{  
xC'(x) \ln^2(x) = 1  
}$

$\mathsf{  
C'(x) = \dfrac 1 {x\ln^2(x)}  
}$

$\mathsf{  
C(x) = -\dfrac 1{\ln(x)} + \overline C  
}$

$\mathsf{  
y = \overline C \ln^2(x) - \ln(x)  
}$

  

## Особые решения

1. $\mathsf{  
    \ln(x) = 0  
    }$
    
    $\mathsf{  
    x = 1  
    }$
    
    **НЕ ПОДХОДИТ**
    
2. $\mathsf{  
    2y = 0  
    }$
    
    **НЕ ПОДХОДИТ**
    

# №144

## Условия

$\mathsf{  
xy' + (x + 1) y = 3x^2 e^{-x}  
}$

## Решение

$\mathsf{  
y' = \dfrac{3x^2 e^{-x} - y(x + 1)}{x}  
}$

$\mathsf{  
y' =-\dfrac{y(x + 1)} x + 3xe^{-x}  
}$

### Лагранж

$\mathsf{  
y' = -y - \dfrac y x  
}$

$\mathsf{  
\dfrac{dy}{y} = -(1 + \dfrac{1}{x})dx  
}$

  

$\mathsf{  
-\ln(y) = x + \ln(x) + C  
}$

$\mathsf{  
y = \dfrac C {xe^x}  
}$

  

$\mathsf{  
y = \dfrac{C(x)}{x e^x}  
}$

$\mathsf{  
y' = \dfrac{(C'(x) - C(x))x - C(x)}{x^2 e^x}  
}$

$\mathsf{  
\dfrac{(C'(x) - C(x))x - C(x)}{x^2 e^x} = - \dfrac{\dfrac{C(x)}{x e^x}(x + 1)}{x} + 3xe^{-x}  
}$

$\mathsf{  
(C'(x) - C(x)) x - C(x) = - C(x) (x + 1) + 3x^3  
}$

$\mathsf{  
C'(x) x - C(x)x - C(x) = -C(x)x - C(x) + 3x^3  
}$

$\mathsf{  
C'(x) = 3x^2  
}$

$\mathsf{  
C(x) = 6x + \overline C  
}$

  

$\mathsf{  
y = \dfrac{x^3 +\overline C}{xe^x}  
}$

## Особые решения

1. $\mathsf{  
    x = 0  
    }$
    
    **ПОДХОДИТ**
    
2. $\mathsf{  
    y = 0  
    }$

# №147

## Условия

$\mathsf{  
(\sin^2(y) + x \ctg(y))y' = 1  
}$

## Решение

$\mathsf{  
\sin^2(y) + x \ctg(y) = x'  
}$

## Лагранж

$\mathsf{  
x' = x \ctg(y)  
}$

$\mathsf{  
\dfrac{dx}{x} = \ctg(y) dy  
}$

$\mathsf{  
\ln(x) = \ln(\sin(y)) + C  
}$

$\mathsf{  
x = \sin(y)C  
}$

  

$\mathsf{  
x = C(y) \sin(y)  
}$

$\mathsf{  
x' = C'(y) \sin(y) + C(y) \cos(y)  
}$

  

$\mathsf{  
\sin^2(y) + C(y) \sin(y) \ctg(y) = C'(y) \sin(y) + C(y) \cos(y)  
}$

$\mathsf{  
C'(y) = \sin(y)  
}$

$\mathsf{  
C(y) = -\cos(y) + \overline C  
}$

$\mathsf{  
x = (\overline C - \cos(y)) \sin(y)  
}$

## Особые решения

1. $\mathsf{  
    x = 0  
    }$
    
    **НЕ ПОДХОДИТ**
    
2. $\mathsf{  
    \sin(y) = 0  
    }$
    
    **НЕ ПОДХОДИТ**
    

# №148

## Условия

$\mathsf{  
(2x + y)dy = ydx + 4 \ln(y) dy  
}$

## Решение

$\mathsf{  
(2x + y - 4 \ln(y))dy = ydx  
}$

$\mathsf{  
\dfrac{dx}{dy} = \dfrac{2x} y + \dfrac{y - 4 \ln(y)} y  
}$

### Лагранж

$\mathsf{  
\dfrac{dx}{dy} = \dfrac{2x} y  
}$

$\mathsf{  
\dfrac{dx}{x} = \dfrac{2dy} y  
}$

$\mathsf{  
\ln(x) = 2 \ln(yC)  
}$

$\mathsf{  
x = y^2C  
}$

$\mathsf{  
x = y^2C(y)  
}$

$\mathsf{  
x' = 2yC(y) + y^2C'(y)  
}$

  

$\mathsf{  
2yC(y) + y^2C'(y) = \dfrac{2y^2C(y)} y + \dfrac{y - 4 \ln(y)} y  
}$

$\mathsf{  
2y^2C(y) + y^3C'(y) = 2y^2C(y) + y - 4 \ln(y)  
}$

$\mathsf{  
C'(y) = \dfrac{y - 4 \ln(y)}{y^3}  
}$

$\mathsf{  
C(y) = \dfrac{2\ln(y) - y + 1}{y^2} + \overline C  
}$

$\mathsf{  
x = 2\ln(y) - y + 1 + y^2\overline C  
}$

## Особые решения

1. $\mathsf{  
    y = 0  
    }$
    
    **ПОДХОДИТ**
    
    **НЕ ЯВЛЯЕТСЯ ОСОБЫМ РЕШЕНИЕМ**
    
2. $\mathsf{x = 0}$
    
    **НЕ ПОДХОДИТ**
    

# №149

## Условия

$\mathsf{  
y' = \dfrac y {3x - y^2}  
}$

## Решение

$\mathsf{  
\dfrac{dx}{dy} = \dfrac{3x - y^2}{y}  
}$

### Лагранж

$\mathsf{  
\dfrac{dx}{dy} = \dfrac{3x}{y}  
}$

$\mathsf{  
\dfrac{dx}{3x} = \dfrac{dy} y  
}$

$\mathsf{  
\ln(x) = 3 \ln(yC)  
}$

$\mathsf{  
x = y^3C  
}$

$\mathsf{  
x = y^3 C(y)  
}$

$\mathsf{  
x' = 3y^2 C(y) + y^3 C'(y)  
}$

  

$\mathsf{  
3y^2 C(y) + y^3 C'(y) = \dfrac{3y^3C(y)}{y} - y  
}$

$\mathsf{  
C'(y) = - \dfrac 1 {y^2}  
}$

$\mathsf{  
C(y) = \dfrac 1 y + \overline C  
}$

$\mathsf{  
x = y^2 + y^3 \overline C  
}$

## Особые решения

1. $\mathsf{  
    y = 0  
    }$
    
    **ПОДХОДИТ**
    
    **ЯВЛЯЕТСЯ ОСОБЫМ РЕШЕНИЕМ**
    
2. $\mathsf{  
    3x = 0  
    }$
    
    **НЕ ПОДХОДИТ**
    

# №150

## Условия

$\mathsf{  
(1 - 2xy)y' = y(y - 1)  
}$

## Решение

$\mathsf{  
x' = \dfrac{1-2xy}{y(y - 1)}  
}$

$\mathsf{  
x' = - \dfrac{2x}{y - 1} + \dfrac{1}{y(y - 1)}  
}$

### Лагранж

$\mathsf{  
x' = - \dfrac{2x}{y - 1}  
}$

$\mathsf{  
\dfrac{dx}{2x} = -\dfrac{dy}{y - 1}  
}$

$\mathsf{  
\ln(x) = -2\ln(y - 1) + C  
}$

$\mathsf{  
x = \dfrac{C}{(y - 1)^2}  
}$

  

$\mathsf{  
x = \dfrac{C(y)}{(y - 1)^2}  
}$

$\mathsf{  
x' = \dfrac{C'(y)}{(y - 1)^2} - \dfrac{2C(y)}{(y - 1)^3}  
}$

$\mathsf{  
\dfrac{C'(y)}{(y - 1)^2} - \dfrac{2C(y)}{(y - 1)^3} = - \dfrac{2\dfrac{C(y)}{(y - 1)^2}}{y - 1} + \dfrac{1}{y(y - 1)}  
}$

$\mathsf{  
\dfrac{C'(y)}{y - 1} = \dfrac 1 y  
}$

$\mathsf{  
C'(y) = 1 - \dfrac 1 y  
}$

$\mathsf{  
C(y) = y - \ln(y) + \overline C  
}$

$\mathsf{  
x = \dfrac{y - \ln(y) + \overline C}{(y - 1)^2}  
}$

  

## Особые решения

1. $\mathsf{  
    y(y - 1) = 0  
    }$
    1. $\mathsf{  
        y = 0  
        }$
        
        **ПОДХОДИТ**
        
        **ЯВЛЯЕТСЯ ОСОБЫМ РЕШЕНИЕМ**
        
    2. $\mathsf{  
        y = 1  
        }$
        
        **ПОДХОДИТ**
        
        **ЯВЛЯЕТСЯ ОСОБЫМ РЕШЕНИЕМ**
        
2. $\mathsf{  
    2x = 0  
    }$
    
    **НЕ ПОДХОДИТ**