---
Owner: Artemii
tags:
  - ДЗ
---
683-688

# №683

## Условия

$\mathsf{  
xy'' - (2x + 1)y' + (x + 1)y = 0  
}$

## Решение

$\mathsf{  
y_1 = e^{\lambda x}  
}$

$\mathsf{  
\lambda^2 xe^{\lambda x} - 2x\lambda e^{\lambda x} - \lambda e^{\lambda x} + xe^{\lambda x} + e^{\lambda x} = 0  
}$

$\mathsf{  
e^{\lambda x} \left(\lambda^2x - 2x \lambda - \lambda + x + 1 \right) = 0  
}$

$\mathsf{  
x \left(\lambda^2 - 2 \lambda + 1\right) + x^0 \left(- \lambda + 1\right) = 0x + 0x^0  
}$

$\begin{cases}  
\mathsf{\lambda^2 - 2 \lambda + 1 = 0} \\  
\mathsf{- \lambda + 1 = 0}  
\end{cases} \quad \mathsf{\lambda = 1}$

  

$\mathsf{  
y_1 = e^x  
}$

$\mathsf{  
- \int \dfrac{-(2x + 1)}{x}dx = 2x + \ln(x)  
}$

$\mathsf{  
\dfrac{y_2}{e^x} = \int \dfrac{Ce^{2x} \cdot x}{e^{2x}}dx  
}$

$\mathsf{  
\dfrac{y_2}{e^x} = \dfrac{Cx^2}{2} + C_1  
}$

$\mathsf{  
y = C_1e^x + \dfrac{C_2}{2}x^2  
}$

# №684

## Условия

$\mathsf{  
xy'' + 2y' - xy = 0  
}$

$\mathsf{  
y_1 = \dfrac{e^x}{x}  
}$

## Решение

$\mathsf{  
- \int \dfrac{2}{x}dx = -2 \ln(x)  
}$

$\mathsf{  
\dfrac{xy_2}{e^x} = C\int \dfrac{-2x^3}{e^{2x}}dx = \int \dfrac{C}{e^{2x}}dx = - \dfrac{C}{2e^{2x}} + C_1  
}$

$\mathsf{  
y_2 = -\dfrac C {2e^xx} + C_1 \dfrac{e^x}{x}  
}$

  

# №685

## Условия

$\mathsf{  
y'' - 2(1 + \tg^2(x))y = 0  
}$

$\mathsf{  
y_1 = \tg(x)  
}$

## Решение

$\mathsf{  
- \int \dfrac{0}{1}dx  
}$

$\mathsf{  
\dfrac{y_2}{\tg(x)} = \int \dfrac{Ce^0}{\tg^2(x)}dx = \int \dfrac{C}{\frac{1}{\cos^2} - 1}dx = C\int \dfrac{ \cos^2(x)}{1 - \cos^2(x)}dx = C \int \dfrac{\cos^2(x) - 1}{1 - \cos^2(x)} + \dfrac{1}{1 - \cos^2(x)}dx = -Cx - \dfrac C {\tg(x)} + C_1  
}$

$\mathsf{  
y_2 = - C \left(\tg(x) x + 1\right) + C_1 \tg(x)  
}$

  

# №686

## Условия

$\mathsf{  
x(x - 1) y'' - xy' + y = 0  
}$

## Решение

$\mathsf{  
y_1 = x^n  
}$

$\mathsf{  
n \cdot (n - 1)(x - 1)x^{n - 1} - nx^n + x^n = 0  
}$

$\mathsf{  
x^n \left(n^2 - n - n + 1\right) = 0  
}$

$\mathsf{  
n = 1  
}$

  

$\mathsf{  
y_1 = C_1x + C_2  
}$

  

$\mathsf{  
0 - xC_1 + C_1x + C_2 = 0  
}$

$\mathsf{  
C_2 = 0  
}$

  

$\mathsf{  
-\int \dfrac{-x}{x(x - 1)}dx = \int \dfrac{1}{x - 1}dx = \ln(x - 1)  
}$

$\mathsf{  
\dfrac{y_2}{x} = C \int \dfrac{e^{\ln(x - 1)}}{(x)^2}dx  
}$

$\mathsf{  
y_2 = C x\ln(x) + C + C_1 x  
}$

# №687

## Условия

$\mathsf{  
(e^x + 1)y'' - 2y' - e^xy = 0  
}$

$\mathsf{  
y_1 = e^x - 1  
}$

## Решение

$\mathsf{  
-\int \dfrac{-2}{e^x + 1}dx = 2 x-2\ln\left({e}^{x}+1\right)  
}$

$\mathsf{  
\dfrac{y_2}{e^x - 1} = C\int e^{2x} \dfrac{1}{(e^x - 1)^2 \cdot (e^x + 1)^2}  
}$

$\mathsf{  
y_2 = - C\dfrac{e^x - 1}{2e^{2x} - 2} + C_1(e^x - 1)  
}$

# №688

## Условия

$\mathsf{  
x^2 y'' \ln(x) - xy' + y = 0  
}$

## Решение

$\mathsf{  
y_1 = x^n  
}$

$\mathsf{  
x^n \cdot n \cdot (n - 1) \ln(x) - x^n \cdot n + x^n = 0  
}$

$\mathsf{  
x^n [n - 1][n\ln(x) - 1] = 0  
}$

$\mathsf{  
n = 1  
}$

Подходит

$\mathsf{  
n = \dfrac{1}{\ln(x)}  
}$

Не подходит

  

$\mathsf{  
-\int \dfrac{-x}{x^2 \ln(x)}dx = \int \dfrac{1}{x \ln(x)}dx = \ln(\ln(x))  
}$

$\mathsf{  
\dfrac{y_2}{x} = C \int \dfrac{\ln(x)}{x^2}dx  
}$

$\mathsf{  
y_2 = Cx - C_1 \left(\ln(x) + 1\right)  
}$