---
Owner: Artemii
tags:
  - ДЗ
---
57-64

# №57

$\mathsf{  
2x^2 y\dfrac {dy}{dx} + y^2 = 2  
}$

$\mathsf{  
2x^2y dy = (2 - y^2)dx  
}$

$\mathsf{  
\dfrac{2y dy}{2-y^2} = \dfrac{dx}{x^2}  
}$

$\mathsf{  
\int \dfrac{y dy}{2 - y^2} = \int \dfrac{dx}{x^2}  
}$

$\mathsf{  
-\ln(|y^2 - 2|) + A = -\dfrac 1 x + C  
}$

$\mathsf{  
\ln(|y^2 - 2|) = \dfrac 1 x + C_1  
}$

$\mathsf{  
y^2 = C_1 e^{\frac 1 x} + 2  
}$

  

1. $\mathsf{  
    x^2 = 0  
    }$
    
    $\mathsf{y^2 = 2}$
    
    **НЕ ПОДХОДИТ**
    
2. $\mathsf{  
    y = \pm \sqrt 2  
    }$
    
    $\mathsf{0 = 0}$
    
    **ПОДХОДИТ**
    
    $\mathsf{  
    |y^2 - 2| = e^{x^{-1}} \cdot e^{C_1}  
    }$
    
    $\mathsf{  
    C_2 = e^{C_1}  
    }$
    
    $\mathsf{  
    |y^2 - 2| = e^{x^{-1}} \cdot C_2  
    }$
    

  

# №58

$\mathsf{  
\dfrac{dy}{dx} - xy^2 = 2xy  
}$

$\mathsf{  
\dfrac{dy}{dx} = x(y^2 + 2y)  
}$

$\mathsf{  
\dfrac{dy}{y^2 + 2y} = xdx  
}$

$\mathsf{  
\dfrac 1 {y(y + 2)} = \dfrac {A}{y} + \dfrac{B}{y + 2}  
}$

$\mathsf{  
1 = 2A + Ay + By  
}$

  

$\mathsf{  
0 = A + B  
}$

$\mathsf{  
1 = 2A  
}$

  

$\mathsf{  
B = -\dfrac 1 2  
}$

$\mathsf{  
A = -B = \dfrac 1 2  
}$

  

$\mathsf{  
\int \dfrac 1 2 \left( \dfrac 1 {y} - \dfrac 1 {y + 2} \right) dy = \int x dx  
}$

$\mathsf{  
\dfrac 1 2 \ln(y) - \dfrac 1 2 \ln(y + 2) = \dfrac {x^2} 2 + C  
}$

  

1. $\mathsf{  
    y = 0  
    }$
    
    $\mathsf{0 = 0}$
    
    **ПОДХОДИТ**
    
    $\mathsf{  
    \dfrac 1 2 \ln(y) - \dfrac 1 2 \ln(y + 2) = \dfrac{x^2}{2} + \ln(C)  
    }$e
    
    $\mathsf{  
    \dfrac 1 2\ln ([\dfrac {yC} {y + 2}]) = \dfrac{x^2} 2  
    }$
    
    $\mathsf{  
    \dfrac y {y + 2} \cdot C = e^{x^2}  
    }$
    
    $\mathsf{  
    e^{x^2}\dfrac{y + 2}{y} = C  
    }$
    
2. $\mathsf{  
    y = -2  
    }$
    
    **ПОДХОДИТ**
    
      
    

  

# №59

$\mathsf{  
e^{-s} (1 + \dfrac{ds}{dt}) = 1  
}$

$\mathsf{  
1 + \dfrac{ds}{dt} = \dfrac{1}{e^{-s}}  
}$

$\mathsf{  
ds = (\dfrac{1}{e^{-s}} - 1)dt  
}$

$\mathsf{  
\dfrac{ds}{\dfrac{1}{e^{-s}} - 1} = dt  
}$

$\mathsf{  
\int \dfrac 1 {e^{2s} - e^s} d(e^s) = \int dt  
}$

$\mathsf{  
\ln(|e^s - 1|) - s = t + C  
}$

  

1. $\mathsf{  
    e^s = 1  
    }$
    
    **ПОДХОДИТ**
    
    $\mathsf{  
    \dfrac{e^s - 1}{C} = e^{t + s}  
    }$
    
    $\mathsf{  
    \dfrac{e^s - 1}{e^{t} e^{s}} = C  
    }$
    

# №60

$\mathsf{  
\dfrac{dz}{dx} = 10^{x + z}  
}$

$\mathsf{  
\dfrac{dz}{dx} = 10^x \cdot 10^z  
}$

$\mathsf{  
\dfrac{dz}{10^z} = 10^x dx  
}$

$\mathsf{  
\int -10^{-z} d(-z) = \int 10^x dx  
}$

$\mathsf{  
-\dfrac{1}{\ln(10) \cdot 10^z} = \dfrac{10^x}{\ln(10)} + C  
}$

  

# №61

$\mathsf{  
x \dfrac{dx}{dt} + t = 1  
}$

$\mathsf{  
xdx = (1 - t) dt  
}$

$\mathsf{  
\dfrac{x^2}{2} = t - \dfrac{t^2}{2} + C  
}$

  

# №62

$\mathsf{  
\dfrac{dy}{dx} = \cos(y - x)  
}$

  

$\mathsf{  
t = y - x  
}$

$\mathsf{  
y = t + x  
}$

  

$\mathsf{  
\dfrac{d(t + x)}{dx} = \cos(t)  
}$

$\mathsf{  
\dfrac{dt}{dx} + 1 = \cos(t)  
}$

$\mathsf{  
\dfrac{dt}{\cos(t) - 1} = dx  
}$

$\mathsf{  
z = \tg(\dfrac t 2)  
}$

$\mathsf{  
\cos(t) = \dfrac{1 - z^2}{1 + z^2}  
}$

$\mathsf{  
dt = \dfrac{2dz}{1 + z^2}  
}$

$\mathsf{  
\int \dfrac{\dfrac{2dz}{1 + z^2}}{\dfrac{1 - z^2}{1 + z^2} - 1} = \int dx  
}$

$\mathsf{  
\int \dfrac{2dz}{1 - z^2 - 1 - z^2} = \int dx  
}$

$\mathsf{  
\int \dfrac{2dz}{-2z^2} = \int dx  
}$

$\mathsf{  
\ctg(\dfrac t 2) = x + C  
}$

$\mathsf{  
\ctg(\dfrac{y - x} 2) = x + C  
}$

  

1. $\mathsf{  
    \cos(y - x) = 1  
    }$
    
    $\mathsf{  
    \left[0 = y - x \right]  
    }$
    
    **ПОДХОДИТ**
    
    $\mathsf{  
    C = \dfrac {1}{2y - 2x} - \dfrac 1 {2y} + \dfrac 1 {2x}  
    }$
    

  

# №63

$\mathsf{  
y' - y = 2x - 3  
}$

$\mathsf{  
y' = 2x + y - 3  
}$

$\mathsf{  
t = 2x + y - 3  
}$

$\mathsf{  
y = t - 2x + 3  
}$

  

$\mathsf{  
\dfrac{d(t - 2x + 3)}{dx} = t  
}$

$\mathsf{  
\dfrac{dt}{dx} - 2 = t  
}$

$\mathsf{  
\dfrac{dt}{t + 2} = dx  
}$

  

$\mathsf{  
\ln(2x + y - 3 + 2) = x + C  
}$

  

1. $\mathsf{  
    2x + y = 1  
    }$
    
    $\mathsf{  
    y = 1 - 2x  
    }$
    
    **ПОДХОДИТ**
    
      
    
    $\mathsf{  
    \dfrac{2x + y - 1}{e^x} = C  
    }$
    

  

# №64

$\mathsf{  
(x + 2y) \dfrac {dy}{dx} = 1  
}$

$\mathsf{  
y(0) = -1  
}$

  

$\mathsf{  
t = x + 2y  
}$

$\mathsf{  
y = \dfrac{t - x}{2}  
}$

  

$\mathsf{  
t \dfrac{d(\frac{t - x} 2)}{dx} = 1  
}$

$\mathsf{  
\dfrac t 2(\dfrac{dt}{dx} - 1) = 1  
}$

$\mathsf{  
\dfrac 2 t = \dfrac{dt}{dx} - 1  
}$

$\mathsf{  
dx = \dfrac{dt}{\frac 2 t + 1}  
}$

  

$\mathsf{  
\dfrac 1 {\frac 2 t + \frac t t} = \dfrac t {2 + t} = \dfrac {2 + t - 2}{2 + t} = \dfrac{2 + t}{2 + t} + \dfrac 2 {2 + t}  
}$

  

$\mathsf{  
x = t + 2 \ln(2 + t) + C  
}$

$\mathsf{  
x = x + 2y + 2 \ln(2 + x + 2y) + C  
}$

  

1. $\mathsf{  
    t = -2  
    }$
    
    $\mathsf{  
    x + 2y = -2  
    }$
    
    $\mathsf{  
    y = \dfrac{-x - 2}{2}  
    }$
    
    **ПОДХОДИТ**
    
    $\mathsf{  
    0 = 2y + 2 \ln (\dfrac{2 + x + 2y} C)  
    }$
    
    $\mathsf{  
    e^{-y} = \dfrac{2 + x + 2y}{C}  
    }$
    
    $\mathsf{  
    C = (2 + x + 2y)e^y  
    }$
    
      
    
2. $\mathsf{  
    t = 0  
    }$
    
    $\mathsf{  
    y = \dfrac{-x}{2}  
    }$
    
    **НЕ ПОДХОДИТ**