---
Owner: Artemii
tags:
  - ДЗ
---
527 - 531

591, 592, 600

# №527

## Условия

$\mathsf{  
y''' - 3y'' + 3y' - y =0  
}$

## Решение

$\mathsf{  
\lambda^3 - 3\lambda^2 + 3 \lambda - 1 = 0  
}$

$\mathsf{(\lambda - 1)^3 = 0}$

$\mathsf{  
\lambda = 1  
}$

$\mathsf{  
y = \left(C_1 + C_2x + C_3x^2 \right)e^x  
}$

# №528

## Условия

$\mathsf{  
y''' - y'' - y' + y = 0  
}$

## Решение

$\mathsf{  
\lambda^3 - \lambda^2 - \lambda + 1 = 0  
}$

$\mathsf{  
\left(\lambda^2 - 1\right)(\lambda - 1) = 0  
}$

$\mathsf{  
\lambda = \pm 1  
}$

$\mathsf{  
\lambda = 1  
}$

$\mathsf{  
y = \left(C_1 + C_2x\right)e^x + Ce^{-x}  
}$

# №529

## Условия

$\mathsf{  
y^{(4)} - 5y'' + 4y = 0  
}$

## Решение

$\mathsf{  
\lambda^4 - 5\lambda^2 +4 = 0  
}$

$\mathsf{  
t^2 - 5t +4 = 0  
}$

$\mathsf{  
D = 25 - 16 = 9  
}$

$\mathsf{  
t = \dfrac{5 \pm 3}{2}  
}$

$\mathsf{  
t_1 = 4  
}$

$\mathsf{  
t_2 = 1  
}$

  

$\mathsf{  
\lambda_{1, 2} = \pm 1  
}$

$\mathsf{  
\lambda_{3, 4} = \pm 2  
}$

  

$\mathsf{  
y = \left(C_1 e^x + C_2e^{-x} \right) + \left(C_3e^{2x} + C_4e^{-2x}\right)  
}$

# №530/

## Условия

$\mathsf{  
y^{(5)} + 8y''' + 16y' = 0  
}$

## Решение

$\mathsf{  
\lambda^5 + 8\lambda^3 + 16\lambda = 0  
}$

$\mathsf{  
\lambda_1 = 0  
}$

$\mathsf{  
t^2 + 8t + 16 = 0  
}$

$\mathsf{  
(t + 4)^2 = 0  
}$

$\mathsf{  
\lambda_{2, 3} = \pm 2i  
}$

$\mathsf{  
y = C_1e^{0x} + C_2e^{0x}\cos(2 \cdot x) + C_3e^{0x} \sin(2 \cdot x)  
}$

# №531

## Условия

$\mathsf{  
y''' - 3y' + 2y = 0  
}$

## Решение

$\mathsf{  
\lambda^3 - 3\lambda + 2 = 0  
}$

$\mathsf{  
\lambda \cdot (\lambda^2 - 4) + \lambda + 2 = 0  
}$

$\mathsf{  
(\lambda + 2)\left(\lambda \cdot (\lambda - 2) + 1 \right) = 0  
}$

$\mathsf{  
\lambda^2 - 2\lambda + 1 = 0  
}$

$\mathsf{  
\lambda_1 = -2  
}$

$\mathsf{  
\lambda_{2, 3} = 1  
}$

$\mathsf{  
y = \left(C_1 + C_2 x \right)e^{x} + C_3e^{-2x}  
}$

# №591

## Условия

$\mathsf{  
x^3 y''' + xy' - y = 0  
}$

## Решение

$\mathsf{  
x^3 \lambda^3 + x\lambda - 1 = 0  
}$

$\mathsf{  
x = e^t  
}$

$\mathsf{  
\lambda(\lambda - 1)(\lambda - 2) + (\lambda - 1) = 0  
}$

$\mathsf{  
\lambda = 1  
}$

$\mathsf{  
\lambda^2 - 2 \lambda + 1 = 0  
}$

$\mathsf{  
\lambda_{2, 3} = 1  
}$

$\mathsf{  
y = \left(C_1 + C_2t + C_3t^2 \right)e^{t} = \left(C_1 + C_2ln(x) + C_3 \ln(x)^2\right)x  
}$

# №592

## Условия

$\mathsf{  
x^2 y''' = 2y'  
}$

## Решение

$\mathsf{  
x^2 \lambda^3 - 2\lambda = 0  
}$

$\mathsf{  
\lambda(\lambda - 1)(\lambda - 2) - 2 \lambda = 0  
}$

$\mathsf{  
\lambda_{1, 2} = 0  
}$

$\mathsf{  
\lambda = 3  
}$

$\mathsf{  
y = \left(C_1 + C_2t\right) e^{0e^{t}} + C_3 e^{3t} = C_1 + C_2\ln(x) + C_3x^3  
}$

# №600

## Условия

$\mathsf{  
(2x + 3)^3 y''' + 3(2x + 3)y' - 6y = 0  
}$

## Решение

$\mathsf{  
p = 2x + 3  
}$

$\mathsf{  
p = e^t  
}$

$\mathsf{  
t = \ln(2x + 3)  
}$

$\mathsf{  
8 \lambda(\lambda - 1)(\lambda - 2) + 6 \left(\lambda - 1\right) = 0  
}$

$\mathsf{  
\lambda = 1  
}$

$\mathsf{  
8\lambda(\lambda - 2) + 6 = 0  
}$

$\mathsf{  
8\lambda^2 - 16\lambda + 6 = 0  
}$

$\mathsf{  
\lambda_{1, 2} = 1 \pm \dfrac 1 2  
}$

$\mathsf{  
y = C_1(2x + 3) + C_1 \left(2x + 3\right)^{\frac 1 2} + C_2 \left(2x + 3\right)^{\frac 3 2}  
}$