---
Owner: Artemii
tags:
  - ДЗ
---
# №251

## Условия

$\mathsf{  
(y')^2 + xy = y^2 + xy'  
}$

## Решение

$\mathsf{  
(y')^2 - y^2 = x(y' - y)  
}$

$\mathsf{  
(y' - y)(y' + y) = x(y' - y)  
}$

### Первое решение

$\mathsf{  
y' + y = x  
}$

**Лагранж**

$\mathsf{  
y' + y = 0  
}$

$\mathsf{  
\dfrac{dy}{y} = -dx  
}$

$\mathsf{  
\ln(y) = -x + C  
}$

$\mathsf{  
y = Ce^{-x}  
}$

$\mathsf{  
y' = C'(x) e^{-x} + C(x) e^{-x} \cdot (-1)  
}$

$\mathsf{  
C'(x) e^{-x} - C(x) e^{-x} + C(x) e^{-x} = x  
}$

$\mathsf{  
C'(x) = x e^x  
}$

$\mathsf{  
C(x) = xe^x + \int e^x dx = (x - 1) e^x + \overline C  
}$

  

$\mathsf{  
y = x - 1 + e^{-x} \overline C  
}$

  

### Второе решение

$\mathsf{  
y' - y = 0  
}$

$\mathsf{  
y' = y  
}$

$\mathsf{  
\dfrac{dy} y = dx  
}$

$\mathsf{  
\ln(y) = x + C  
}$

$\mathsf{  
y = Ce^x  
}$

  

$\mathsf{  
\begin{cases}  
\mathsf{(y')^2 - y^2 = x(y' - y)} & \mathsf{(\dfrac x 2)^2 -y^2 = x(\dfrac x 2 - y) } \\  
\mathsf{2y' = x} & \mathsf{y = \dfrac x 2}  
\end{cases}  
}$

**НЕ ПОДХОДИТ**

## Особые решения

1. $\mathsf{  
    y = 0  
    }$
    
    **ПОДХОДИТ**
    
    $\mathsf{  
    \begin{cases}  
    \mathsf{0 = Ce^x} & \mathsf{0 = 0}  
    \end{cases}  
    }$
    
    **НЕ ЯВЛЯЕТСЯ ОСОБЫМ РЕШЕНИЕМ**
    
2. $\mathsf{  
    y = \dfrac x 2  
    }$
    
    **НЕ ПОДХОДИТ**
    

# №252

## Условия

$\mathsf{  
xy' (xy' + y) = 2y^2  
}$

## Решение

$\mathsf{  
x^2 (y')^2 + xyy' - 2y^2 = 0  
}$

$\mathsf{  
D = (xy)^2 - 4 \cdot x^2 \cdot (-2y^2) = 9x^2 y^2  
}$

$\mathsf{  
y' = \dfrac y x  
}$

$\mathsf{  
y' = - \dfrac{2y} x  
}$

  

### Решение для $\mathsf{  
y' = \dfrac y x  
}$

$\mathsf{  
y = C_1 x  
}$

### Решение для $\mathsf{  
y' = - \dfrac {2y}{x}  
}$

$\mathsf{  
\dfrac{dy}y = -\dfrac{2dx}x  
}$

$\mathsf{  
\ln(y) = C_2 - 2 \ln(x)  
}$

$\mathsf{  
y = \dfrac{C_2}{x^2}  
}$

  

$\mathsf{  
\begin{cases}  
\mathsf{xy'(xy' + y) = 2y^2} & \mathsf{-\dfrac{x^2y}{2x^2}(-\dfrac{x^2y}{2x^2} + y) = 2y^2} \\  
\mathsf{2x^2 y' + xy = 0} & \mathsf{y = 0}  
\end{cases}  
}$

$\mathsf{  
\begin{cases}  
\mathsf{C_1 x = 0} & \mathsf{\dfrac{C_2}{x^2} = 0} \\  
\mathsf{C_1 = 0} & \mathsf{-\dfrac{2C_2}{x^3} = 0}  
\end{cases}  
}$

## Особые решения

1. $\mathsf{y = 0}$
    
    **ПОДХОДИТ**
    
    **НЕ ЯВЛЯЕТСЯ ОСОБЫМ РЕШЕНИЕМ (****$\mathsf{C_1 = 0}$****)**
    

# №253

## Условия

$\mathsf{  
x(y')^2 - 2yy' + x = 0  
}$

## Решение

$\mathsf{  
p = y'  
}$

$\mathsf{  
dy = pdx  
}$

$\mathsf{  
y = \dfrac{px}{2} + \dfrac{x}{2p}  
}$

$\mathsf{  
dy = \dfrac{p^3 dx + pdx + p^2xdp - xdp}{2p^2}  
}$

$\mathsf{  
\left(\dfrac p 2 - \dfrac 1 {2p} \right)dx = \left(\dfrac x 2 - \dfrac x {2p^2}\right)dp  
}$

$\mathsf{  
dx = \dfrac{xdp}{p}  
}$

$\mathsf{  
\ln(x) = \ln(p) + C  
}$

$\mathsf{  
x = pC  
}$

$\mathsf{  
y = \dfrac{x^2 + C^2}{2C}  
}$

  

$\mathsf{  
\begin{cases}  
\mathsf{x(y')^2 - 2yy' + x = 0} & \mathsf{x(\dfrac y x)^2 - 2y \dfrac y x + x = 0} \\  
\mathsf{2xy' - 2y = 0} & \mathsf{y = \pm x}  
\end{cases}  
}$

$\mathsf{  
\begin{cases}  
\mathsf{\dfrac{x^2 + C^2}{2C} = \pm x} \\  
\mathsf{\dfrac{x}{C} = 0}  
\end{cases}  
}$

**Подходит**

**Является особым решением**

## Особые решения

1. $\mathsf{  
    2p = 0  
    }$
    
    $\mathsf{  
    p = 0  
    }$
    
    **НЕ ПОДХОДИТ**
    
2. $\mathsf{  
    x = 0  
    }$
    
    **НЕ ПОДХОДИТ**
    
3. $\mathsf{  
    \dfrac p 2 - \dfrac 1 {2p} = 0  
    }$
    
    **НЕ ПОДХОДИТ**
    

# №254

## Условия

$\mathsf{  
x (y')^2 = y(2y' - 1)  
}$

## Решение

$\mathsf{  
p = y'  
}$

$\mathsf{  
x (y')^2 = y(2y' - 1)  
}$

$\mathsf{  
x p^2 = y(2p - 1)  
}$

$\mathsf{  
dx = \dfrac{dy}p  
}$

$\mathsf{  
x = \dfrac{2y}{p} - \dfrac y{p^2}  
}$

$\mathsf{  
dx = \dfrac{2p^2 dy - pdy - 2pydp + 2ydp}{p^3}  
}$

$\mathsf{  
(\dfrac 1 p - 1)dy = (\dfrac{2y}{p^2} - \dfrac{2y}{p})dp  
}$

$\mathsf{  
\dfrac{dy}{y} = \dfrac{2dp}{p}  
}$

$\mathsf{  
\ln(y) = 2 \ln(p) + C  
}$

$\mathsf{  
y = p^2 C  
}$

$\mathsf{  
p = \pm \sqrt{\dfrac y C}  
}$

$\mathsf{  
x = \dfrac{2y}{\pm \sqrt{\dfrac y C}} - \dfrac{y}{\dfrac y C}  
}$

$\mathsf{  
x = \pm 2 \sqrt C \sqrt y - C  
}$

$\mathsf{  
y = \dfrac{C^2 + 2 Cx + x^2}{4C}  
}$

$\mathsf{  
\begin{cases}  
\mathsf{x(y')^2 = y(2y' - 1)} & \mathsf{x(\dfrac{y}{x})^2 - y(2 \dfrac y x - 1) = 0} \\  
\mathsf{2xy' - 2y = 0} & \mathsf{y = 0 \quad y = x}  
\end{cases}  
}$

**ПОДХОДИТ**

$\mathsf{  
\begin{cases}  
\mathsf{x = \dfrac{C^2 + 2Cx + x^2}{4C}} \\  
\mathsf{1 = \dfrac 1 2 + \dfrac{x}{2C}}  
\end{cases}  
}$

Является особым решением

$\mathsf{  
\begin{cases}  
\mathsf{0 = \dfrac{C^2 + 2Cx + x^2}{4C}} \\  
\mathsf{0 = \dfrac 1 2 + \dfrac x {2C}}  
\end{cases}  
}$

Является особым решением

  

## Особые решения

1. $\mathsf{  
    p^2 = 0  
    }$
    
    $\mathsf{  
    y = 0  
    }$
    
    **ПОДХОДИТ**
    
    **ЯВЛЯЕТСЯ ОСОБЫМ РЕШЕНИЕМ**
    
2. $\mathsf{  
    \dfrac 1 p - 1 = 0  
    }$
    
    $\mathsf{  
    y = x  
    }$
    
    **ПОДХОДИТ**
    
    **ЯВЛЯЕТСЯ ОСОБЫМ РЕШЕНИЕМ**
    
      
    

# №255

## Условия

$\mathsf{  
(y')^2 + x = 2y  
}$

## Решение

$\mathsf{  
p = y'  
}$

$\mathsf{  
dx = \dfrac {dy} p  
}$

$\mathsf{  
x = 2y - p^2  
}$

$\mathsf{  
dx = 2dy - 2p dp  
}$

$\mathsf{  
dy = p(2dy - 2pdp)  
}$

$\mathsf{  
dy = \dfrac{2p^2}{2p - 1}dp  
}$

$\mathsf{  
y = \dfrac 1 4 \ln(2p - 1) + \dfrac 1 2 (p^2 + p) + C  
}$

$\mathsf{  
- \ln( \pm 2 \sqrt{2y - x} - 1) \mp 2 \sqrt{2y - x} = C - 2x  
}$

$\mathsf{\dfrac 1 2\ln(\pm 2 \sqrt{y - x} - 1) \pm \sqrt{2y - x} + \dfrac 1 2C = x}$

  

$\mathsf{  
\begin{cases}  
\mathsf{(y')^2 + x = 2y} & \mathsf{0 + x = 2y} \\  
\mathsf{2y' = 0} & \mathsf{y = \dfrac x 2}  
\end{cases}  
}$

**НЕ ПОДХОДИТ**

  

## Особые решения

1. $\mathsf{  
    1 - 2p = 0  
    }$
    
    $\mathsf{  
    p = \dfrac 1 2  
    }$
    
    $\mathsf{  
    y = \dfrac 1 2 x + \dfrac 1 8  
    }$
    
    **ПОДХОДИТ**
    
    **ЯВЛЯЕТСЯ ОСОБЫМ РЕШЕНИЕМ**
    

# №256

## Условия

$\mathsf{  
(y')^3 + (x + 2)e^y = 0  
}$

## Решение

$\mathsf{  
y' = - \sqrt[3]{x + 2} e^{\frac y 3}  
}$

$\mathsf{  
\dfrac{dy}{e^{\frac y 3}} = - \sqrt[3]{x + 2}dx  
}$

$\mathsf{  
y = 3 \left(- \ln\left[\sqrt[3]{x + 2} (3x + 6) + C \right] + \ln(3) + 2 \ln(2)\right)  
}$

$\begin{cases}  
\mathsf{(y')^3 + (x + 2) e^y = 0} & \mathsf{(x + 2) e^y = 0} \\  
\mathsf{3(y')^2 = 0} & \mathsf{x = -2}  
\end{cases}$

**НЕ ПОДХОДИТ**

## Особые решения

1. $\mathsf{  
    e^{\frac y 3} = 0  
    }$
    
    **НЕ ПОДХОДИТ**