---
Owner: Artemii
tags:
  - Практика
---
# №1

$\mathsf{  
(y + 2) dx = (2x + y - 4) dy  
}$

$\mathsf{  
\dfrac{y + 2}{2x + y - 4} = \dfrac{dy}{dx}  
}$

  

$\mathsf{  
\begin{cases}  
\mathsf{y + 2 = 0} & \mathsf{y = -2} & \mathsf{y = -2} \\  
\mathsf{2x + y - 4 = 0} & \mathsf{2x = 6} & \mathsf{x = 3}  
\end{cases}  
}$

  

$\mathsf{  
\begin{matrix}  
\mathsf{u = y + 2} & \mathsf{y = u - 2} \\  
\mathsf{v = x - 3} & \mathsf{x = v + 3}  
\end{matrix}  
}$

  

$\mathsf{  
\dfrac{u}{2v + u} = \dfrac{du}{dv}  
}$

  

$\mathsf{  
t = \dfrac u v  
}$

$\mathsf{  
u = tv  
}$

  

$\mathsf{  
t + v\dfrac{dt}{dv} = \dfrac{t}{2 + t}  
}$

  

$\mathsf{  
\dfrac{dt}{\dfrac{t}{2 + t} - t} = \dfrac{dv}{v}  
}$

$\mathsf{  
\ln(|t + 1|) - 2 \ln(|t|) - \ln(|v|) = C  
}$

$\mathsf{  
\ln(|\dfrac u v + 1|) - 2 \ln(|\dfrac u v|) - \ln(|v|) = C  
}$

$\mathsf{  
y + 2 \quad x - 3  
}$

$\mathsf{  
\ln(|\dfrac{y + 2}{x - 3} + 1|) - 2\ln(|\dfrac{y + 2}{x - 3}|) - \ln(|x - 3|) = \ln(|C|)  
}$

  

  

  

1. $\mathsf{  
    2x + y - 4 = 0  
    }$
2. $\mathsf{  
    2 + t = 0  
    }$
3. $\mathsf{  
    v = 0  
    }$
    
    $\mathsf{  
    x = 3  
    }$
    
4. $\mathsf{  
    \dfrac{t}{2 + t}-t = 0  
    }$

  

# №2

$\mathsf{  
\dfrac{dy}{dx} = \dfrac{2x + y + 1}{4x + 2y - 3}  
}$

$\mathsf{  
z = 2x + y + 1  
}$

$\mathsf{  
y = 2x - z + 1  
}$

$\mathsf{  
y' = 2 - \dfrac{dz}{dx}  
}$

$\mathsf{  
\dfrac{z}{z - 5} = 2 - \dfrac{dz}{dx}  
}$

$\mathsf{  
\int \dfrac{dz(2z - 5)}{5z - 10} = \int dx  
}$

  

# №3

$\mathsf{  
x^3 (y' - x) = y^2  
}$

$\mathsf{  
y = z^m  
}$

$\mathsf{  
x^3 (m z^{m - 1} z' - x) = z^{2m}  
}$

  

$\mathsf{  
mx^3 z^{m - 1} z' - x^4 = z^{2m}  
}$

$\mathsf{  
m - 1 + 3 = 4 = 2m  
}$

$\mathsf{m = 2}$

  

$\mathsf{  
x^3 (2z z' - x) = z^4  
}$

$\mathsf{  
z' = \dfrac{z^4 + x^4}{2x^3z}  
}$

$\mathsf{  
u = \dfrac z x  
}$

$\mathsf{  
z = ux  
}$

$\mathsf{  
u'x = \dfrac{x^4(u^4 + 1)}{2x^4 u}  
}$

$\mathsf{  
u' = \dfrac{(u^2 - 1)^2}{2ux}  
}$

  

$\mathsf{  
\dfrac{du \cdot u}{dv(u^2 - 1)^2} = \dfrac 1 2 \ln(x) + \ln(C)  
}$

  

$\mathsf{  
\dfrac 1 2 \int \dfrac{d(u^2 -1)}{(u^2 - 1)^2} = - \dfrac 1 {u^2 - 1} = \ln(x) + C  
}$

  

# №4

$\mathsf{  
2x^2 y' = y^3 + xy  
}$

$\mathsf{  
y = z^m  
}$

$\mathsf{  
2x^2 \cdot m z^{m - 1} \cdot z' = z^{3m} + xz^m  
}$

  

  

ДЗ:  
118-120  

122-127