---
Owner: Artemii
tags:
  - Практика
---
  

$\mathsf{  
F(x, y, y', \ldots, y^{(n)})  
}$

$\mathsf{  
F(x, ky, ky', \ldots, ky^{(n)}) = k^m F(x, y, y', \ldots, y^{(m)})  
}$

$\mathsf{  
y' = yz  
}$

$\mathsf{  
z = z(x)  
}$

  

# №1

$\mathsf{  
y \cdot y^{(2)} = (y')^2 + 15 y^2 \sqrt x  
}$

  

  

$\mathsf{  
F(\xi x, \xi^k y, \xi^{k - 1} y', \ldots, \xi^{k - n} y^{(n)}) = \xi^m F(x, y, y', \ldots, y^{(n)})  
}$

$\mathsf{  
x = e^t  
}$

$\mathsf{  
y = z(t) \cdot e^{kt}  
}$

  

# №2

$\mathsf{  
\dfrac{y^2}{x^2} + (y')^2 = 3xy'' + \dfrac 2x y y'  
}$

$\mathsf{  
-2 + 2k = 2k - 2 = k - 1 = 2k - 2 \implies k = 1  
}$

$\mathsf{  
y' = (z'_t + z)t'_x e^t = z' + z  
}$

$\mathsf{  
y'' = (z'' + z') e^{-t}  
}$

$\mathsf{  
\dfrac{dx}{dt} = e^t  
}$

$\mathsf{  
\dfrac{dt}{dx} = e^{-t}  
}$

$\mathsf{  
z^2 + (z' + z)^2 = 3(z'' + z'') + 2z (z' + z)  
}$

$\mathsf{  
z^3 + (z')^2 + z^2 + 2zz' = 3z'' + 3z' + 2zz' + 2z^2  
}$

$\mathsf{  
(z')^2 - 3z'' = 3z'  
}$

$\mathsf{  
z' = u(t)  
}$

$\mathsf{  
z'' = u'  
}$

$\mathsf{  
u^2 - 3u' - 3u = 0  
}$

$\mathsf{  
\int \dfrac{3}{u^2 - 3u}du = \int dt  
}$

$\mathsf{  
\ln(|\dfrac{u - 3}{u}|) + C = t  
}$

$\mathsf{  
e^{t + C} = 1 - \dfrac 3 u  
}$

Дальше всё аналогично

  

  

$\mathsf{  
F(x, y, y', \ldots, y^{(n)}) = G'(x, y, y', \ldots, y^{(n)})  
}$

$\mathsf{  
yy'' + (y')^2 + 2y^2 (y')^2 = \dfrac{yy'} x  
}$

$\mathsf{  
(yy')' = \dfrac{yy'}{x} - 2(yy')^2  
}$

$\mathsf{  
\dfrac{(y y')'}{yy'} = \dfrac 1 x - (y^2)'  
}$

$\mathsf{  
(\ln(yy'))' = (\ln(x))' - (y^2)'  
}$

$\mathsf{  
\ln(yy') - \ln(x) + y^2 = C  
}$

$\mathsf{  
\dfrac{(y^2)'}{x} = \dfrac{yy'}{2x} = C_0 e^{-y^2}  
}$

$\mathsf{  
(y^2)' e^{y^2} = 2C_0 x  
}$

$\mathsf{  
(e^{y^2})' = 2C_0x  
}$

$\mathsf{  
e^{y^2} = C_0 x^2 + C_1  
}$

  

ДЗ

456, 457, 459, 466-471