---
Owner: Artemii
tags:
  - Практика
---
Однородная функция порядка $\mathsf k$

$\mathsf{  
M(\lambda x \lambda y) = \lambda^k M(x, y)  
}$

$\mathsf{  
\forall \lambda > 0  
}$

  

$\mathsf{  
(x + 2y) dx - x dy = 0  
}$

$\mathsf{  
y' = f(\dfrac y x)  
}$

$\mathsf{  
y' = \dfrac{dy}{dx} = \dfrac{x + 2y} 2 = 1 + \dfrac{2y} x  
}$

  

$\mathsf{  
\dfrac y x = z  
}$

$\mathsf{  
y' = \dfrac{2y} x  
}$

$\mathsf{  
y = x \cdot z  
}$

$\mathsf{  
y' = z(x) + x z'(x)  
}$

  

$\mathsf{  
z + xz' = 1 + \dfrac{2x \cdot z}{x}  
}$

$\mathsf{  
xz' = 1+ z  
}$

  

$\mathsf{  
\dfrac{dz}{dx} = \dfrac{1 + z} x  
}$

$\mathsf{  
\dfrac{dz}{1 + z} = \dfrac{dx} x  
}$

$\mathsf{  
\ln(1 + z) = \ln (Cx)  
}$

$\mathsf{  
1 + z = Cx  
}$

$\mathsf{  
1 + \dfrac y x = Cx  
}$

$\mathsf{  
x + y = Cx ^2  
}$

  

1. $\mathsf{  
    x = 0  
    }$
    
    **ПОДХОДИТ**
    
2. $\mathsf{  
    z = -1  
    }$
    
    $\mathsf{  
    y = -x  
    }$
    
    **ПОДХОДИТ**
    
    Не является специальным решением при $\mathsf{  
    C = 0  
    }$
    

  

  

# №2

$\mathsf{  
(x - y) dx + (x + y) dy = 0  
}$

Проверка на однородность:

$\mathsf{  
(kx \pm ky) = k (x \pm y)  
}$

  

$\mathsf{  
t = \dfrac y x  
}$

$\mathsf{  
y = tx  
}$

  

$\mathsf{  
(x - tx) dx + (x + tx) d(tx) = 0  
}$

$\mathsf{  
d(tx) = t dx + x dt  
}$

  

$\mathsf{  
x(1 - t) dx + xt(1 + t)dx + x^2 (1 + t)dt = 0  
}$

$\mathsf{  
(1 + t^2) dx + x (1 + t) dt = 0  
}$

  

$\mathsf{  
\int \dfrac{dx} x = -\int \dfrac{1 + t}{1 + t^2} dt  
}$

$\mathsf{  
\ln(x) = - \left(\arctg(t) + \dfrac 1 2 \ln(t^2 + 1)\right)  
}$

$\mathsf{  
\arctg(t) + \ln (\sqrt{t^2 + 1}) = \ln(\dfrac C x)  
}$

  

1. $\mathsf{  
    x = 0  
    }$
    
    **НЕПОДХОДИТ**
    

  

# №3

$\mathsf{  
(x^2 + y^2) y' = 2xy  
}$

$\mathsf{  
((kx)^2 + (ky)^2) = k (x^2 + y^2)  
}$

$\mathsf{  
t = \dfrac yx  
}$

$\mathsf{  
y = tx  
}$

  

$\mathsf{  
\dfrac{dy}{dx} = \dfrac{2xy}{x^2 + y^2}  
}$

  

$\mathsf{  
x\dfrac{dt}{dx} + t = \dfrac{2x^2 t}{x^2 + t^2x^2}  
}$

$\mathsf{  
\dfrac {dt}{dx} x + t = \dfrac{2t}{1 + t^2}  
}$

$\mathsf{  
\dfrac{dt}{\dfrac{3t + t^3}{1 + t^2}} = \dfrac{dx}{x}  
}$

$\mathsf{  
\int \dfrac{(1 + t^2) dt}{3t + t^3} = \int \dfrac{dx}{x}  
}$

  

$\mathsf{  
\dfrac{1}{t(3 + t^2)} = \dfrac{A}{t} + \dfrac{Bt + C}{3 + t^2}  
}$

  

ПРОПУСТИМ

  

$\mathsf{  
\dfrac{t}{t^2 - 1} = xC  
}$

  

$\mathsf{  
\dfrac{\dfrac y x}{(\dfrac y x)^2 - 1} = xC  
}$

$\mathsf{  
\dfrac{yx}{y^2 - x^2} = C  
}$

  

1. $\mathsf{  
    t = 0  
    }$
    
    $\mathsf{  
    y = 0  
    }$
    
    **ПОДХОДИТ**
    
2. $\mathsf{  
    y = \pm x  
    }$
    
      
    
      
    

# №4

$\mathsf{  
y^2 + x^2 y' = xy y'  
}$

$\mathsf{  
y^2 dx = (xy - x^2)dy  
}$

  

$\mathsf{  
y = tx  
}$