---
Owner: Artemii
tags:
  - Практика
---
# №1

$\mathsf{  
2xydx + (x^2 - y^2) dy = 0  
}$

$\mathsf{  
(2xy)'_y = 2x \quad F'_x = 2xy \implies F = x^2 y + \phi(y)  
}$

$\mathsf{  
(x^2 - y^2)'_x = 2x \quad F'_y = x^2 - y^2  
}$

(Подставляем $\mathsf F$ в $\mathsf{F’_y}$)

$\mathsf{  
F'_y = x^2 + \phi'(y) = x^2 - y^2 \iff \phi'(y) = -y^2 \iff \phi(y) = -\dfrac{y^3} 3 + C  
}$

$\mathsf{  
x^2 y - \dfrac{y^3} 3 = C  
}$

  

## №2

$\mathsf{  
(x^2 + y^2 + x) dx + ydy = 0  
}$

  

$\mathsf{  
(x^2 + y + x)'_y = 2y  
}$

$\mathsf{  
y'_x = 0  
}$

$\mathsf{  
N p'_x - Mp'_y = p(M'_y - N'_x)  
}$

  

$\mathsf{  
yp'_x - (x^2 + y^2 + x)p'_y = p \cdot 2y  
}$

  

Пусть $\mathsf{  
p = p(x)  
}$

  

$\mathsf{  
y p'_x = p \cdot 2y  
}$

$\mathsf{  
\dfrac{dp} p = 2dx  
}$

$\mathsf{  
\ln(p) = 2x  
}$

$\mathsf{  
p = e^{2x}  
}$

  

$\mathsf{  
e^{2x}(x^2 + y^2 + x)dx + e^{2x} y dy = 0  
}$

$\mathsf{  
(e^{2x}(x^2 + y^2 + x))'_y = 2e^{2x} \cdot y  
}$

$\mathsf{  
(e^{2x} y)'_x = 2e^{2x} \cdot y  
}$

  

$\mathsf{  
F'_x = M = e^{2x}(x^2 + y^2 + x)dx  
}$

$\mathsf{  
F'_y = N = e^{2x} y dy \implies F = e^{2x} \cdot \dfrac{y^2} 2 + \phi(x)  
}$

  

$\mathsf{  
F'_x = e^{2x} y^2 + \phi'(x)= e^{2x}(x^2 + y^2 + x)  
}$

$\mathsf{  
\phi'(x) = e^{2x} (x^2 + x)dx  
}$

$\mathsf{  
\phi(x) = \dfrac{x^2} 2 \cdot e^{2x}  
}$

$\mathsf{  
F = e^{2x} \dfrac{y^2} 2 + \dfrac{x^2} 2 e^{2x} = C  
}$

  

# ДОП

$\mathsf{  
d(xy) = ydx + xdy \quad d(y^2) = 2y dy  
}$

$\mathsf{  
d(\dfrac x y) = \dfrac{y dx - xdy}{y^2} \quad d() = \dfrac{dy} y  
}$

  

$\mathsf{  
(x^2 + y^2 + x) dx + y dy = 0  
}$

$\mathsf{  
(x^2 + y^2) + \dfrac 1 2 d(x^2) + \dfrac 1 2 d(y^2) = 0  
}$

$\mathsf{  
(x^2 + y^2) dx + \dfrac 1 2 d(x^2 + y^2) = 0  
}$

$\mathsf{  
tdx + \dfrac 1 2 dt = 0  
}$

  

# №3

## Условия

$\mathsf{  
(x^2 + y^2 + y) dx - x dy = 0  
}$

$\mathsf{  
(x^2 + y^2 + y)'_y = 2y + 1  
}$

$\mathsf{  
-x'_x = -1  
}$

  

$\mathsf{  
p'_x N - p'_yM = p(M'_y - N'_x)  
}$

  

$\mathsf{  
-p'_xx - p'_y(x^2 + y^2 + y) = p(2y +2)  
}$

  

$\mathsf{  
(x^2 + y^2)dx + y^2d(\dfrac x y) = 0  
}$

$\mathsf{  
t = \dfrac y x \quad y = tx  
}$

$\mathsf{  
(t^2 + 1)dx = -dt  
}$

  

$\mathsf{  
-dx = \dfrac{dt}{t^2 + 1}  
}$

  

$\mathsf{  
-x = \arctg(t) + C  
}$

$\mathsf{  
-x = \arctg(\dfrac x y) + C  
}$

  

1. $\mathsf{  
    y = 0  
    }$
    
    **НЕ ЯВЛЯЕТСЯ ОСОБЫМ РЕШЕНИЕМ**
    
      
    

# №4

$\mathsf{  
xy^2(xy' + y) = 1  
}$

$\mathsf{  
x^2 y^2 y' + xy^3 - 1 = 0  
}$

$\mathsf{  
(x^2 y^2) dy + (xy^3 - 1) dx = 0  
}$

$\mathsf{  
(xy^3 - 1) dx + x^2 y^2 dy = 0  
}$

  

$\mathsf{  
(xy^3 - 1)'_y = 3xy^2  
}$

$\mathsf{  
(x^2 y^2)'_x = 2xy^2  
}$

  

$\mathsf{  
p'_x x^2y^2 - p'_y(xy^3) = p_xy^2  
}$

$\mathsf{  
1  
}$

  

$\mathsf{  
\dfrac{dp}{p} = \dfrac{dx} x  
}$

$\mathsf{  
\ln(p) = \ln(x)  
}$

$\mathsf{p = x}$

$\mathsf{  
(x^2 y^3 - x)dx + x^3 y^2 dy = 0  
}$

  

$\mathsf{  
(x^2 y^3 - x)'_y = 3x^2 y^2  
}$

$\mathsf{  
(x^3y^2)'_x = 3x^2y^2  
}$

  

  

  

  

187-190

199-203