---
Owner: Artemii
tags:
  - Практика
---
# Теория

$\mathsf{  
F(x, y, y') = 0  
}$

$\mathsf{  
x = \Phi(y, y')  
}$

$\mathsf{  
y = \psi(x, y')  
}$

  

$\mathsf{  
y' = p  
}$

$\mathsf{  
x = \Phi(y, p)  
}$

$\mathsf{  
dx = d \Phi(y, p) = \dfrac{\partial \Phi}{\partial y} \cdot dy + \dfrac{\partial \Phi}{\partial p} dp  
}$

  

$\mathsf{  
y' = \dfrac{dy}{dx} = p  
  
}$

$\mathsf{  
dx = \dfrac{dy} p  
}$

$\mathsf{  
p \neq 0!  
}$

  

$\mathsf{  
dy\left(\dfrac 1 p - \dfrac{\partial \Phi}{\partial y}\right) = \dfrac{\partial \Phi}{\partial p} dp  
}$

$\mathsf{  
y = \phi(p, c)  
}$

  

$\mathsf{  
\begin{cases}  
\mathsf{x = \Phi(\phi(p, c), p)} \\  
\mathsf{y = \phi(p, c)}  
\end{cases}  
}$

# №267

## Условия

$\mathsf{  
x = (y')^3 + y'  
}$

## Решение

$\mathsf{  
y' = p  
}$

$\mathsf{  
x = p^3 + p  
}$

$\mathsf{  
dx = 3p^2 dp + dp  
}$

$\mathsf{  
\dfrac{dy}{p} = 3p^2 dp + dp  
}$

$\begin{cases}  
\mathsf{  
y = \dfrac{3}{4}p^4 + \dfrac 1 2 p^2 + C  
} \\  
\mathsf{x = p^3 + p}  
\end{cases}$

## Особые решения

1. $\mathsf{  
    p = 0  
    }$
    
    **НЕ ПОДХОДИТ**
    

  

# №271

## Условия

$\mathsf{  
y = (y')^2 + 2(y')^3  
}$

$\mathsf{  
y' = p  
}$

## Решение

$\mathsf{  
y' = p = \dfrac{dy}{dx}  
}$

$\mathsf{  
dy = pdx  
}$

  

$\mathsf{  
y = p^2 + 2p^3  
}$

$\mathsf{  
dy = (2p + 6p^2)dp  
}$

$\mathsf{  
pdx = (2p + 6p^2)dp  
}$

$\mathsf{  
dx = (2 + 6p) dp  
}$

$\begin{cases}  
\mathsf{x = 2p + 3p^2 + C}\\  
\mathsf{y = p^2 + 2p^3}  
\end{cases}$

  

## Особые решения

1. **$\mathsf{  
    p = 0  
    }$**
    
    **ПОДХОДИТ**
    
    **ЯВЛЯЕТСЯ ОСОБЫМ РЕШЕНИЕМ**
    

# №293

## Условия

$\mathsf{  
xy' - y = \ln(y')  
}$

## Решение

$\mathsf{  
y = xy' - \ln(y')  
}$

$\mathsf{  
p = y'  
}$

$\mathsf{  
dy = pdx  
}$

$\mathsf{  
y = xp - \ln(p)  
}$

  

$\mathsf{  
dy = xdp + pdx - \dfrac{dp} p  
}$

$\mathsf{  
0 = xdp - \dfrac{dp} p  
}$

$\mathsf{  
x = \dfrac 1 p  
}$

$\mathsf{  
y = \dfrac 1 p \cdot p - \ln(p)  
}$

  

$\mathsf{  
p = \dfrac 1 x  
}$

$\mathsf{  
y = 1 + \ln(x)  
}$

Проверка:

$\mathsf{  
1 + \ln(x) = 1 - \ln(\dfrac 1 x) = 1 + \ln(x)  
}$

**Особое решение**

$\mathsf{  
dp = 0  
}$

$\mathsf{  
p = C  
}$

$\mathsf{  
y = xC - \ln(C)  
}$

**Общее**

$\mathsf{  
y' = \dfrac 1 x  
}$

  

# №286

## Условие

$\mathsf{  
y(y - 2xy')^3 = (y')^2  
}$

## Решение

$\mathsf{  
(y - 2xy')^3 = \dfrac{(y')^2}y  
}$

$\mathsf{  
y - 2xy' = (\dfrac{(y')^2}{y})^{\frac 1 3}  
}$

$\mathsf{  
x = \dfrac{y}{(y')^2} - \dfrac 1 2 (\dfrac{(y')^2}{y})^{\frac 1 3} \cdot \dfrac 1 {y'}  
}$

## Особые решения

1. $\mathsf{  
    y = 0  
    }$
    
    **ПОДХОДИТ**
    

  

275-280

294-296