---
Owner: Artemii
tags:
  - Практика
---
# №1

$\mathsf{  
\overline F = m \overline a  
}$

$\mathsf{  
r(t) = x (t) \cdot \overline i + y (t)\cdot \overline j  
}$

  

$\mathsf{  
\overline a = r''  
}$

  

$\begin{cases}  
\mathsf{m \cdot x'' = 0} \\  
\mathsf{m y'' = - m \cdot g}  
\end{cases}$

  

$\begin{cases}  
\mathsf{mx' = C_1} & \mathsf{mx = ct + c_1} \\  
\mathsf{my' = -mgt + \overset{\sim} c} & \mathsf{my = -\dfrac{mgt^2} 2 + \overset{\sim}ct + \overset{\sim} c_1}  
\end{cases}$

  

$\mathsf{  
\overline V = \left\{|V| \cdot \cos(\alpha),\ |V| \cdot \sin(\alpha)\right\}  
}$

  

$\mathsf{  
\begin{cases}  
\mathsf{x(0) = 0} & \mathsf{x'(0) = |V| \cos(\alpha)} \\  
\mathsf{y(0) = 0} & \mathsf{y'(0) = |V| \sin(\alpha)}  
\end{cases}  
}$

  

$\mathsf{  
x = \dfrac{|V|} m \cos(\alpha t)  
}$

  

$\mathsf{  
\overline a =  
}$

  

  

  

  

$\mathsf{  
M_1(x) N_1(y) dx = M_2(x) N_2(y) dy  
}$

$\downarrow$

$\mathsf{  
\int \dfrac{M_1(x) dx}{M_2(x)} = \int \dfrac{N_2(y) dy}{N_1(y)}  
}$

  

  

# №2

Найти особые решений

$\mathsf{  
xy \cdot dx + (x + 1) dy = 0  
}$

Решения:

1. $\mathsf{  
    y = 0  
    }$
    1. Можно получить из 3-го, поэтому особым решением не является.
2. $\mathsf{  
    x = -1  
    }$
3. $\mathsf{  
    \int \dfrac{x}{x + 1} = \int - \dfrac{dy} y  
    }$  
      
    $\mathsf{  
    \int (1 - \dfrac 1 {x^2 + 1})dx = - \ln(y)  
    }$  
      
    $\mathsf{  
    x - \ln(x + 1) = - \ln(y) + \ln(C)  
    }$  
      
    $\mathsf{  
    x - \ln(x + 1) = \ln(\dfrac C y)  
    }$  
      
    $\mathsf{  
    x = \ln\left((x + 1) \cdot \dfrac C y\right)  
    }$  
      
    $\mathsf{  
    e^x = (x + 1) \cdot \dfrac C y  
    }$  
      
    $\mathsf{  
    y = C (x + 1) \cdot e^{-x}  
    }$

  

# №3

$\mathsf{  
(y^2 + 1) dx = xy dy  
}$

Решение:

$\mathsf{  
\dfrac{dx} x = \dfrac{y dy}{y^2 + 1}  
}$

$\mathsf{  
\ln(x) = \dfrac 1 2 \ln(y^2 + 1) + \ln(C)  
}$

$\mathsf{  
\ln(x) = \ln(C \cdot \sqrt {y^2 + 1})  
}$

$\mathsf{  
x(y) = C \sqrt{y^2 + 1}  
}$

  

# №4

$\mathsf{  
\begin{cases}  
\mathsf{(x^2 - 1) \dfrac {dy}{dx} + 2xy^2 = 0} \\  
\mathsf{y(0) = 1}  
\end{cases}  
}$

$\mathsf{  
(x^2 - 1) dy = -2xy^2 dx  
}$

$\mathsf{  
\dfrac{dy}{y^2} = \int -\dfrac{2x dx}{x^2 - 1}  
}$

$\mathsf{  
\dfrac 1 y = \ln\left((x^2 - 1)C\right)  
}$

$\mathsf{  
1 = \ln(C)  
}$

$\mathsf{  
C = e  
}$

  

# №5

$\begin{cases}  
\mathsf{y' \cdot \ctg(x) + y = 2} \\  
\mathsf{y(x) \to -1 \text{ при } x \to 0}  
\end{cases}$

$\mathsf{  
y = 2  
}$

$\mathsf{  
\int \dfrac{dy}{2 - y} = \int\tg(x) dx  
}$

$\mathsf{  
- \ln(y - 2) = - \ln |\cos(x)| - C  
}$

$\mathsf{  
y = C \cos(x) + 2  
}$

$\mathsf{  
-1 = A + 2 \implies A = - 3  
}$

  

# №6

$\begin{cases}  
\mathsf{x y' + y = y^2} \\  
\mathsf{y(1) = 0.5}  
\end{cases}$