---
Owner: Artemii
tags:
  - Практика
---
# №1. Линейное неоднородное

## Условия

$\mathsf{  
(2x + 1) y' = 4x + 2y  
}$

## Решения

### Пояснения

$\mathsf{  
y' + p(x) y = q(x)  
}$

$\mathsf{  
y = z + v  
}$

$\mathsf{  
z'p(x)z = q(x)  
}$

*

$\mathsf{  
v' + p(x)v = 0  
}$

### Решение методом Лагранжа

$\mathsf{  
y' - \dfrac 2 {2x + 1} y = \dfrac{4x}{2x + 1}  
}$

1. Общее однородное
    
    $\mathsf{  
    y' - \dfrac{2y}{2x + 1} = 0  
    }$
    
    $\mathsf{  
    y' = \dfrac 2 {2x + 1} y  
    }$
    
    $\mathsf{  
    \dfrac {dy}y = \dfrac {2dx}{2x + 1}  
    }$
    
    $\mathsf{  
    \ln(y) = \ln(2x + 1) + \ln(C)  
    }$
    
    $\mathsf{  
    y = C(2x + 1)  
    }$
    
2. Пусть C - функция
    
    $\mathsf{  
    y = C(x) \cdot (2x + 1)  
    }$
    
    $\mathsf{  
    y' = C(x) \cdot (2x + 1) + 2C(x)  
    }$
    
    $\mathsf{  
    (2x + 1)(C' \cdot (2x + 1) + 2C) = 4x + 2C(2x + 1)  
    }$
    
    $\mathsf{  
    C' (2x + 1)^2 = 4x  
    }$
    
    $\mathsf{  
    C' = \dfrac{4x}{(2x + 1)^2}  
    }$
    
    $\mathsf{  
    C(x) = \ln(2x + 1) - \dfrac{1}{2x + 1} + \overline C  
    }$
    
    $\mathsf{  
    y = (2x + 1)(\ln(2x + 1) + \dfrac 1 {2x + 1} + \overline C)  
    }$
    

### Решение методом Бернулли

1. Частное неоднородное
    
    $\mathsf{  
    y' - \dfrac 2{2x + 1} y = \dfrac{4x}{2x + 1}  
    }$
    
    $\mathsf{  
    y = uv \quad y' = u' v + uv'  
    }$
    
    $\mathsf{  
    u'v + uv' - \dfrac 2 {2x + 1} uv = \dfrac {4x}{2x + 1}  
    }$
    
    $\mathsf{  
    \begin{cases}  
    \mathsf{v(u' - \dfrac 2 {2x + 1} u) = 0} \\  
    \mathsf{uv' = \dfrac{4x}{2x + 1}}  
    \end{cases}  
    }$
    
    $\mathsf{  
    \dfrac{u'} u = \dfrac 2 {2x + 1}  
    }$
    
    $\mathsf{  
    \ln(u) = \ln(2x + 1) + \ln(C)  
    }$
    
    $\mathsf{  
    u = C (2x + 1)  
    }$
    
    $\mathsf{  
    (2x + 1) v' = \dfrac{4x}{2x + 1}  
    }$
    
    $\mathsf{  
    v' = \dfrac{4x}{(2x + 1)^2}  
    }$
    
    $\mathsf{  
    v = \ln(2x + 1) + \dfrac 1 {2x + 1} + C  
    }$
    

## Особые решения

1. $\mathsf{  
    x = - \dfrac 1 2  
    }$

  

$\mathsf{y'+2y=y^2 e^x}$

$\mathsf{y=u\cdot v}$

$\mathsf{u'v+uv'+2uv=u^2 v^2 e^x}$

$\mathsf{u(v'+2v) = 0}$

$\mathsf{v'+2v = 0}$

$\mathsf{v = C \cdot e^{-2x}}$

$\mathsf{u'=u^2 e^{-x}}$

$\mathsf{- \dfrac 1 u = -e^{-x} - C}$

$\mathsf{u=\dfrac{1}{e^{-x}+C}}$

  

  

# №1

$\mathsf{  
y' + t \tg(x) = \sec(x)  
}$

$\mathsf{  
y' + y \tg(x) = 0  
}$

$\mathsf{  
\ln(y) = \ln(\cos(x)) + \ln(C)  
}$

$\mathsf{  
y = \cos(x)C  
}$

$\mathsf{  
y = C(x) \cos(x)  
}$

$\mathsf{  
y' = -\sin(x) C(x) + \cos(x) C'(x)  
}$

$\mathsf{  
\cos(x) C'(x) - \sin(x) C(x)  
}$

  

  

**Домашнее задание:**

139-144

147-150