# Условие
Найти минимум функции в пространстве $\mathbb{R}^{n}$ методом градиентного спуска

$f_{0}(x) = \frac{1}{2}\left( x^{T} Ax \right) + b \cdot x$
$g(x) = ||x - x_{0}|| - r$
	Предположим, что $g(x) = 0$
$A = 3 \times 3$. Невырожденная

# Решение
## Неудачное решение
Пусть $A = \begin{pmatrix}1 & 0 & 0 \\ 0 & 1 & 0 \\ 1 & 1 & 2\end{pmatrix}  \quad b = \begin{pmatrix}1 & 1 & 1\end{pmatrix}$
$\sqrt{ (x - x_{0}) } - r \leq 0$
$\sqrt{ (x - x_{0}) } \leq r$
$x - x_{0} - r^{2} \leq 0$

$f(x) = \frac{1}{2}\left( x_{1}x_{3} + x_{2}^{2} + x_{1}^{2} \right) + x_{3}^{2} + x_{3} + x_{2} + x_{1}$
$L(\lambda, x) = \frac{1}{2}\left( x_{1}x_{3} + x_{2}^{2} + x_{1}^{2} \right) + x_{3}^{2} + x_{3} + x_{2} + x_{1} + \lambda \left( \left[ \left( x_{1} - p_{1} \right)^{2} + \left( x_{2} - p_{2} \right)^{2} + \left( x_{3} - p_{3} \right)^{2} \right] - r^{2} \right)$

$$
\nabla L(\lambda, x) = \begin{cases}
\dfrac{\partial F}{\partial \lambda} = \left[ \left( x_{1} - p_{1} \right) ^{2} + \left( x_{2} - p_{2} \right) ^{2} + \left( x_{3} - p_{3} \right) ^{2} \right] - r^{2}  \\
\dfrac{\partial F}{\partial x_{1}} = \frac{1}{2}x_{3} + x_{1} + 1 + 2\lambda x_{1} - 2\lambda p_{1} \\
\dfrac{\partial F}{\partial x_{2}} = x_{2} + 1 +2\lambda x_{2} - 2\lambda p_{2} \\
\dfrac{\partial F}{\partial x_3} = \frac{1}{2}x_{1} + 2x_{3} + 1 + 2\lambda x_{3} - 2\lambda p_{3}
\end{cases}
$$
$$
\nabla L(\lambda, x) =  0
$$

$$
\begin{cases}
\left[ (x_{1} - p_{1})^{2} + \left( x_{2} - p_{2} \right) ^{2} + \left( x_{3} - p_{3} \right) ^{2} \right] - r^{2} = 0 \\

\end{cases}
$$

## Второе решение
$$
A = \begin{pmatrix}
1 & 0 & 0 \\
0 & 1 & 0 \\
0 & 0 & 1
\end{pmatrix} \quad b = \begin{pmatrix}
1 & 1 & 1
\end{pmatrix} 
$$
$\sqrt{ (x - x_{0}) } - r = 0$
$\sqrt{ (x - x_{0}) } = r$
$x - x_{0} - r^{2} = 0$

$f(x) = \frac{1}{2}\left( x_{1}^{2} + x_{2}^{2} + x_{3}^{2} \right) + x_{1} + x_{2} + x_{3}$
$L(\lambda, x) =  \frac{1}{2}\left( x_{1}^{2} + x_{2}^{2} + x_{3}^{2} \right) + x_{1} + x_{2} + x_{3} + \lambda \left( \left[ \left( x_{1} - p_{1} \right)^{2} + \left( x_{2} - p_{2} \right)^{2} + \left( x_{3} - p_{3} \right)^{2} \right] - r^{2} \right)$
$x_{0} = \begin{pmatrix}0 \\ 0 \\ 0\end{pmatrix} \quad r = \sqrt{ 3 }$
$$
\nabla L(\lambda, x) = \begin{pmatrix}
x_{1}^{2} + x_{2}^{2} + x_{3}^{2} - r^{2} \\
x_{1} + 1 + 2\lambda x_{1} \\
x_{2} + 1 + 2\lambda x_{2} \\
x_{3} + 1 + 2\lambda x_{3}
\end{pmatrix}
$$

