# Условие
$f(x) = \frac{1}{2}\left( x^{T} A x \right) + b  x$
$g \leq 0  \quad  g(x) = ||x - x_{0}|| - r$

# Решение
$$
A = \begin{pmatrix}
1 & 0 & 2 & 0 \\
0 & 1 & 0 & 0 \\
2 & 0 & 1 & 0 \\
0 & 0 & 0 & 1
\end{pmatrix}
$$
$$b = \begin{pmatrix}1 & 1 & 1 & 1\end{pmatrix}$$

$\sqrt{ (x - x_{0}) } - r \leq 0$
$\sqrt{ (x - x_{0}) } \leq r$
$x - x_{0} - r^{2} \leq 0$

$$
f(x) = \frac{1}{2}\left( x_{4}^{2} + x_{3}^{2} + x_{2}^{2} + x_{1}^{2} \right) + 2x_{1}x_{3} + x_{4} + x_{3} + x_{2} + x_{1}
$$
$$
F(x) = \left[ \frac{1}{2}\left( x_{4}^{2} + x_{3}^{2} + x_{2}^{2} + x_{1}^{2} \right) + 2x_{1}x_{3} + x_{4} + x_{3} + x_{2} + x_{1} \right] + \lambda \left[ { \sum \limits_{ i=1 }^{ n } \left( x_{i} - p_{i} \right) ^{2} } - r^{2} \right]  
$$
$$
\begin{cases}
\dfrac{\partial F}{\partial x_{1}} = (2\lambda + 1)x_{1} + 2x_{3} - 2\lambda p_{1} + 1= 0 \\
\dfrac{\partial F}{\partial x_{2}} = (2\lambda + 1)x_{2} - 2\lambda p_{2} + 1 = 0 \\
\dfrac{\partial F}{\partial x_{3}} = (2\lambda + 1)x_{3} + 2x_{1} - 2\lambda p_{3} + 1 = 0 \\
\dfrac{\partial F}{\partial x_{4}} = (2\lambda + 1)x_{4} - 2\lambda p_{4} + 1 \\
\dfrac{\partial F}{\partial \lambda} = {x_{4}}^{2}-2\,p_{4}\,x_{4}+{x_{3}}^{2}-2\,p_{3}\,x_{3}+{x_{2}}^{2}-2\,p_{2}\,x_{2}+{x_{1}}^{2}-2\,p_{1}\,x_{1}-{r}^{2}+{p_{4}}^{2}+{p_{3}}^{2}+{p_{2}}^{2}+{p_{1}}^{2} = 0
\end{cases}
$$
$$
H = \begin{pmatrix}
(2\lambda + 1) & 0 & 2 & 0 & 2x_{1}-2p_{1} \\
0 & (2\lambda + 1) & 0 & 0 & 2x_{2} - 2p_{2} \\
2 & 0 & (2\lambda + 1) & 0 & 2x_{3} - 2p_{3} \\
0 & 0 & 0 & (2\lambda + 1) & 2x_{4} - 2p_{4} \\
2x_{1} - 2p_{1} & 2x_{2} - 2p_{2} & 2x_{3} - 2p_{3} & 2x_{4} - 2p_{4} & 0
\end{pmatrix}
$$

