---
Редакторы: Artemii
Тэги:
  - II семестр
  - Практика
Дата: 2023-02-06
Статус: В процессе
---
1. $\mathsf  
    {  
    u = 3 \cdot x^3 \cdot y^4 + \sqrt{x} \cdot \sqrt[3]{y} + \sin(x + 2 y)  
    }$
    1. Считаем $\mathsf y$ за $\mathsf{const}$
    2. $\mathsf{u'_x = 9 \cdot x^2 \cdot y^4 + \dfrac{1}{2 \sqrt x} \cdot \sqrt[3] y + \cos(x + 2y) \cdot 1  
        }$
    3. $\mathsf  
        {  
        u_y' = 12 \cdot x^3 \cdot y^3 + \sqrt x \cdot \dfrac{1}{3 \sqrt[3]{y^2}} + \cos(x + 2y) \cdot 2  
        }$

$\mathsf  
{  
u_x' = \dfrac {\sigma u}{\sigma x}  
}$

$\mathsf  
{  
u_x' = \dfrac {du}{dy}  
}$

$\mathsf  
{  
\dfrac{\sigma }{\sigma x} \left(f(x, y)\right)  
}$

  

1. $\mathsf  
    {  
    u = \arctg \dfrac y x  
    }$
    1. $\mathsf  
        {  
        u'_x = \dfrac {-1} {1 + (\dfrac y x)^2} \cdot \dfrac{y}{x^2}  
        }$
    2. $\mathsf  
        {  
        u_y' = \dfrac{1}{1 + (\dfrac y x)^2} \cdot \dfrac 1 x  
        }$
2. $\mathsf  
    {  
    u = x^y  
    }$
    1. $\mathsf  
        {  
        \dfrac {\sigma u}{\sigma x} = y \cdot x^{y - 1}  
        }$
    2. $\mathsf{  
        \dfrac {\sigma u}{\sigma y} = x^y \cdot \ln(x)  
        }$

  

  

  

  

  

  

$\mathsf  
{  
x \dfrac{\sigma u}{\sigma x} + y \dfrac{\sigma u}{\sigma y} = 2  
}$

1. $\mathsf  
    {  
    u = \ln(x^2 + xy + y^2)  
    }$
    1. $\mathsf  
        {  
        \dfrac{\sigma u}{\sigma x} = \dfrac {1}{x^2 + x6 + y^2} \cdot (2x + y)  
        }$
    2. $\mathsf  
        {  
        \dfrac {\sigma u}{\sigma y} = \dfrac{1}{x^2 + xy + y^2} \cdot (x + 2y)  
        }$
    3. $\mathsf  
        {  
        \dfrac{x(2x + y)}{x^2 + xy + y^2} + \dfrac {y(x + 2y)}{x^2 + xy + y^2} = \dfrac{2x^2 + xy + yx + 2y^2}{x^2 + xy + y^2} = 2  
        }$

  

  

  

$\mathsf  
{  
u = f(x, y)  
}$

$\mathsf  
{  
du = u_x' \cdot dx + u_y' \cdot dy  
}$

$\mathsf  
{  
u'_x \neq \dfrac {du}{dx}  
}$

$\mathsf  
{  
u'_x = \dfrac {\sigma u}{\sigma x}  
}$

$\mathsf  
{  
\vartriangle u = \dfrac {\sigma u}{\sigma x_1} \cdot \vartriangle x_1 + \ldots + \dfrac{\sigma u}{\sigma x_m} + 0(\vartriangle \rho)  
}$

  

1. $\mathsf  
    {  
    u = y \cdot x^y  
    }$
    1. $\mathsf  
        {  
        u'_x = y^2 \cdot x^{y - 1}  
        }$
    2. $\mathsf  
        {  
        u'_y = y \cdot x^y \cdot \ln(x) + 1 \cdot x^y  
        }$
    3. $\mathsf  
        {  
        du = y^2 \cdot x^{y - 1} dx + (y \cdot x^y \cdot \ln(x) + 1 \cdot x^y) dy  
        }$

  

  

$\mathsf  
{  
df (3, 4, 5) - ?  
}$

$\mathsf  
{  
f(x, y, z) = \dfrac{z}{\sqrt{x^2 + y^2}}  
}$

$\mathsf  
{  
\dfrac{\sigma f}{\sigma x} = -\dfrac{xz}{(x^2 + y^2)^{\frac 3 2}}  
}$

$\mathsf  
{  
\dfrac{\sigma f}{\sigma y} = -\dfrac {yz}{(x^2 + y^2)^{\frac 3 2}}  
}$

$\mathsf  
{  
\dfrac{\sigma f}{\sigma z} = \dfrac{1}{(x^2 + y^2)^{\frac 1 2}}  
}$

$\mathsf  
{  
df = -\dfrac{xz dx}{(x^2 + y^2)^\frac 3 2} - \dfrac{yz dy}{(x^2 + y^2)^\frac 3 2} + \dfrac{dz}{(x^2 + y^2)^\frac 1 2}  
}$

$\mathsf  
{  
df(3, 4, 5) = \dfrac 1 {25} (-3dx - 4dy + 5dz)  
}$