---
Редакторы: Artemii
Тэги:
  - II семестр
  - Практика
Дата: 2023-11-04
Статус: Готово
---
$\mathsf  
{  
\int \frac{P_n(x) dx}{\sqrt{ax^2 + bx + c}} = Q_{n - 1}(x) \cdot \sqrt{ax^2 + bx + c} + \alpha\int \frac{dx}{\sqrt{ax^2 + bx + c}}  
}$

  

1. $\mathsf  
    {  
    \int \frac{x^3 - 6x^2 + 11x - 6}{\sqrt{x^2 + 4x + 3}}dx = (Ax^2 + Bx + C) \cdot \sqrt{x^2 + 4x + 3} + \alpha \int \frac{dx}{\sqrt{x^2 + 4x + 3}}  
    }$
    1. $\mathsf  
        {  
        \frac{x^3 - 6x^2 + 11x - 6}{\sqrt{x^2 + 4x + 3}} = (2Ax + B)\sqrt{x^2 + 4x + 3} + (Ax^2 + Bx + C)\cdot \frac{2x + 4}{2\sqrt{x^2 + 4x + 3}} + \frac{\alpha}{\sqrt{x^2 + 4x + 3}}  
        }$
    2. $\mathsf  
        {  
        \frac{x^3 - 6x^2 + 11x - 6}{\sqrt{x^2 + 4x + 3}} = \frac{(2Ax + B)(x^2 + 4x + 3) + (Ax^2 + Bx + C)(x + 2) + \alpha}{\sqrt{x^2 + 4x + 3}}  
        }$
    3. Далее всё по стандарту
2. $\mathsf  
    {  
    \int \frac{dx}{x^4 \cdot \sqrt{x^2 + 1}} =  
    \begin{vmatrix}  
    \mathsf{t = \frac 1 x} & \mathsf{x = \frac 1 t} \\  
    \mathsf{dx = \frac{-dt}{t^2}}  
    \end{vmatrix} =  
    - \int \frac{dt}{t^2 \cdot \frac 1 {t^4} \cdot \sqrt{\frac 1 {t^2} + 1}} = -\int \frac{t^3}{\sqrt{1 + t^2}}dt =  
    }$
    1. $\mathsf  
        {  
        (At^2 + Bt + C) \sqrt{1 + t^2} + \alpha \int \frac{dt}{\sqrt{1 + t^2}}  
        }$
    2. $\mathsf  
        {  
        -\frac{t^3}{\sqrt{1 + t^2}} = (2A + B) \sqrt{1 + t^2} + (At^2 + Bt + C) \frac{2t}{2\sqrt{1 + t^2}} + \frac{\alpha}{\sqrt{1 + t^2}}  
        }$
    3. $\mathsf  
        {  
        -t^3 = (2At + B)(1 + t^2) + (At^2 + Bt + C)t + \alpha  
        }$
    4. $\ldots$
    5. $\mathsf  
        {  
        =(-\frac{t^2}{3} +\frac 2 3) \sqrt{1 + t^2} = (-\frac 1 {3x^2} + \frac 2 3) \sqrt{1 + \frac 1 {x^2}} + C  
        }$
3. $\mathsf  
    {  
    \int \frac{dx}{(x - 1)^3\cdot \sqrt{x^2 + 3x + 1}} =  
    \begin{vmatrix}  
    \mathsf{t = \frac 1 {x - 1}} & \mathsf{x = \frac 1 t + 1} \\  
    \mathsf{dx = -\frac{dt}{t^2}}  
    \end{vmatrix} =  
    \int \frac{dt}{t^2(\frac 1 t + 1 - 1)^3 \cdot \sqrt{(\frac 1 t + 1)^2 + 3 (\frac 1 t + 1) + 1}} = - \int \frac{dt}{t^2 \cdot \frac 1 {t^3} \cdot \sqrt{\frac 1 {t^2} + \frac 5 t + 5}}  
    }$
    1. $\mathsf  
        {  
        - \int \frac{t^2 dt}{\sqrt{1 + 5t + 5t^2}} = (At + B) \sqrt{5t^2 + 5t + 1} + \alpha \int \frac{dt}{\sqrt{5t^2 + 5t + 1}}  
        }$
    2. $\ldots$
4. $\mathsf  
    {  
    \int  
    }$