---
Редакторы: Artemii
Тэги:
  - II семестр
  - Практика
Статус: В процессе
---
$\mathsf  
{  
F(x, y, z) = 0  
}$

$\mathsf  
{  
z = z(x, y)  
}$

Если в $(\cdot)  
\mathsf  
{  
M_0(x_0, y_0, z_0)  
}$ частная производная: $\mathsf{F'_z(M_0) \neq 0}$, то $\mathsf  
{  
z'_x(M_0) = -\dfrac{F'_x(M_0)}{F'_z(M_0)}; \quad z'_y(M_0) = -\dfrac{F'_y(M_0)}{F'_z(M_0)}  
}$

  

**==№1==**

$\mathsf{x^2+y^2+z^2-2xz=2; \ M_0(0;1;-1)}$

$\mathsf{Z'_x(M_0),\ Z'_y(M_0) - ?}$

$\mathsf{x^2+y^2+z^2-2xz - 2 = 0}$

  

$\mathsf  
{  
\begin{matrix}  
\mathsf{F'_x = 2x - 2z} & \mathsf{F'_x(M_0) = 2} \\  
\mathsf{F'_y = 2y} & \mathsf{F'_y(M_0) = 2}  
\end{matrix}  
}$

$\mathsf  
{  
z'_x(M_0) = -\dfrac{2}{-2} = 1  
}$

$\mathsf  
{  
z'_y(M_0) = -\dfrac 2 {-2} = 1  
}$

$\mathsf  
{  
F'_z = 2z - 2x  
}$

$\mathsf  
{  
F'_z(M_0) = -2 \neq 0  
}$

$\mathsf{F(x,y) = 0}$

$\mathsf{\dfrac{dy}{dx} = \dfrac{f'_x(x,y)}{f'_y(x,y)}}$

  

==**№2**==

$\mathsf  
{  
\dfrac{x^2}{a^2} + \dfrac{y^2}{b^2} - 1 = 0  
}$

$\mathsf  
{  
F'_x = \dfrac{2x}{a^2}  
}$

$\mathsf  
{  
F'_y = \dfrac{2y}{b^2}  
}$

$\mathsf  
{  
\dfrac{dy}{dx} = -\dfrac{x \cdot b^2}{a^2 \cdot y}  
}$

$\mathsf  
{  
\dfrac{d^2 y}{dx^2} = -\dfrac{b^2 a^2 y - xb^2 \cdot a^2 \cdot y}{a^4 \cdot y^2} = -\dfrac{b^2 a^2 y^2 + x^2 b^4}{a^4 y^3}  
}$

  

==**№3**==

$\mathsf{x^2+y^2 -z^2 -xy+yz=0}$

$\mathsf  
{  
\dfrac{\partial z}{\partial x}; \dfrac{\partial z}{\partial y}; \dfrac{\partial^2 z}{\partial x^2}; \dfrac{\partial^2 z}{\partial x \partial y}; \dfrac{\partial ^2 z}{\partial y^2}  
}$

$\mathsf  
{  
F'_x(x,y,z) = 2x-y  
}$

$\mathsf{F'_y (x,y,z)=2y-x+z}$

$\mathsf{F'_z(x,y,z) = -2z+y}$

$\mathsf  
{  
\dfrac{\partial z}{\partial x} = -\dfrac{F'_x}{F'_z} = - \dfrac{2x - y}{-2z + y} = \dfrac{2x - y}{2z - y}  
}$

  

$\mathsf{\dfrac{\partial z}{\partial y} = \dfrac{F'_y}{F'_z}=\dfrac{2y-x+z}{2z-y}}$

  

  

$\mathsf  
{  
\dfrac{\partial^2 z}{\partial x \partial y} = \dfrac{-(2z-y)-(2x-y)(2\dfrac{2y-x+z}{2z-y}-1)}{(2z-y)^2} =  
}$

$\mathsf{= \dfrac{-(2z-y)^2-(2x-y)(2(2y-z+z)-(2z-y))}{(2z-y)^3} =}$

$\mathsf{\dfrac{-(2z-y)^2-(2x-y)(5y-2x)}{(2z-y)^2}}$

$\mathsf  
{  
\dfrac{\partial^2 z}{\partial x^2} = \dfrac{2(2z - y)^2 - 2(2x - y)^2}{(2z - y)^3}  
}$

  

$\mathsf{\dfrac{\partial^2z}{\partial y^2} = \dfrac{(2+Z'_y)(2z-y)-(2Z'_y-1)(2y-x+z)}{(2z-y)^2}}$