---
Редакторы: ArtemiiVandevald
Тэги:
  - II семестр
  - Практика
Статус: В процессе
---
$\mathsf  
{  
f(M) = f(M_0) + \dfrac{1}{1!} df(M_0) + \dfrac{1}{2!} d^2 f(M_0) + \ldots + \dfrac{1}{n!} d^n f(M_0) + R_n  
}$

$\mathsf  
{  
f(x, y) = f(x_0, y_0) + f'_x ( x_0, y_0) \cdot (x - x_0) + f'_y (x_0, y_0) \cdot (y - y_0) +  
}$

$\mathsf  
{  
+ \dfrac{1}{2} (f_{xx}'' (x_0, y_0) \cdot (x - x_0)^2 + 2 f_{xy}'' (x_0), y_0) \cdot (x - x_0)\cdot(y - y_0) + f_{yy}''(x_0, y_0) \cdot (y - y_0)^2) + R_2  
}$

==**1)**== $\mathsf{f(x,y) =x^3 -5x^2-xy-y^2 + 10 x + 5y; \quad M_0(2;-1)}$

  

$\mathsf{f(2;-1) = 8 - 20 + 2 - 1 + 20 -5 = 4}$

$\mathsf{f'_x = 3x^2 -10x - y + 10}$

$\mathsf{f'_x(2;-1) = 12-20 +1+10 = 3}$

$\mathsf{f;_y = -x -2y + 5}$

$\mathsf{f'_y(2;-1)= -2 + 2 + 5 = 5}$

$\mathsf{f_{x}'' = 6x-10; \quad f_{x}''(2;-1) = 2}$

$\mathsf{f_{xy}'' = - 1; \quad f_{yy}'' = -2; \quad f_{xxx}''' = 6 }$

  

$\mathsf{f(x,y) = 4 + 3(x-2) + 5 (y+1)+\dfrac{1}{2}(2(x-2)^2+2(-1)(x-2)(y+1)-2(y+1)^2)+ \dfrac{1}{6} 6(x-2)^3}$$\mathsf{f(x,y) = 4 + 3(x-2) +5(y+1)+(x-2)^2- (x-2)(y+1)-(y+1)^2}+(x-2)^3$

  

==**2)**== $\mathsf  
{  
f(x, y) = e^{x + 2y}; \quad M_0(1; -1)  
}$

  

2) Формула Тэйлора до 3-го порядка влючительно

$\mathsf  
{  
f(1; -1) = e^{1- 2} = e^{-1} = \dfrac 1 e  
}$

$\mathsf  
{  
f'_x = e^{x + 2y} \quad f'_x(1; -1) = \dfrac 1 e  
}$

$\mathsf  
{  
f'_y = e^{x + 2y} \cdot 2 \quad f'_y(1; -1) = \dfrac 2 e  
}$

$\mathsf  
{  
f''_{xx} = e^{x + 2y} \quad f_xx''(1; -1) = \dfrac 1 e  
}$

$\mathsf  
{  
f''_{xy} = 2e^{x + 2y} \quad f''_{xy} (1; -1) = \dfrac 2 e  
}$

  

$\mathsf  
{  
f''_{yy} = 4 e^{x + 2y} \quad f''_{yy} (1; -1) = \dfrac 4 e  
}$

$\mathsf  
{  
f'''_{xxx} = e^{x + 2y} \quad f'''_{xxx}(1; -1) = \dfrac 1 e  
}$

$\mathsf  
{  
f'''_{xxy} = 2e^{x + 2y} \quad f'''_{xxy} (1; -1) = \dfrac 4 e  
}$

$\mathsf  
{  
f'''_{xyy} = 4e^{x + 2y} \quad f'''_{xyy} (1; -1) = \dfrac 4 e  
}$

$\mathsf  
{  
f'''_{yyy} = 8e^{x + 2y} \quad f'''_{yyy}(1; -1) = \dfrac 8 e  
}$

$\mathsf  
{  
f(x, y) = \dfrac 1 e + \dfrac 1 e(x - 1) + \dfrac 2 e(y + 1) +} \\  
\mathsf{+ \dfrac 1 {2e} (x - 1)^2 + \dfrac 2 e (x - 1) (y+ 1) +\dfrac 2 e (y + 1)^2 +} \\  
\mathsf{\dfrac 1 {6e} (x - 1)^3 + \dfrac 1 e (x - 1)^2 (y + 1)+ + \dfrac 2 e(x - 1)(y + 1)^2 + \dfrac 4 {3e} (y + 1)^3 + R_3}$

  

3) $\mathsf{\phi(x,y) = y \cdot f(x^2+y^2); }$

$\mathsf{f(u)}$ - дифференцируемая

$\mathsf{y^2 = \dfrac {\partial \phi}{\partial x} + xy \cdot \dfrac{\partial \phi}{\partial y} = x \phi}$

$\mathsf{\dfrac{\partial \phi}{\partial x} = y \cdot f'(u) \cdot 2x}$

$\mathsf{\dfrac{\partial \phi}{\partial y} = f(u) - 2y^2 \cdot f'(x)}$

$\mathsf{2y^3x F'(u) + xy (f(u) - 2y^2 f'(u)) = 2y^3 x f'(u) + y f(u) - 2y^3 x f'(u) = xy f(u) = x \cdot \phi}$

  

  

==**3)**==

$\mathsf  
{  
\phi (x, y) = f(x, y) + \sqrt{xy} \cdot g(\dfrac y x), \quad f(x, y); g (\dfrac y x)  
}$ - дважды дифференцируема.

$\mathsf  
{  
x^2 \cdot \dfrac{\partial^2 u}{ \partial x^2} - y^2 \dfrac{\partial^2 u}{\partial y^2} = 0  
}$

$\mathsf{\dfrac{\partial u}{\partial x} = f'_x(x,y) + \dfrac{\sqrt{y}}{2 \sqrt{x}} \cdot g(\dfrac{y}{x}) + \sqrt{xy} \cdot g'(\dfrac{y}{x})(-y \dfrac{1}{x^2}) =  
}$

$\mathsf  
{  
= f'_x(x, y) + \dfrac {\sqrt y}{2 \sqrt x} \cdot g(\dfrac y x) - x^{- \frac 3 2} \cdot y^\frac 3 2 \cdot g'(\dfrac y x)  
}$

$\mathsf  
{  
\dfrac{\partial ^2 u}{\partial x^2} = f''_{xx}(x, y) - \dfrac{\sqrt y}{4 x^\frac 3 2} \cdot g(\dfrac y x) + \dfrac {\sqrt y}{2\sqrt x} \cdot g'(\dfrac xy) \cdot( - y \dfrac 1 x^2) + \dfrac 3 2 x^{-\dfrac 5 2} \cdot y^\frac 3 2 \cdot g'(\dfrac y x) - x^{- \frac 3 2} \cdot y^\frac 3 2 \cdot g''(\dfrac y x) \cdot (-y \dfrac 1 {x^2})  
}$

  

  

$\mathsf{\dfrac{\partial^2 u } {\partial y^2} = f_{yy}'' (x,y) - \dfrac{\sqrt{x}}{y} \cdot y^{-\dfrac{3}{2}} \cdot g(\dfrac{y}{x}) + \dfrac{\sqrt{x}}{2\sqrt{y}} g'(\dfrac{y}{x}) \cdot \dfrac{1}{x}}$