---
Номер практики: 10
Редакторы: Artemii
Тэги:
  - II семестр
  - Практика
Статус: Готово
---
$\mathsf  
{  
\int \frac{P(x)}{Q(x)}dx = \frac{P_1(x)}{Q_1(x)} + \int \frac{P_2(x)}{Q_2(x)}dx  
}$

  

1. $\mathsf  
    {  
    \int \frac{xdx}{(x - 1)^2(x + 1)^3} = \frac{Ax^2 + Bx + C}{(x - 1)(x + 1)^2} + \int \frac{Dx + E}{(x - 1)(x + 1)} dx = \circ  
    }$
    
    $\mathsf  
    {  
    \frac{x}{(x - 1)^2(x + 1)^3} = \frac{(2Ax + B)(x - 1)(x + 1)^2 - (Ax^2 + Bx + C)((x + 1)^2 + (x - 1) \cdot 2(x + 1)}{(x - 1)^2(x + 1)^3} + \frac{Dx + E}{(x - 1)(x + 1)}  
    }$
    
    $\mathsf  
    {  
    x = (2Ax + B)(X^2 - 1) - (Ax^2 + Bx + C)(3x - 1) + (Dx + F)(x - 1)(x + 1)^2  
    }$
    
    $\mathsf  
    {  
    \begin{matrix}  
    \mathsf{x^4:} & \mathsf{0 = D} && \mathsf{A = - \frac 1 8} \\  
    \mathsf{x^3:} & \mathsf{0 = 2A - 3A + E + D} && \mathsf{B = - \frac 1 8} \\  
    \mathsf{x^2:} & \mathsf{0 = B - 3B + D + E + A} && \mathsf{C = -\frac 1 4} \\  
    \mathsf{x^1:} & \mathsf{1 = -2A + B - 3C + D - E} && \mathsf{D = 0} \\  
    \mathsf{x^0:} & \mathsf{0 = -B + C - E} && \mathsf{E = -\frac 1 8}  
    \end{matrix}  
    }$
    
    $\mathsf  
    {  
    \circ = \frac{-\frac 1 8 x^2 - \frac 1 8 x - \frac 1 4}{(x - 1)(x + 1)^2} + \int \frac{- \frac 1 8}{(x - 1)(x + 1)}dx = \frac{- \frac 1 8 x^2 - \frac 1 8 x - \frac 1 4}{(x - 1)(x + 1)^2} - \frac 1 {16} \ln \left| \frac{x - 1}{x + 1}\right| + C  
    }$
    
2. $\mathsf  
    {  
    \int \frac{dx}{(x^2 + 1)^3} = \frac{Ax^3 + Bx^2 + Cx + D}{(x^2 + 1)^2} + \int \frac{Ex + F}{(x^2 + 1)}dx = \circ  
    }$
    
    $\mathsf  
    {  
    \frac{1}{(x^2 + 1)^3} = \frac{(3Ax^2 + 2Bx + C)(x^2 + 1)^{\cancel {2}} - (Ax^3 + Bx^2 + Cx + D)\cdot 2\cancel{(x^2 + 1)} \cdot 2x}{(x^2 + 1)^{\cancel 4}} + \frac{Ex + F}{x^2 + 1}  
    }$
    
    $\mathsf  
    {  
    1 = (3Ax^2 + 2Bx + C)(x^2 + 1) - (Ax^3 + Bx^2 + Cx + D) \cdot 4x + (Ex + F)(x^4 + 2x^2)  
    }$
    
    $\mathsf  
    {  
    \begin{matrix}  
    \mathsf{x^5:} & \mathsf{0 = E} && \mathsf{A = \frac 3 8} \\  
    \mathsf{x^4:} & \mathsf{0 = 3A - 4A + F} && \mathsf{B = 0} \\  
    \mathsf{x^3:} & \mathsf{0 = 2B - 4B + 2E} && \mathsf{C = \frac 5 8} \\  
    \mathsf{x^2:} & \mathsf{0 = 3A + C - 4C + 2F} && \mathsf{D = 0} \\  
    \mathsf{x^1:} & \mathsf{0 = 2B - 4D + E} && \mathsf{E = 0} \\  
    \mathsf{x^0:} & \mathsf{1 = C + F} && \mathsf{F = \frac 3 8}  
    \end{matrix}  
    }$
    
    $\mathsf  
    {  
    1  
    }$
    
3. $\mathsf  
    {  
    \int \frac{x^2 dx}{(x^2 + 2x + 2)^2} =  
    \frac{Ax + B}{x^2 + 2x + 2} + \int \frac{Cx + D}{x^2 + 2x + 2}dx  
    }$