---
Редакторы: Artemii
Тэги:
  - II семестр
  - Практика
Дата: Invalid date
Статус: В процессе
---
$\mathsf  
{  
\underset{\underset{(x \to - \infin)}{x \to + \infin}} \lim x^{\alpha} \cdot f(x) = k  
}$

1. $\mathsf  
    {  
    \alpha > 1,\quad 0 < k < +\infin  
    }$, сходится
2. $\mathsf  
    {  
    \alpha \le 1,\quad 0 \lt k \lt +\infin  
    }$, расходится

  

  

  

1. $\mathsf  
    {  
    \overset{+\infin} {\underset 1 \int} \dfrac {dx}{\sqrt[3]{2x^5 + x^2}} =  
    \overset{+\infin} {\underset 1 \int} \dfrac {dx}{x^{\frac 5 3} \sqrt[3]{2 + \frac 1 {x^3}}}  
    }$
    1. $\mathsf  
        {  
        \alpha = \dfrac 5 3  
        }$
    2. $\mathsf  
        {  
        \underset{x \to +\infin}\lim x^{\frac 5 3} \cdot \dfrac{1}{x^{\frac 5 3} \cdot \sqrt[3]{2 + \dfrac 1 {x^3}} } = \dfrac 1 {\sqrt[3]{2}} = k  
        }$
    3. $\mathsf{\dfrac 5 3 > 1}$, интеграл сходится
2. $\mathsf  
    {  
    \overset{+\infin} {\underset 1 \int} \dfrac{\sqrt x~ dx}{\sqrt[4]{x^5 + 3x^3 + 4}} = \overset{+\infin} {\underset 1 \int} \dfrac{x^{\frac 1 2}~dx}{x^{\frac 5 4}\cdot \sqrt[4]{1 + \frac 3 {x^2} + \frac 4 5}} =  
    \overset{+\infin} {\underset 1 \int} \dfrac{dx}{x^{\frac 3 4}\cdot\sqrt[4]{1 + \frac 3{x^2} + \frac 4 {x^5}}}  
    }$
    
    1. $\mathsf{\alpha = \dfrac 3 4}$
    2. $\mathsf  
        {  
        \underset{x \to +\infin}\lim{x^{\frac 3 4} \cdot \dfrac{1}{x^{3\frac 3 4}\cdot\sqrt[4]{1 + \frac 3 {x^2} + \frac 4 {x^5}}}} = 1 = k  
        }$
    3. $\mathsf{\dfrac 3 4 < 1}$, интеграл расходится
    
      
    
      
    
      
    
      
    

$\mathsf  
{  
f(x)  
}$ определена на $\mathsf  
{  
[a, b)  
}$, $\mathsf  
{  
\overset b {\underset a \int} f(x) dx = \underset{\epsilon \to +0} \lim \overset{b - \epsilon}{\underset a \int} f(x) dx  
}$

$\mathsf  
{  
f(x)  
}$ определена на $\mathsf  
{  
(a, b]  
}$, $\mathsf  
{  
\overset b {\underset a \int} f(x) dx = \underset{\epsilon \to +0} \lim \overset b {\underset {a + \epsilon} \int} f(x) dx  
}$

$\mathsf  
{  
f(x) \to \infin  
}$ при $\mathsf  
{  
x \to c \in [a, b]  
}$, $\mathsf  
{  
\overset b {\underset a \int} f(x) dx = \overset c {\underset a \int} f(x) dx + \overset b {\underset c \int} f(x) dx  
}$

  

$\mathsf  
{  
\overset 1 {\underset 0 \int} \dfrac{dx}{\sqrt{1 - x^2}} = \underset{\epsilon \to +0} \lim \overset {1 - \epsilon} {\underset 0 \int} \dfrac{dx}{\sqrt{1 - x^2}} = \underset{\epsilon \to +0} \lim (\arcsin(x) \overset {1-\epsilon} {\underset 0 \mid}) = \underset{\epsilon \to +0}\lim(\arcsin(1 - \epsilon) - \arcsin(0)) = \dfrac \pi 2  
}$

$\mathsf  
{  
\sqrt{1 - x^2} = 0  
} \\  
\mathsf{  
x = \pm 1  
}$

  

  

  

$\mathsf  
{  
\overset 2 {\underset 1 \int} \dfrac {dx}{x \ln (x)} = \underset{\epsilon \to +0} \lim \overset 2 {\underset {1 + \epsilon} \int} \dfrac{dx}{x \ln(x)} =  
\begin{vmatrix}  
\mathsf{t = \ln(x)} &  
\mathsf{dt = \dfrac 1 x~ dx} \\  
\mathsf{x = 2} & \mathsf{x = 1+\epsilon}\\  
\mathsf{t = \ln(1 + \epsilon)} & \mathsf{t = \ln(1 + \epsilon)}  
\end{vmatrix} =  
\underset{\epsilon \to +0} \lim \overset {\ln(2)} {\underset {\ln(1 + \epsilon)} \int} \dfrac 1 t~ dt = \underset{\epsilon \to +0}\lim (\ln(t) \overset {\ln(2)} {\underset {\ln(1 + \epsilon)} \mid}) =  
}$

$\mathsf  
{  
= \underset{\epsilon \to +0}\lim (\ln(\ln(1 + \epsilon)) - \ln(\ln(2))) = \ln(\ln(2)) - \ln(0) = +\infin  
}$

  

  

  

## Исследование на сходимость несобственного интеграла

$\mathsf{  
\underset{x \to b - 0} \lim (b - x)^\alpha \cdot f(x) = k  
}$

1. Если $\alpha < 1$ и $\mathsf  
    {  
    0 \le k \lt +\infin  
    }$, то $\mathsf  
    {  
    \overset b {\underset a \int} f(x) dx  
    }$ сходится.
2. Если $\mathsf  
    {  
    \alpha \ge 1  
    }$ и $\mathsf  
    {  
    0 \lt k \le + \infin  
    }$, то $\mathsf  
    {  
    \overset b {\underset a \int} f(x) dx  
    }$ расходится

  

$\mathsf  
{  
\overset 1 {\underset 0 \int} \dfrac{dx}{\sqrt[5]{x^5 + 6x}} = \overset 1 {\underset 0 \int} \dfrac{dx}{x^{\frac 1 5} \cdot \sqrt[5]{x^4 + 6}}  
}$

$\mathsf  
{  
\underset{x \to 0} \lim~ x^{\frac 1 5} \cdot \dfrac{1}{x^{\frac1 5} \cdot (x^4 + 6)^{\frac 1 5}} = \dfrac 1 {6^{\frac 1 5}} = k  
}$

$\mathsf  
{  
\alpha \le \dfrac 1 5 \le 1 \implies  
}$ сходится