---
Редакторы: Artemii
Тэги:
  - II семестр
  - Практика
Статус: В процессе
---
$\mathsf  
{  
grad~ f = (f'_x, f'_y, f'_z)  
}$

$\mathsf  
{  
\dfrac{\partial f}{\partial l} = f'_x \cdot \cos(\alpha) + f'_y \cdot \cos(\beta) + f'_z \cdot \cos(\gamma)  
}$

$\mathsf  
{  
\cos(\alpha) = \dfrac{l_1}{|l|}; \quad \cos(\beta) = \dfrac{l_2}{|l|}; \quad \cos(\gamma) = \dfrac{l_3}{|l|}  
}$

$\mathsf  
{  
u = f(x, y, z) \quad M_0 (x_0, y_0, z_0) \quad \overline l = (l_1, l_2, l_3)  
}$

$\mathsf  
{  
f'_x(M_0) - ? \quad f'_y(M_0) - ? \quad f'_z(M_0) - ? \quad grad~ f(M_0) - ? \quad \dfrac{\partial t}{\partial l} /_{M_0} - ?  
}$

  

1. $\mathsf  
    {  
    f(x, y, z) = \dfrac{x^2 \cdot z}{y - x} \quad M_0(1, 3, 5) \quad l = (2, -3, 1)  
    }$
    1. $\mathsf  
        {  
        f'_x (x, y, z) = \dfrac{2xz(y - x) + x^2z}{(y - x)^2} = \dfrac{2xyz - 2x^2z + x^2z}{(y - x)^2}  
        }$
        1. $\mathsf  
            {  
            f'_x(M_0) = \dfrac{30 - 10 + 5}{4} = \dfrac{25}{4} = 6,25  
            }$
    2. $\mathsf  
        {  
        f'_y(x, y, z) = \dfrac{-x^2 z}{(y - x)^2}  
        }$
        1. $\mathsf  
            {  
            f'_y (M_0) = \dfrac{-5}{4} = -1, 25  
            }$
    3. $\mathsf  
        {  
        f'_z(x, y, z) = \dfrac{x^2}{y - x}  
        }$
        1. $\mathsf  
            {  
            f'_z(M_0) = \dfrac{1}{2} = 0,5  
            }$
    4. $\mathsf  
        {  
        grad~f = (\dfrac{2xyz - 2x^2z + x^2z}{(y - x)^2}; \dfrac{-x^2 z}{(y - x)^2}; \dfrac{x^2}{y - x})  
        }$
    5. $\mathsf  
        {  
        grad~ f(M_0) = (6,25; -1,25; 0,5)  
        }$
    6. $\mathsf  
        {  
        |l| = \sqrt {14}  
        }$
    7. $\mathsf  
        {  
        \cos(\alpha) = \dfrac {2}{\sqrt {14}}; \quad \cos(\beta) = \dfrac{-3}{\sqrt{14}}; \quad \cos(\gamma) = \dfrac{1}{\sqrt{14}}  
        }$
    8. $\mathsf  
        {  
        \dfrac{\partial f}{\partial l}|_{M_0} = 6, 25 \cdot \dfrac{2}{\sqrt {14}} - 1,25 \cdot \dfrac{-3}{\sqrt{14}} + 0,5 \cdot \dfrac{1}{\sqrt{14}} = \dfrac{67}{4 \sqrt{14}}  
        }$

  

  

### Касательная плоскости и нормали

$\mathsf  
{  
z = f(x, y); \quad M_0(x_0, y_0, z_0)  
}$

Касательная плоскости: $\mathsf  
{  
z - z_0 = f'_x (x_0, y_0) \cdot(x - x_0) + f'_y(x_0, y_0) \cdot(y - y_0)  
}$

Нормаль: $\mathsf  
{  
\dfrac{x - x_0}{f'_x(x_0, y_0)} = \dfrac{y - y_0}{f'_y(x_0, y_0)} = \dfrac{z - z_0}{-1}  
}$

$\mathsf  
{  
Ax + By + Cz + D = 0; \quad \overline n = (A, B, C)  
}$

  

1. $\mathsf  
    {  
    z = x^2 + 3y^2 - 5; \quad M_0(-1; 2; 8)  
    }$
    1. $\mathsf  
        {  
        f'_x = 2x;\quad f'_x(-1; 2) = -2  
        }$
    2. $\mathsf  
        {  
        f'_y = 6y; \quad f'_y(-1; 2) = 12  
        }$
    3. Касательная: $\mathsf  
        {  
        z - 8 = -2 \cdot (x + 1) + 12 \cdot (y - 2)  
        }$
        1. $\mathsf  
            {  
            2x - 12y + z + 18 = 0  
            }$
    4. Нормаль:
        1. $\mathsf  
            {  
            \dfrac{x + 1}{-2} = \dfrac{y - 2}{12} = \dfrac{z - 8}{-1}  
            }$

  

Функция заданная неявно $\mathsf  
{  
F(x, y, z) = 0 \quad M_0 (x_0, y_0, z_0)  
}$

Касательная: $\mathsf  
{  
F'_x (M_0) \cdot(x - x_0) + F'_y (M_0) \cdot (y - y_0) + F'_z (M_0) \cdot (z - z_0) = 0  
}$

Нормаль: $\mathsf  
{  
\dfrac{x - x_0}{F'_x(M_0)} = \dfrac{y - y_0}{F'_y(M_0)} = \dfrac{z - z_0}{F'_z(M_0)}  
}$

  

1. $\mathsf  
    {  
    M_0 (2; -1; 3); \quad x^2\cdot y + 2z \cdot x - z^2 \cdot y^2 + 1 = 0  
    }$
    1. Производные
        1. $\mathsf  
            {  
            F'_x = 2xy + 2z \quad F'_x (M_0) = 2  
            }$
        2. $\mathsf  
            {  
            F'_y = x^2 - 2yz^2 \quad F'_y (M_0) = 22  
            }$
        3. $\mathsf  
            {  
            F'_z = 2x - 2zy^2 \quad F'_z (M_0) - 2  
            }$
    2. Касательная
        1. $\mathsf  
            {  
            2 \cdot (x - 2) + 2 \cdot (y + 1) - 2 \cdot (z - 3) = 0  
            }$
        2. $\mathsf  
            {  
            x - 2 + 11 (y + 1) - (z - 3) = 0  
            }$
        3. $\mathsf  
            {  
            x + 11 y - z + 12 = 0  
            }$
    3. Нормаль
        1. $\mathsf  
            {  
            \dfrac{x - 2}{2} = \dfrac{y + 1}{22} = \dfrac{z - 3}{-2}  
            }$

  

$\mathsf  
{  
z = f(x, y); \quad x = x(t); \quad y = y(t); \quad \dfrac{dz}{dt} |_{t = t_0}  
}$

$\mathsf  
{  
\dfrac{dz}{dt} = \dfrac{\partial f}{\partial x} \cdot \dfrac{dx}{dt} + \dfrac{\partial f}{\partial y} \cdot \dfrac{dy}{dt}  
}$

  

$\mathsf  
{  
z = x^y; \quad x = \sin(t); \quad y = \cos(t); \quad t_0 = \dfrac \pi 2  
}$

  

$\mathsf  
{  
\dfrac{\partial z}{\partial x} = y \cdot x^{y - 1} \quad \dfrac{dx}{dt} = \cos(t)  
}$

$\mathsf  
{  
\dfrac{\partial z}{\partial y} = x^y \cdot \ln(x) \quad \dfrac{dy}{dt} = -\sin(t)  
}$

$\mathsf  
{  
\dfrac{dz}{dt} = y \cdot x^{y - 1} \cdot \cos(t) - x^y \cdot \ln(x) \cdot \sin(t)  
}$

$\mathsf  
{  
x_0 = \sin (\dfrac \pi 2) = 1; \quad y_0 = \cos(\dfrac \pi 2) = 0  
}$

$\mathsf  
{  
\dfrac{dz}{dt} \mid_{\frac \pi 2}  
= -1 \cdot 0 \cdot 1 = 0}$