---
Редакторы: Artemii
Тэги:
  - II семестр
  - Практика
Статус: Готово
---
1) $\mathsf  
{  
\int \frac{{^3}\sqrt{1 + {^4}\sqrt x}}{\sqrt x} dx =  
\int x^{-\frac 1 2}(1 + x^{\frac 1 4})^{\frac 1 3}dx =  
\underset{\text{2-й случай}}{\begin{vmatrix}  
\mathsf{z = (a + bx^{\frac 1 4})^{\frac 1 3}} & \mathsf{x = (z^3 - 1)^4} \\  
\mathsf{dz = \ldots} & \mathsf{dx = 4 (z^3 - 1)^3 \cdot 3z^2 \cdot dz}  
\end{vmatrix}} =  
  
}$

$\mathsf  
{  
= \int ((z^3 - 1)^4)^{-\frac 1 2} \cdot z \cdot 4(z^3 - 1)^3 \cdot 3z^2 \cdot dz = 12 \int (z^3 - 1) \cdot z^3 \cdot dz =  
}$

$\mathsf  
{  
= 12 \int (z^6 - z^3) \cdot dz = 12 (\frac{z^7}{7} - \frac{z^4} 4) + C =  
12(\frac{(1 + x^\frac{1}{4})^\frac{7}{3}}{7} - \frac{(1 + x^\frac{1}{4})^\frac{4}{3}}{4}) + C  
}$

  

---

  

2) $\mathsf  
{  
\int \frac{dx}{x^2(2 + x^3)^{\frac 5 3}} = \int x^{-2}(2 + x^3)^{- \frac 5 3}dx =  
\underset{\text{2-й способ}}{  
\begin{vmatrix}  
\mathsf{z = (\frac 2 {x^3} + 1)^{\frac 1 3}} & \mathsf{x = 2^{\frac 1 3}(z^3 - 1)^{- \frac 1 3}} \\  
\mathsf{dx = 2^\frac 1 3 \cdot(-\frac 1 3)(z^3 - 1)^{- \frac 4 3} 3z^2 dz}  
\end{vmatrix}} =  
}$

$\mathsf  
{  
= - \int (\frac 2 {z^3 - 1})^{-\frac 2 3} \cdot (\frac{2z^3}{z^3 - 1}) \cdot 2^\frac 1 3 \cdot \frac 1 3 (z^3 - 1)^{-\frac 4 3} \cdot 3z^2 dz =  
-2^{-2} \int \frac{z^3 - 1}{z^3} dz = -\frac 1 4 z - \frac 1 4 \cdot \frac 1 {4z^4} + C  
}$

  

---

  

3)$\mathsf  
{  
\int \sqrt{x^3 + x^4} dx = \int x^\frac 3 2 (1 + x)^\frac 1 2 dx = \underset{}{\begin{vmatrix}  
\mathsf{z = (\frac 1 x + 1)^\frac 1 2} & \mathsf{x = {(z^2 - 1)}^{-1}} \\  
&\mathsf{dx = -(z^2 - 1)^{-2} \cdot 2z dz}  
\end{vmatrix}} =  
}$

$\mathsf  
{  
= \int(x^3(1 + x))^\frac 1 2 dx = \int x^\frac 3 2 (1 + x)^\frac 1 2dx = \int (\frac {z^2} {z^2 - 1}) ^ \frac 1 2((z^2 - 1)^{-2}\cdot2z)\cdot(\frac 1 {z^2 - 1})^\frac 3 2 dz =  
}$

$\mathsf  
{  
=- \int z (\frac 1 {z^2 - 1})^{\frac 1 2 + \frac 3 2} \cdot (z^3 - 1)^{-2} \cdot2z)dz =  
- \int \frac{2z^2}{(z^2 - 1)^4}dz  
}$