$\begin{cases}x' = x - y \\ y' = y - 4x\end{cases}$

$A = \begin{pmatrix}1 - \lambda & -1 \\ -4 & 1 - \lambda \end{pmatrix}$

$\det A = (1 - \lambda)(1-\lambda) - 4 = 0$
$\lambda_{1} = 3$
$\lambda_{2} = -1$

$\lambda = {3}:$
$\begin{pmatrix}-2 & -1 \\ -4 & -2\end{pmatrix} \cdot \begin{pmatrix}\alpha \\ \beta \end{pmatrix} = 0$

$\begin{cases}-2 \alpha - \beta = 0 \\ -4\alpha - 2\beta = 0 \end{cases}$
$\begin{pmatrix}-\frac{1}{2} \\ 1\end{pmatrix}$

$\lambda = 1:$
$\begin{pmatrix}2 & 1 \\ -4 & 2\end{pmatrix} \cdot \begin{pmatrix}\alpha \\ \beta \end{pmatrix}$
$\begin{pmatrix}\frac{1}2 \\ 1\end{pmatrix}$

$$
\begin{pmatrix}
x \\
y 
\end{pmatrix} = \begin{pmatrix}
-\frac{1}{2} \\
1
\end{pmatrix} C_{1} \cdot e^{3t} + \begin{pmatrix}
\frac{1}{2} \\
1
\end{pmatrix} C_{2} \cdot e^{-1t}
$$