$$
y' + y = \sin(x)
$$
$$
y' + y = 0
$$
$$
\frac{dy}{dx} = -y
$$
$$
dy = -ydx
$$
$$
\int \frac{dy}{y} = \int-dx
$$
$$
\ln(y) = -x + C
$$
$$
y = e^{-x} \cdot C
$$

$$
C = C(x)
$$
$$
y' = C'(x)e^{-x} -e^{-x}C(x)
$$
$$
C'(x)e^{-x} - e^{-x}C(x) + e^{-x}C(x) = \sin(x)
$$
$$
e^{-x}C'(x) = \sin(x)
$$

$C(x) =e^{-x}\left( \frac{e^{x}\sin(x) - \cos(x)e^{x}}{2} + C \right)$


# №1
$$
\begin{cases}
x' = x + 2y \\
y' = x - 5\sin(t)
\end{cases}
$$
Общее однородное очевидно (см. [[Диффуры/Домашние работы/ДЗ 3#№834|ДЗ 3]])

## Частное неоднородное
$$
\begin{matrix}
x = -C_{1}(t) \cdot e^{-t} + 2C_{2}e^{2t} \\
y = C_{1}(t)e^{-t} + C_{2}(t)e^{2t}
\end{matrix}
$$
$$
\begin{matrix}
x' = -C'(t) \cdot e^{-t} + C_{1}(t) e^{-t} + 2C_{2}'(t) e^{2t} + 4C_{2}(t) e^{2t} \\
y' = C_{1}'(t) \cdot e^{-t} - C_{1}(t) e^{-t} + C_{2}'(t)e^{2t} + 2C_{2}(t)e^{2t}
\end{matrix}
$$