$$\begin{cases}
{x''=2x-3y} \\
{y''=x-2y}
\end{cases}$$
$$\begin{cases}
{x''-x+3y=0} \\
{-x+y''+2y=0}
\end{cases}$$
$$
\det\begin{pmatrix}
{\lambda^{2}-2} && {3} \\
{-1} && {\lambda^{2}+2}
\end{pmatrix} = \lambda^{4}-1=0
\implies \lambda_{1,2}=\pm 1\quad \lambda_{3,4}=\pm i
$$
$$
(1) \begin{cases} 
{-\alpha+3\beta=0} \\
{-\alpha+3\beta=0}
\end{cases}\implies\begin{pmatrix}
{3} \\
{1}
\end{pmatrix}
$$

# â„–3
$$
\begin{align}
\begin{cases}
x'' = 3x + 4y \\
y'' = -x - y
\end{cases} \\
\begin{cases}
x'' - 3x - 4y = 0 \\
x + y'' + y = 0
\end{cases}
\end{align}
$$


$$
\begin{vmatrix}
\lambda^{2} - 3 & -4 \\
1 & \lambda^{2} + 1
\end{vmatrix} = (\lambda^{2} - 3)(\lambda^{2} + 1) + 4 = \lambda^{4} - 2\lambda^{2} + 1 = 0
$$
$$
(\lambda^{2} - 1)^{2} = 0
$$
$\lambda_{1, 2} = 1$
$\lambda_{3, 4} = -1$

## $\lambda = 1$
$$
\begin{vmatrix}
-2  & -4 \\
1 & 2
\end{vmatrix}.\ rank = 1
$$
$$
\begin{vmatrix}
qt + w \\
at + s
\end{vmatrix}e^{t}
$$

$$
\begin{align}
x = \left( qt + w \right) e^{t} \\
x' = qe^{t} + \left( qt + w \right) e^{t} \\
x'' = qe^{t} + qe^{t} + \left( qt + w \right) e^{t} \\
x'' = 2qe^{t} + \left( qt + w \right) e^{t}
\end{align}
$$

$$
\begin{align} \\
\ldots \\
y'' = 2ae^{t} +\left( at + s \right) 
\end{align}
$$

