# Теория
$$\begin{cases}
x' = 2x + y \\
y' = 3x + 4y
\end{cases}$$
## Решение в лоб
$$\begin{cases}
x' = 2x + y & y = x' - 2x \\
y' = 3x + 4y & (x' - 2x)' = 3x + 4 x' - 8x
\end{cases}$$
$$
x'' - 2x = 3x + 4x' -  8x
$$
$$
x'' - 6x' + 5x = 0
$$
$$
\lambda^2 - 6\lambda + 5 = 0
$$
$$
\lambda_{1, 2} = \dfrac{6 \pm \sqrt{ 16 }}2 = 3 \pm 2
$$
$$
x = C_{1} e ^t + C_{2} e^{5t}
$$
$$
y = C_{1} e^t + 5C_{2}e^{5t} - 2C_{1} e^t - 2C_{2}e^{5t} = -C_{1}e^t + 3C_{2} e^{5t}
$$
$$
f(t) = \begin{cases}
y = -C_{1} e^t + 3C_{2} e^{5t} \\
x = C_{1}e^t + C_{2}e^{5t}
\end{cases}
$$
## Решение с помощью собственного вектора
$$
A = \begin{pmatrix}
2 & 1 \\
3 & 4
\end{pmatrix} \quad m = \begin{pmatrix}
\alpha \\
\beta
\end{pmatrix}
$$
$$
Am = \lambda m
$$
$$
(A - \lambda E) m = 0
$$
$$
\begin{vmatrix}
2 - \lambda & 1 \\
3 & 4 - \lambda
\end{vmatrix} = (2 - \lambda)(4 - \lambda) - 3 \cdot 1 = 8 - 4\lambda - 2\lambda + \lambda^2 - 3 = 0
$$
$$
\lambda^2 - 6\lambda + 5 = 0
$$
$$
\lambda_{1} = 1 \quad \lambda_{2} = 5
$$
При $\lambda_{1}$:
$$
\begin{pmatrix}
1 & 1 \\
3 & 3
\end{pmatrix} \cdot \begin{pmatrix}
\alpha \\
\beta
\end{pmatrix} = 0
$$
$$
\begin{cases}
\alpha + \beta = 0 & \alpha = -1 \\
3 \alpha + 3 \beta = 0 & \beta = 1
\end{cases}
$$
При $\lambda_{2}:$
$$
\begin{pmatrix}
-3 & 1 \\
3 & -1
\end{pmatrix} \cdot \begin{pmatrix}
\alpha \\
\beta
\end{pmatrix} = 0
$$
$$
\begin{cases}
-3 \alpha + \beta = 0 & \alpha = 3 \\
3 \alpha - \beta = 0 & \beta = 1
\end{cases}
$$
$$\begin{pmatrix}
x \\
y
\end{pmatrix} = 
$$
# Практика
## №1
$$
\begin{cases}
x' = x + z - y \\
y' = x + y - z \\
z' = 2x - y
\end{cases}
$$
$$
A = \begin{pmatrix}
1 & -1 & 1 \\
1 & 1 & -1 \\
2 & -1 & 0
\end{pmatrix}
$$
$$
\begin{vmatrix}
1 - \lambda & -1 & 1 \\
1 & 1 - \lambda & -1 \\
2 & -1 & -\lambda
\end{vmatrix} = -\lambda + 2 \lambda^2 - \lambda^3 - 2 + 2\lambda + 2 - 1 = 0
$$
$$
\lambda = \left\{-1; 1; 2\right\} 
$$
$$
\begin{pmatrix}
2 & -1 & 1 \\
1 & 2 & -1 \\
2 & -1 & 1
\end{pmatrix} \cdot \begin{pmatrix}
\alpha \\
\beta \\
\gamma
\end{pmatrix} = \begin{pmatrix}
0 \\
0 \\
0
\end{pmatrix}
$$
$$\ldots$$
$$
x_{1}^* = \begin{pmatrix}
1 \\
1 \\
1
\end{pmatrix} \quad
x_{2}^* = \begin{pmatrix}
1 \\
-3 \\
-5
\end{pmatrix} \quad
x_{3}^* = \begin{pmatrix}
1 \\
0 \\
1
\end{pmatrix}

$$

$$
\begin{pmatrix}
x \\
y \\
z
\end{pmatrix} = C_{1} \begin{pmatrix}
1 \\
1 \\
1
\end{pmatrix}
e^t + C_{2}
$$
# ДЗ
Нет)