$a_{0}(x)y'' + a_{1}(x)y' + a_{2}(x)y = 0$
1. $y = \alpha(x) \cdot z$
2. $t = \phi(x)$

# 1
$x^{2}y'' - 2xy' + \left( x^{2} + 2 \right)y = 0$

$y' = \alpha' z + \alpha z'$
$y'' = \alpha''z + 2\alpha'z' + \alpha z''$
$x^{2}\left( \alpha''z + 2\alpha'z' + \alpha z'' \right) - 2x\left( \alpha'z + \alpha z' \right) + \left( x^{2} + 2 \right)\alpha \cdot z = 0$
$x\alpha' - \alpha = 0 \implies x\alpha' = \alpha \implies \frac{\alpha'}{\alpha} = \frac{1}{x} \implies \ln(\alpha) = \ln(x) + \ln(C)$
$C = 1$
$\alpha = x$

$x^{3}z''$
