---
Редакторы: Artemii
Тэги:
  - II семестр
  - Практика
Статус: Готово
---
$\mathsf  
{  
\int(\frac{x^5 + x^4 - 8}{x^3 - 4x})dx =  
\int((x^2 + x + 4) + \frac{4x^2 + 16x - 8}{x^3 - 4x})dx  
}$

$\mathsf  
{  
(x^5 + x^4 - 8) / (x^3 - 4x) = x^2 + x + 4  
}$

$\mathsf  
{  
\frac{4x^2 + 16x - 8}{x(x - 2)(x + 2)} = \frac{A}{x} + \frac{B}{x - 2} + \frac{C}{x + 2}  
}$

$\mathsf  
{  
4x^2 + 16x - 8 = A(x^2 - 4) + B(x^2 + 2x) + C(x^2 - 2x)  
}$

$\mathsf  
{  
4x^2 + 16x - 8 = Ax^2 - 4A + Bx^2 + 2Bx + Cx^2 - 2Cx  
}$

$\mathsf  
{  
4x^2 + 16x - 8 = (A + B + C)x^2 + (2B - 2C)x + (-4A)x^0  
}$

$\begin{matrix}  
\mathsf{x^2:} & \mathsf{4 = A + B + C} && \mathsf{x:}& \mathsf{16 = 2b - 2C} && \mathsf{x^0:} & \mathsf{-8 = -4A}  
\end{matrix}$

![[/Untitled 22.png|Untitled 22.png]]

  

---

  

$\mathsf  
{  
\int \frac{3x^2 - 15}{(x - 1)(x^2 + 5x + 6)}dx  
}$

$\mathsf  
{  
\frac{3x^2 - 15}{(x - 1)(x^2 + 5x + 6)} =  
\frac {A}{x + 2} + \frac{B}{x + 3} + \frac{C}{x - 1}  
}$

  

---

  

$\mathsf  
{  
\int \frac{x^2 dx}{(x + 2)^2(x + 4)^2}  
}$

$\mathsf  
{  
x^2 = A(x + 4)^2 + B(x + 2)(x + 4)^2 + C(x + 2)^2 + D(x + 4)(x + 2) ^2  
}$

$\begin{matrix}  
\mathsf{x = -4} & \mathsf{16 = 4C} && \mathsf{C = 4} \\  
\mathsf{x = -2} & \mathsf{4 = A4} && \mathsf{A = 1} \\  
\mathsf{x^3:} & \mathsf{0 = B + D} && \mathsf{B = -D} \\  
\mathsf{x^2:} & \mathsf{1 = A + 10B + C + 8D} && \mathsf{D = 2;\quad B = -2}  
\end{matrix}$

  

---

  

$\mathsf  
{  
\int \frac{2x^2 - 3x - 3}{(x - 1)(x^2 - 2x + 5)}dx  
}$

$\mathsf  
{  
2x^2 - 3x - 3 = A(x^2 - 2x + 5) + Bx(x - 1) + C(x - 1)  
}$

$\begin{matrix}  
\mathsf{x = 1} & \mathsf{-4 = 4A} & \mathsf{A = 1} \\  
\mathsf{x^2:} & \mathsf{2 = A + B} & \mathsf{B = 3} \\  
\mathsf{x:} & \mathsf{-3 = -2A + C - B} & \mathsf{C = 2}  
\end{matrix}$

  

---

  

$\mathsf  
{  
\int \frac{x^3 - 6}{x^4 + 6x^2 + 8} dx =  
\int \frac{x^3 - 6}{(x^2 + 2)(x^2 + 4)} =  
\int (\frac{-x -3}{x^2 + 2} + \frac{2x^3}{x^2 + 4})dx =  
-\frac 1 2 \ln|x^2 + 2| - \frac 3 {\sqrt 2} \arctg \frac x {\sqrt 2} + \ln|x^2 + 4| + \frac 3 2 \arctg \frac x 2 + c  
}$

$\mathsf  
{  
\frac{x^3 - 6}{(x^2 + 2)(x^2 + 4)} = \frac{Ax + B}{x^2 + 2} + \frac{Cx + D}{x^2 + 4}  
}$

$\mathsf  
{  
x^3 - 6 = Ax^3 + 4Ax + Bx^2 + 4B + Cx^3 + 2Cx + Dx^2 + 2D  
}$

$\mathsf  
{  
\begin{matrix}  
\mathsf{x^3:} & \mathsf{1 = A + C} && \mathsf{x^2:} & \mathsf{0 = B + D} \\  
\mathsf{x^1:} & \mathsf{0 = 4A + 2C} && \mathsf{x^0:} & \mathsf{-6 = 4B + 2D}  
\end{matrix}  
}$

$\begin{matrix}  
\mathsf{A = -1} & \mathsf{B = -3} \\  
\mathsf{C = 2} & \mathsf{D = 3}  
\end{matrix}$

  

---

  

$\mathsf  
{  
\int \frac{2x + 7}{(x - 3)^{10}} dx =  
2 \int \frac{x + \frac 7 2}{(x - 3)^{10}}dx =  
2 \int \frac{(x - 3) + 3 + \frac 7 2}{(x - 3)^{10}}dx =  
2 \int (\frac 1 {(x - 3)^9} + \frac {13} {2 (x - 3)^{10}})dx = 2 \frac{(x - 3)^{-8}}{-8} + \frac{2 \cdot 13}{2}\frac{(x - 3)^{-9}}{-9} + C  
}$

  

---

  

$\mathsf  
{  
\int \frac{x^3 + x + 1}{(x^2 + 2)^2} dx = \int (\frac{x}{x^2 + 2} + \frac{-x + 1}{(x^2 + 2)^2})dx =  
\frac{1}{2}\ln|x^2 + 2| - \frac 1 2 \int \frac{d(x^2 + 2)}{(x^2 + 2)^2} + \frac x {2 \cdot 2(x^2 + 2)} + \frac{2 - 1}{2 \cdot 2} \int \frac {dx}{x^2 + 2}  
}$

$\mathsf  
{  
= \frac{x}{4(x^2 + 2)} + \frac 1 {4 \sqrt 2} \arctg \frac x {\sqrt 2} + C  
}$

$\mathsf  
{  
\frac 1 2 \ln |x^2 + 2| + \frac 1 {x^2 + 2} + \frac x {4(x^2 + 2)} + \frac 1 {4 \sqrt 2} \arctg \frac x {\sqrt 2} + C  
}$

  

$\mathsf  
{  
\frac{x^3 + x + 1}{(x^2 + 2)^2} = \frac{Ax + B}{x^2 + 2} + \frac{Cx + D}{(x^2 + 2)^2}  
}$

$\mathsf  
{  
x^3 + x + 1 = Ax^3 + 2Ax + Bx^2 + 2B +Cx + D  
}$

$\mathsf  
{  
\begin{matrix}  
\mathsf{x^3:} & \mathsf{1 = A} && \mathsf{x^2:} & \mathsf{0 = B} \\  
\mathsf{x^1:} & \mathsf{1 = 2A + C} && \mathsf{x^0:} & \mathsf{1 = 2B + D}  
\end{matrix}  
}$

$\begin{matrix}  
\mathsf{A = 1} & \mathsf{B = 0} \\  
\mathsf{C = -1} & \mathsf{D = 1}  
\end{matrix}$

$\mathsf  
{  
I_{k + 1} = \frac x {xkm^2(x^2 + m^2)^k} + \frac{2k - 1}{2km^2} I_K  
}$

$\mathsf  
{  
I_k = \int \frac{dx}{(x^2 + m^2)^k}  
}$

---

  

$\mathsf  
{  
\int \frac{dx}{(1 + x^2)^4} = \frac x {2 \cdot 3(1 + x^2)^3} + \frac{2 \cdot 3 - 1}{2 \cdot 3} \cdot \int \frac{dx}{(1 + x^2)^3} = \frac{x}{6(1 + x^2)^3} + \frac 5 6 (\frac{x}{2 \cdot 2 (1 + x^2)^2} + \frac {2 \cdot 2 - 1}{2 \cdot 2} (\frac x {2 (1 + x^2)} + \frac {2 - 1} 2 \int \frac{dx}{1 + x^2})) =  
}$$\mathsf  
{  
\frac{x}{6(1 + x^2)^3} + \frac 5 6 (\frac x {4(1 + x^2)^2} + \frac 3 4(\frac{x}{2(1 + x^2)} + \frac 1 2 \arctg x)) + C  
}$

  

---

  

$\mathsf  
{  
\int \frac {dx}{\cos(x) + 2 \sin(x) + 3} =  
\begin{vmatrix}  
\mathsf{t = \tg \frac x 2} & \mathsf{x = 2\arctg t} \\  
\mathsf{dx = \frac{2 dt}{1 + t^2}} & \mathsf{\sin x = \frac{2t}{1 + t^2} \quad \cos x = \frac{1 - t^2}{1 + t^2}}  
\end{vmatrix} =  
\int \frac{\frac{2dt}{1 + t^2}}{\frac{1 - t^2}{1 + t^2} + \frac{4t}{1 + t^2} + 3} =  
\int \frac{2dt}{(1 + t^2)(\frac{1 - t^2}{1 + t^2}) + \frac{4t}{1 + t^2} + 3} =  
  
}$$\mathsf  
{  
= \int \frac{2dt}{4 + 2t^2 + 4t} = \int \frac{dt}{t^2 + 2t + 2} =  
\int \frac{d(t + 1)}{(t + 1)^2 + 1} = \arctg(t + 1) + C =  
\arctg|\tg\frac x 2 + 1|  
}$

  

---

  

$\mathsf  
{  
\int \frac{\cos (x) dx}{1 + \cos(x)} =  
\begin{vmatrix}  
\mathsf{t, cosx, x, dx}  
\end{vmatrix} =  
\int \frac{1 - t^2}{(1 + t^2)(1 + \frac{1 - t^2}{1 + t^2})} \cdot \frac {2dt}{1 + t^2} = 2 \int \frac{(1 - t^2)}{1 + t^2 + 1 - t^2}\cdot \frac {dt}{1 + t^2} = \int \frac{1 - t^2}{1 + t^2} dt =  
}$

$\mathsf  
{  
-\int \frac{(t^2 + 1) - 2}{t^2 + 1}dt = - \int (1 - \frac 2 {t^2 + 1})dt = -t + 2\arctg(t) + C = -\tg \frac x 2 + \frac {2x} 2 + C  
}$

  

---

  
  
$\mathsf  
{  
\int \frac{dx}{\sin^2x - 5\sin x \cdot \cos x} =  
\begin{vmatrix}  
\mathsf{t = \tg x} & \mathsf{x = \arctg t} \\  
\mathsf{dx = \frac{dt}{1 + t^2}} &  
\mathsf{\sin x = \frac t {\sqrt{1 + t^2}}} & \mathsf{\cos x = \frac 1 {\sqrt{1 + t^2}}}  
\end{vmatrix} =  
\int \frac{\frac{dt}{1 + t^2}}{\frac{t^2}{1 + t^2} - 5 \cdot(\frac t {\sqrt{1 + t^2}}) \cdot \frac 1 {\sqrt{1 + t^2}}} =  
\int \frac{\frac{dt}{1 + t^2}}{\frac{t^2 - 5t\sqrt{1 + t^2}}{1 + t^2}} =  
}$$\mathsf  
{  
\int \frac{dt}{t^2 - 5t} = \int \frac{dt}{(t - \frac 5 2)^2 - \frac{25} 4} =  
\int \frac{d(t - \frac 5 2}{(t - \frac 5 2)^2 - \frac {25} 4} =  
\frac{1}{5} \cdot \ln\begin{vmatrix}  
\mathsf{t - \frac 5 2 - \frac 5 2} \\ --- \\ \mathsf{t + \frac 5 2 + \frac 5 2}  
\end{vmatrix} + c =  
\frac{1}{5} \cdot \ln \begin{vmatrix}  
\mathsf{t - 5} \\ --- \\ \mathsf{t}  
\end{vmatrix} + c =  
\frac{1}{5} \ln  
\begin{vmatrix}  
\mathsf{\tg x - 5} \\ --- \\ \mathsf{\tg x}  
\end{vmatrix} + c  
}$

---

  

$\mathsf  
{  
\int \frac{dx}{\sin^2 x + 3 \sin x \cdot \cos x - \cos^2 x} =  
\begin{vmatrix}  
\mathsf{t = \tg x} & \mathsf{x = \arctg t} \\  
\mathsf{dx = \frac{dt}{1 + t^2}} & \mathsf{\sin x = \frac t {\sqrt{1 + t^2}}} & \mathsf{\cos x = \frac 1 {\sqrt{1 + t^2}}}  
\end{vmatrix} =  
}$