---
Редакторы: Artemii
Тэги:
  - II семестр
  - Практика
Статус: Готово
---
03/03/2023

$\mathsf  
{  
\frac{P_n(x)}{Q_m(x)} - \text{неправильная, если}\ n \ge m  
}$

$\mathsf  
{  
P_n(x), Q_m(x)  
}$ - многочлен степени n и m соответственно

  

$\mathsf  
{  
P_n(x) / Q_m(x) = \underset{\text{целая часть}}{S_{n - m}(x)} + \frac{\underset{\text{остаток}}{R_k(x)}}{Q_m(x)}  
}$

$\mathsf  
{  
k < m  
}$

  

$\mathsf  
{  
\int \frac{2x^4 + 5x^3 - 3x^2 + x - 7}{x - 3} dx =  
\int (2x^3 + 11x^2 + 30x + 91 + \frac{266}{x-3}) dx = \ldots \ (\text{Дальше идёт интегрирование)}  
}$

![[/Untitled 21.png|Untitled 21.png]]

  

---

  

$\mathsf  
{  
\int \frac{3x^4 - x^3 + 2x^2 + 3x + 5}{x^2 - 2}dx = \int(3x^2 - x + 8 + \frac{x + 21}{x^2 - 2})dx = ... (\text{Дальше идёт интегрирование})  
}$

  

---

  

$\mathsf  
{  
x^2 + px + q = \left ( x + \frac{p}{2}\right)^2 - \left ( \frac{p}{2} \right ) ^ 2 + q  
}$

$\mathsf  
{  
-x^2 + px + q = -\left(x - \frac{p}{2}\right)^2 + \left(\frac{p}{2} \right)^2 + q  
}$

  

---

  

$\mathsf  
{  
\int \frac{7dx}{3x^2 - 2x + 5} =  
\frac{7}{3}\int \frac{dx}{x^2 - \frac{2x}{3} + \frac{5}{3}} =  
\frac{7}{3} \int \frac{dx}{(x - \frac{1}{3})^2 - \frac{1}{9} + \frac{5}{3}} =  
\begin{vmatrix}  
\mathsf{t = x - \frac{1}{3}} \\  
\mathsf {dt = dx}  
\end{vmatrix} =  
\frac{7}{3}\int \frac{dt}{t^2 + \frac{14}{9}} =  
\frac{\sqrt{7}}{ \sqrt{2}} \arctg{}  
}$

  

---

  

$\mathsf  
{  
\int \frac{5x - 3}{6x - 2x^2 - 12}dx =  
-\frac{1}{2} \int \frac{5x - 3}{x^2 - 3x + 6} dx =  
- \frac{1}{2} \int \frac{5x - 3}{\left(x - \frac{3}{2}\right)^2 - \frac{9}{4}} dx =  
\begin{vmatrix}  
\mathsf{t = x - \frac{3}{2}} \\  
\mathsf{dt = dx} \\  
\mathsf{x = t + \frac{3}{2}}  
\end{vmatrix} =  
-\frac{1}{2} \int \frac{5(t + \frac{3}{2}) - 3}{t^2 + \frac{15}{4}}dt =  
-\frac{1}{2} \int \frac{5t}{t^2 + \frac{15}{4}}dt - \frac{1}{2} \int \frac{\frac{9}{2}}{t^2 + \frac{15}{4}}dt =  
-\frac{5}{2} * \frac{1}{2} \ln {t^2 + \frac{15}{4}}  
}$Не дорешено

---

  

$\mathsf  
{  
\int \frac{2dx}{\sqrt{3x - 3x^2 + 5}} =  
\frac{2}{\sqrt{3}} \int \frac{dx}{\sqrt{-x^2 + x + \frac{5}{3}}} =  
\frac{2}{\sqrt{3}} \int \frac{dx}{\sqrt{-(x - \frac 1 4 + \frac 5 3) }} =  
\begin{vmatrix}  
\mathsf{t = x - \frac 1 2} \\  
\mathsf {dt = dx}  
\end{vmatrix} =  
\frac 2 {\sqrt 3} \arcsin \left(\frac{t \sqrt {12}}{\sqrt{23}}\right) + c =  
\frac 2 {\sqrt 3} \arcsin \left(\frac{2 \sqrt 3 x - \sqrt 3}{\sqrt{23}}\right) + c  
}$