---
Ğ ĞµĞ´Ğ°ĞºÑ‚Ğ¾Ñ€Ñ‹: Artemii
Ğ¢ÑĞ³Ğ¸:
  - II ÑĞµĞ¼ĞµÑÑ‚Ñ€
  - ĞŸÑ€Ğ°ĞºÑ‚Ğ¸ĞºĞ°
Ğ”Ğ¾Ğ¿-Ñ€ĞµĞ´Ğ°ĞºÑ‚Ğ¾Ñ€Ñ‹: Fezwer
Ğ¡Ñ‚Ğ°Ñ‚ÑƒÑ: Ğ’ Ğ¿Ñ€Ğ¾Ñ†ĞµÑÑĞµ
---
$\mathsf  
{  
\overset{+\infin} {\underset a \int}f(x) dx = \underset{b \to +\infin} \lim \overset{b} {\underset a \int} f(x) dx  
}$

$\mathsf  
{  
\overset{b} {\underset {- \infin} \int}f(x) dx = \underset{a \to -\infin} \lim \overset{b} {\underset {- \infin} \int} f(x) dx  
}$

$\mathsf  
{  
\overset{+\infin} {\underset {- \infin} \int} f(x) dx= \overset{0} {\underset {- \infin} \int}f(x) dx + \overset{+\infin} {\underset {0} \int} f(x) dx  
}$

  

  

1. $\mathsf  
    {  
    \overset{+ \infin} {\underset 1 \int} \dfrac {dx} {x^4} = \underset{b \to +\infin}\lim \overset{b} {\underset 1 \int} \dfrac {dx} {x^4} = \underset{b \to +\infin}\lim \dfrac {x^{-3}}{-3} \overset{b} {\underset 1 \mid} = \underset{b \to +\infin} \lim (\dfrac{b^{-3}}{-3} + \dfrac 1 3) = \dfrac 1 3  
    }$
2. $\mathsf  
    {  
    \overset{+\infin} {\underset 2 \int}\dfrac {\ln(x)}x dx = \underset{b \to +\infin}\lim \overset{b} {\underset 2 \int} \dfrac{\ln(x)}x dx = \underset{b \to +\infin}\lim \overset{b} {\underset 2 \int} \ln(x) d(\ln(x)) = \underset{b \to +\infin}\lim \dfrac {\ln^2(x)} 2 \overset{b} {\underset 2 \mid} = \underset{b \to +\infin} \lim (\dfrac{\ln^2(b)} 2 - \dfrac{\ln^2(2)}2) = +\infin  
    }$

  
3. ğŸ”¥ğŸ”¥ğŸ”¥ğŸ”¥ğŸ”¥ğŸ”¥ğŸ”¥ğŸ”¥ğŸ”¥ğŸ”¥ğŸ”¥ğŸ”¥ğŸ”¥ğŸ”¥ğŸ”¥  

1. $\mathsf  
    {  
    \overset{+\infin} {\underset {0} \int} e^{-\sqrt x} \cdot dx = \underset{b \to +\infin} \lim \overset{b} {\underset {0} \int} e^{-\sqrt x} dx = \begin{vmatrix}  
    \mathsf{t = x^{\frac 1 2}} & \mathsf{x = 0 \implies t = 0} \\  
    \mathsf{x = t^2} & \mathsf{x = b \implies t = \sqrt b} \\  
    \mathsf{dx = 2t~ dt}  
    \end{vmatrix} = } \\  
    \mathsf{  
    \underset {b \to +\infin} \lim \overset{\sqrt b} {\underset {0} \int} e^{-t} 2t~dt =  
    \begin{vmatrix}  
    \mathsf{u = 2t} & \mathsf{du = 2dt} \\  
    \mathsf{dv = e^{-t} dt} & \mathsf{v = -e^{-t}}  
    \end{vmatrix} =  
    \underset{b \to +\infin}\lim (-2te^{-t} \overset{\sqrt b} {\underset {0} \int} + \overset{\sqrt b} {\underset {0} \int}e^{-t} \cdot 2dt) =  
    } \\  
    \mathsf  
    {  
    \underset{b \to +\infin}\lim(-2te^{-t} - 2e^{-t}) \overset{\sqrt b} {\underset {0} \mid} = \underset{b \to +\infin} \lim (-2 \sqrt b \dfrac 1 {e^{\sqrt b}} - 2 \dfrac {1}{e^{\sqrt b}} + 2) = 2  
    }$

![[IMG_20230523_125557.jpg]]