---
Редакторы: Artemii
Тэги:
  - Практика
Статус: Не начато
---
### №1

![[/Untitled 41.png|Untitled 41.png]]

$\mathsf{  
\begin{cases}  
\mathsf{y = \sqrt{12 - x^2}} \\  
\mathsf{y = 2 \sqrt 3 - \sqrt{12 - x^2}} \\  
\mathsf{x = 0 } & \mathsf{(x \ge 0)}  
\end{cases}  
}$

  

$\mathsf{\partial D = L_1 \cup L_2 \cup L_3}$

  

  

  

  

### №2

![[/Untitled 1 18.png|Untitled 1 18.png]]

$\mathsf{  
\underset 0 {\overset 1 \int} dx \underset{1 - x^2}{\overset 1 \int} f(x, y) dy + \overset e {\underset 1 \int} dx \overset 1 {\underset {\ln{x}} \int} f(x, y) dy = \underset {D_1} \iint f(x, y) dx dy + \underset{D_2} \iint f(x, y) dx dy  
}  
$

$\mathsf{D_1 = \left\{(x, y):\quad 0 \le x \le 1, \quad 1 - x^2 \le y \le 1 \right \} }$

$\mathsf{  
D_2 = \left\{(x, y):\quad 1 \le x \le e,\quad \ln(x) \le y \le 1\right\}  
}$

![[IMG_20231020_141253.jpg]]

  

  

### №3

$\mathsf{\underset V \iiint \dfrac{dxdydz}{(1 + x + y + z)^3} = \underset D \iint dxdy \underset 0 {\overset {1 - x - y} \int} \dfrac {dz}{(1 + x+ y+z)^3} = \underset D \iint dxdy \left(-\dfrac 1 {2(1 + x + y + z)^2} \underset{z = 0}{\overset{z = 1 - x - y}\mid}\right) =  
}$

$\mathsf{  
= \dfrac 1 2 \underset D \iint dxdy \left(\dfrac 1 {(1 + x + y)^2} - \dfrac 1 8\right) = \dfrac 1 2 \underset 0 {\overset 1 \int} dx \underset 0 {\overset{1 - x} \int} \left(1\right)  
}$