 **Лемма Келлога**
$$
A \ge 0 , \sigma \ge 0
$$
$$
\| (E-\sigma A)(E+\sigma A)^{-1} \|\le 1
$$
**Доказательство**
$$
\|(E-\sigma A)(E+\sigma A)\|^2 = \|T\|^2=\max_\phi \dfrac{(T\phi, T\phi)}{(\phi, \phi)}
$$
$$
(E+\sigma A)^{-1}\phi :=\psi
$$
$$
\|T\|^2 = \max_\psi \dfrac{((E-\sigma A) \psi, (E-\sigma A) \psi)}{((E+\sigma A) \psi, (E+\sigma A) \psi)}=\max_\psi \dfrac{(\psi, \psi) - 2\sigma (A\psi, psi)+\sigma^2(A\psi, A\psi)}{(\psi, \psi) + 2\sigma (A\psi, psi)+\sigma^2(A\psi, A\psi)} \le 1
$$


**Доказательство коммутативности**
$$
(E+\sigma A)^{-1} \quad (E-\sigma A)
$$
$$
\matrix{
{(E+\sigma A)(E-\sigma A) = E + \sigma^{2}A^{2}} \\
{(E-\sigma A)(E+\sigma A) = E + \sigma^{2}A^{2}}
} \implies (E+\sigma A)(E-\sigma A) = (E-\sigma A)(E+\sigma A)
$$
$$
\implies
(E-\sigma A)^{-1}(E-\sigma A)(E+\sigma A) = (E-\sigma A)^{-1}(E+\sigma A)(E-\sigma A)
$$
$$
\implies
(E+\sigma A) = (E-\sigma A)^{-1}(E+\sigma A)(E-\sigma A)
$$
$$
\implies
(E+\sigma A)(E-\sigma A)^{-1} = (E-\sigma A)^{-1}(E+\sigma A)(E-\sigma A)(E-\sigma A)^{-1}
$$
$$
\implies
(E+\sigma A)(E-\sigma A)^{-1} = (E-\sigma A)^{-1}(E+\sigma A)
$$



## Метод Кранка-Николсон
$$
\dfrac{\partial \phi}{\partial t} + A\phi = 0
$$
$$
\phi|_{t=0} = g
$$

$$\left[ t_{j}, t_{j + 1} \right],  \quad \phi^{0} = g $$
$$
\dfrac{\phi^{j + 1} - \phi^{j}}{\tau} + A \dfrac{\phi^{j + 1} + \phi^{j}}{2} = 0
$$

$$
\phi^{j+1}=\phi^j + \tau (\phi^j)'+\dfrac {\tau^2} 2 (\phi^2)''+O(\tau^3)
$$
$$
(\phi^{j})' + \dfrac \tau 2 (\phi^j)'' + O(\tau^2) + A\left( \phi^j + \dfrac \tau 2 (\phi^j)' + O(\tau^2) \right) = (\phi^j)' + A\phi^j + \dfrac \tau 2 ((\phi^j)''+A(\phi^j)') + O(\tau^2) = O(\tau^2)
$$



$$
(E+\dfrac \tau 2 A)\phi^{j+1} = (E- \dfrac \tau 2 A)\phi^j
$$
$$
\phi^{j+1} = (E+\dfrac \tau 2 A)^{-1}(E- \dfrac \tau 2 A)\phi^j
$$
$$
\|\phi^{j+1}\| \le \|(E+\dfrac \tau 2 A)^{-1}(E- \dfrac \tau 2 A)\| \cdot \|\phi^j\| \le \|\phi^j\|
$$
$$
\|T^{j}\| \leq 1
$$
$$
\|\phi^{j + 1}\| \leq \| \phi^{j}\|
$$


$$
\left( E +\frac{\tau}{2} A  \right) ^{ - 1} \left( E + \frac{\tau}{2}A \right) \left( E - \frac{\tau}{2} \right) \left( E + \frac{\tau}{2}A \right)  = \ldots
$$
$$
L\phi = \dfrac{\partial \phi}{\partial t} + A\phi
$$
$$
(L_{\tau}\phi)^j = \dfrac{(\phi)^{j+1} - (\phi)^j}{\tau} + \Lambda^j \dfrac{(\phi)^{j+1} + (\phi)^j}{2}
$$
$$
\|(L_\tau \phi) \| = \max_{t_j} \|(L_\tau \phi)^j\|
$$
$$
(\phi)^{j+1} = (\phi)^j + \tau (\phi_t)^j + \dfrac {\tau^2} 2 (\phi_{tt})^j + O(\tau^3)
$$
$$
\phi_t = -A\phi \quad \phi_{tt} = -A_t \phi - A\phi_t = A^2\phi-A_t \phi
$$
$$
(\phi)^{j+1} = (\phi)^j - \tau A^j(\phi)^j + \dfrac {\tau^2} 2 \left( (A^j)^2 - (A_t)^j \right) (\phi)^j + O(\tau^3)
$$
$$
\|L_\tau \phi \| = \left\|  \dfrac{(\phi)^j-\tau A^j (\phi)^j + \dfrac{\tau^2}{2} ((A^j)^2 (\phi)^j - A^j_t (\phi)^j) + O(\tau^3) - (\phi)^j}{\tau} \right\| + 
$$
$$
+ \Lambda^j \left\|  \dfrac {(\phi)^j - \tau A^j (\phi)^j + \dfrac{\tau^2}{2} ((A^j)^2 (\phi)^j - (A^{j}_t)(\phi)^j) + O(\tau^3) + (\phi)^j}{2} \right\| =
$$
$$
= \left\|-A^{j}\left( \phi \right) ^{j} + \dfrac \tau 2 \left[ \left( A^{j} \right) ^{2}\left( \phi \right) ^{j} - A^{j}_{t}\left( \phi \right)^{j}  \right] + O\left( \tau^{2} \right) + \Lambda^{j}\left( \phi \right) ^{j} - \frac{\tau}{2}\Lambda^{j}A^{j}\left( \phi \right) ^{j} + O\left( \tau^{2} \right) \right\| =
$$
$$
= \left\| \Lambda^j (\phi)^j - A^j (\phi)^j + \dfrac{\tau}{2} \left[ (A^j)^2 - A_t^j - \Lambda^j A^j \right] (\phi)^j + O\left( \tau^{2} \right) \right\| 
$$
$$
\Lambda^j = \left\{ A^{j+\frac 1 2}, \dfrac{A^j + A^{j+1}}{2}, A^j + \dfrac \tau 2 A_t^j \right\}
$$

$$
\dfrac{\partial \phi}{\partial t} + A\phi = f
$$
$$
f^j = f(t_{j+\frac 1 2})
$$

















































