---
Owner: Artemii
tags:
  - Практика
---
$\mathsf{  
a_0 y^{(n)} + a_1 y^{(n - 1)} + \ldots a_{n - 1}y' + a_n y = 0  
}$

$\mathsf{  
a_0 \lambda^n + \ldots + a_n = 0  
}$

  

Для корней первой кратности:

$\mathsf{  
Ce^{\lambda x}  
}$

Кратности k:

$\mathsf{  
P_{k - 1} = C_1+ C_2 x + \ldots + C_k x^{k - 1}  
}$

$\mathsf{  
P_{k - 1} e^{\lambda x}  
}$

Комплексные:

$\mathsf{  
P_{k - 1}e^{Re \lambda x} \cos(Im \lambda x) + Q_{k - 1} e^{Re \lambda x} \sin(Im \lambda x)  
}$

  

# №1

$\begin{cases}  
\mathsf{y'' - 2y' = 0} \\  
\mathsf{y(0) = 0} \\  
\mathsf{y'(0) = 2}  
\end{cases}$

  

$\mathsf{  
\lambda^2 - 2 \lambda = 0  
}$

$\mathsf{  
\lambda^2 = 2 \lambda; \quad \lambda_1 = 0  
}$

$\mathsf{  
\lambda_2 = 2  
}$

  

$\mathsf{  
y = C_1 e^{0x} + C_2e^{2x}  
}$

$\mathsf{  
0 = C_1 + C_2  
}$

$\mathsf{  
C_1 = -1  
}$

  

$\mathsf{  
y = -1 + e^{2x}  
}$

$\mathsf{  
y' = 2e^{2x}  
}$

$\mathsf{  
y'' = 4e^{2x}  
}$

  

$\mathsf{  
y' = 2C_2 e^{2x}  
}$

$\mathsf{  
C_2 = 1  
}$

  

# №2

$\mathsf{  
y'' - 4y' + 5y = 0  
}$

$\mathsf{  
\lambda^2 - 4\lambda + 5 = 0  
}$

$\mathsf{  
D = -4  
}$

$\mathsf{  
\lambda_{1, 2} = 2 \pm i  
}$

  

$\mathsf{  
y = C_1 e^{2x} \cos(x) + C_2 e^{2x} \sin(x)  
}$

  

# №3

$\mathsf{y'' + 4y = 0}$

$\mathsf{  
\lambda^2 + 4 = 0  
}$

$\mathsf{  
\lambda = \pm 2i  
}$

  

$\mathsf{  
C_1 e^{0x}\cos(2x) + C_2 e^{0x} \sin(2x)  
}$

# №4

_Фото_

![[IMG_20240507_122933.jpg]]

# №5

$\mathsf{  
x^2 y'' - 4xy' + 6y = 0  
}$

$\mathsf{  
x = e^t  
}$

$\mathsf{  
e^{2t} y'' - 4e^t y' + 6y = 0  
}$

$\mathsf{  
y'_x = y' t'_x = y' e^{-t}  
}$

$\mathsf{  
y''_x = y''e^{-2t} - y' e^{-t} - t'_x  
}$

$\mathsf{  
e^{2t} (y'' e^{-2t} - t'e^{-t}) - 4e^t \cdot y' e^{-t} + 6y = 0  
}$

$\mathsf{  
y'' - y' - 4y' + 6y = 0  
}$

$\mathsf{  
y'' - 5y' + 6y = 0  
}$

$\mathsf{  
p^2 - 5p + 6 = 0  
}$

$\mathsf{  
D = 1  
}$

$\mathsf{  
p_{1, 2} = 3, 2  
}$

$\mathsf{  
y = C_1 e^{2t} + C_2 e^{3t}  
}$

$\mathsf{  
y = C_1x^2 + C_2 x^3  
}$

$\mathsf{  
y' = 2C_1x + 3C_2x^2  
}$

$\mathsf{  
y'' = 2C_1 + 6C_2 x  
}$

$\mathsf{  
2C_1 x^2 + 6C_2 x^3 - 8C_1 x^2 - 12 C_2 x^3 + 6C_1 x^2 + 6C_2 x^3 = 0  
}$

# №6

$\mathsf{  
x^2 y'' - xy' - 3y = 0  
}$

  

$\mathsf{  
x^k y^{(k)} = \lambda (\lambda - 1) \ldots (\lambda -k + 1)  
}$

  

$\mathsf{  
\lambda(\lambda - 1) - \lambda - 3 = 0  
}$

  

_Фото 2_

![[IMG_20240507_125228.jpg]]

  

527 - 531

591, 592, 600