$\mathsf{ v_n \dfrac {(y_n - \mu)}{G} \overset{n \to \infin}\longrightarrow N(0, 1) }$

$\mathsf{ g(Y_n) \to N(g(\mu), (g'(\mu)^2 \dfrac{c^2}{n}) }$

  

$\mathsf{ \overline T_n = \dfrac 1 n \underset{i = 1}{\overset n \sum} T_i }$

$\mathsf{ E[\overline T_n] = E[T_1] = \dfrac 1 \lambda }$

$\mathsf{ D[\overline T_n] = \dfrac 1 {\lambda ^2} \cdot \dfrac 1 n }$

$\mathsf{ g(x) = \dfrac 1 \lambda \quad g'(x) = -\dfrac 1 {x^2} }$

$\mathsf{ E[g(\overline T_n)] = \lambda \implies g(\overline T_n) = \overline \lambda }$

$\mathsf{ \sqrt n (\overline T_n - \dfrac 1 \lambda) \implies N(0, \dfrac 1 {\lambda^2}) }$

  

$\mathsf{ (g'(\dfrac 1 \lambda))^2 = \lambda^4 }$

$\mathsf{ \sqrt n (g(\overline T_n) - g(\dfrac 1 \lambda)) \implies N(0, \lambda^2) }$